@prefix : <http://postdata.linhd.uned.es/ontology/postdata-poeticAnalysis#> .
@prefix owl: <http://www.w3.org/2002/07/owl#> .
@prefix rdf: <http://www.w3.org/1999/02/22-rdf-syntax-ns#> .
@prefix xml: <http://www.w3.org/XML/1998/namespace> .
@prefix xsd: <http://www.w3.org/2001/XMLSchema#> .
@prefix rdfs: <http://www.w3.org/2000/01/rdf-schema#> .
@base <http://postdata.linhd.uned.es/ontology/postdata-poeticAnalysis#> .

<http://postdata.linhd.uned.es/ontology/postdata-poeticAnalysis#> rdf:type owl:Ontology ;
                                                                   <http://purl.org/dc/elements/1.1/contributor> """Alvaro Pérez (LINHD_POSTDATA-UNED)
https://www.linkedin.com/in/álvaro-pérez-pozo-ab241154/"""@en ,
                                                                                                                 """Bruno Sartini (Bolonia University)
https://orcid.org/0000-0002-9152-4402"""@en ,
                                                                                                                 """Helena Bermúdez Sabel 
https://orcid.org/0000-0001-7782-206X"""@en ,
                                                                                                                 """Javier de la Rosa (LINHD_POSTDATA-UNED)
https://www.linkedin.com/in/versae/"""@en ,
                                                                                                                 """Laura Hernández (LINHD_POSTDATA-UNED)
https://orcid.org/0000-0003-3489-2193"""@en ,
                                                                                                                 """Mirella De Sisto (LINHD_POSTDATA-UNED)
mdesisto@scc.uned.es"""@en ,
                                                                                                                 """Mª Luisa Díez Platas 
https://orcid.org/0000-0002-9416-3147"""@en ,
                                                                                                                 """Omar Khalil Gómez
http://www.linkedin.com/in/omar-k-0959a8129"""@en ,
                                                                                                                 """Oscar Corcho (Universidad Politécnica de Madrid)
http://orcid.org/0000-0002-9260-0753"""@en ,
                                                                                                                 """Salvador Ros Muñoz (LINHD_POSTDATA-UNED)
srosmu@gmail.com"""@en ,
                                                                                                                 """Aitor Díaz Medina
https://www.linkedin.com/in/aitordiazmedina/""" ;
                                                                   <http://purl.org/dc/elements/1.1/contributors> """Alvaro Pérez (LINHD_POSTDATA-UNED)
https://www.linkedin.com/in/álvaro-pérez-pozo-ab241154/"""@en ,
                                                                                                                  """Bruno Sartini (Bolonia University)
https://orcid.org/0000-0002-9152-4402"""@en ;
                                                                   <http://purl.org/dc/elements/1.1/creator> "POSTDATA Project “This project has received funding from the European Research Council (ERC) under the European Union’s Horizon 2020 research and innovation programme (grant agreement Nº [679528])”"@en ;
                                                                   <http://purl.org/dc/elements/1.1/date> "2020-20-01" ;
                                                                   <http://purl.org/dc/elements/1.1/description> """This ontology module provides classes and properties to describe the structure of a Redaction in the context of POSTDATA project. The structure of a Redaction follows a logical break down of its elements: stanzas, lines, words and syllables. It can be useful in applications that require the annotation or retrieval of specific structural elements, which can be characterised by their own features or by their positions in relation to other elements.
This ontology also contains the classes and properties necessary to structure the information of a prosodic analysis, that is to say, the information obtained from the study of the meters and the forms of versification. In poetry, the metric is the basic rhythmic structure of the verses of a poetic work.
Finally, the ontology also provides classes and properties to support the annotation of different literary devices such acrostics, schemes or tropes."""@en ,
                                                                                                                 "This ontology supports the information necessary for the literary analysis of a poetic work. It focuses especially on rhetorical figures or figure of speech such as tropes and schemes."@en ;
                                                                   <http://purl.org/dc/elements/1.1/title> "postdata-poetic-analysis ontology"@en ;
                                                                   <http://purl.org/dc/terms/publisher> """POSTDATA Project

“This project has received funding from the European Research Council (ERC) under the European Union’s Horizon 2020 research and innovation programme (grant agreement Nº [679528])”
Principal Investigator. Elena González Blanco -- https://orcid.org/0000-0002-0448-1812
Technical Director. Salvador Ros Muñoz -- https://orcid.org/0000-0001-6330-4958"""@en ;
                                                                   <http://purl.org/vocab/vann/preferredNamespacePrefix> "pdp" ;
                                                                   owl:versionInfo "V2.0" ;
                                                                   <http://www.w3.org/2003/06/sw-vocab-status/ns#license> "https://creativecommons.org/licenses/by/4.0/"@en .

#################################################################
#    Annotation properties
#################################################################

###  http://creativecommons.org/ns#license
<http://creativecommons.org/ns#license> rdf:type owl:AnnotationProperty .


###  http://purl.org/dc/elements/1.1/contributor
<http://purl.org/dc/elements/1.1/contributor> rdf:type owl:AnnotationProperty .


###  http://purl.org/dc/elements/1.1/contributors
<http://purl.org/dc/elements/1.1/contributors> rdf:type owl:AnnotationProperty .


###  http://purl.org/dc/elements/1.1/creator
<http://purl.org/dc/elements/1.1/creator> rdf:type owl:AnnotationProperty .


###  http://purl.org/dc/elements/1.1/date
<http://purl.org/dc/elements/1.1/date> rdf:type owl:AnnotationProperty .


###  http://purl.org/dc/elements/1.1/description
<http://purl.org/dc/elements/1.1/description> rdf:type owl:AnnotationProperty .


###  http://purl.org/dc/elements/1.1/title
<http://purl.org/dc/elements/1.1/title> rdf:type owl:AnnotationProperty .


###  http://purl.org/dc/terms/publisher
<http://purl.org/dc/terms/publisher> rdf:type owl:AnnotationProperty .


###  http://purl.org/vocab/vann/preferredNamespacePrefix
<http://purl.org/vocab/vann/preferredNamespacePrefix> rdf:type owl:AnnotationProperty .


###  http://www.w3.org/2003/06/sw-vocab-status/ns#license
<http://www.w3.org/2003/06/sw-vocab-status/ns#license> rdf:type owl:AnnotationProperty .


#################################################################
#    Object Properties
#################################################################

###  http://postdata.linhd.uned.es/ontology/postdata-core#hasAgent
<http://postdata.linhd.uned.es/ontology/postdata-core#hasAgent> rdf:type owl:ObjectProperty ;
                                                                owl:inverseOf <http://postdata.linhd.uned.es/ontology/postdata-core#isAgentOf> ;
                                                                rdfs:domain <http://postdata.linhd.uned.es/ontology/postdata-core#AgentRole> ;
                                                                rdfs:range <http://postdata.linhd.uned.es/ontology/postdata-core#Agent> ;
                                                                rdfs:label "has agent"@en .


###  http://postdata.linhd.uned.es/ontology/postdata-core#hasAgentRole
<http://postdata.linhd.uned.es/ontology/postdata-core#hasAgentRole> rdf:type owl:ObjectProperty ;
                                                                    owl:inverseOf <http://postdata.linhd.uned.es/ontology/postdata-core#isAgentRoleOf> ;
                                                                    rdfs:domain :ScansionProcess ;
                                                                    rdfs:range <http://postdata.linhd.uned.es/ontology/postdata-core#AgentRole> ;
                                                                    rdfs:comment "This property points to the agent that participated in the scansion event."@en ;
                                                                    rdfs:label "has agent role"@en .


###  http://postdata.linhd.uned.es/ontology/postdata-core#isAgentOf
<http://postdata.linhd.uned.es/ontology/postdata-core#isAgentOf> rdf:type owl:ObjectProperty ;
                                                                 rdfs:domain <http://postdata.linhd.uned.es/ontology/postdata-core#Agent> ;
                                                                 rdfs:range <http://postdata.linhd.uned.es/ontology/postdata-core#AgentRole> ;
                                                                 rdfs:label "is agent of"@en .


###  http://postdata.linhd.uned.es/ontology/postdata-core#isAgentRoleOf
<http://postdata.linhd.uned.es/ontology/postdata-core#isAgentRoleOf> rdf:type owl:ObjectProperty ;
                                                                     rdfs:domain <http://postdata.linhd.uned.es/ontology/postdata-core#AgentRole> ;
                                                                     rdfs:range :ScansionProcess ;
                                                                     rdfs:label "is agent role of"@en .


###  http://postdata.linhd.uned.es/ontology/postdata-poeticAnalysis#affectsFirstWord
:affectsFirstWord rdf:type owl:ObjectProperty ;
                  owl:inverseOf :isFirstWordAffectedBy ;
                  rdfs:domain :Metaplasm ;
                  rdfs:range :Word ;
                  rdfs:comment """This property points to the first of the words affected by a metaplasm.

For example, if we consider the words \"sparse il\" in the line from the sonnet I from the Canzoniere by Petrarca, namely \"Voi ch'ascoltate in rime sparse il suono\", the first of the words being affected by a metaplasm (synaloepha in this case) is \"sparse\"."""@en ;
                  rdfs:isDefinedBy "http://postdata.linhd.uned.es/ontology/postdata-prosodicElements" ;
                  rdfs:label "affects first word"@en .


###  http://postdata.linhd.uned.es/ontology/postdata-poeticAnalysis#affectsLine
:affectsLine rdf:type owl:ObjectProperty ;
             owl:inverseOf :isLineAffectedBy ;
             rdfs:domain :Enjambment ;
             rdfs:range :Line ;
             rdfs:label "affects line" .


###  http://postdata.linhd.uned.es/ontology/postdata-poeticAnalysis#after
:after rdf:type owl:ObjectProperty ;
       rdfs:domain :Punctuation ;
       rdfs:range :Word ;
       rdfs:comment "This property relates a Punctuation List with its preceeding Word in a Line."@en ;
       rdfs:isDefinedBy "http://postdata.linhd.uned.es/ontology/postdata-poeticAnalysis#" ;
       rdfs:label "after"@en .


###  http://postdata.linhd.uned.es/ontology/postdata-poeticAnalysis#analyses
:analyses rdf:type owl:ObjectProperty ;
          owl:inverseOf :isAnalysedBy ;
          rdfs:domain :AnalyticalUnit ;
          rdfs:label "analyses" .


###  http://postdata.linhd.uned.es/ontology/postdata-poeticAnalysis#analysesFoot
:analysesFoot rdf:type owl:ObjectProperty ;
              rdfs:subPropertyOf :analyses ;
              owl:inverseOf :isFootAnalysedBy ;
              rdfs:domain :BasicAnalyticalUnit ;
              rdfs:range :Foot ;
              rdfs:label "analyses foot"@en .


###  http://postdata.linhd.uned.es/ontology/postdata-poeticAnalysis#analysesGrammaticalSyllable
:analysesGrammaticalSyllable rdf:type owl:ObjectProperty ;
                             rdfs:subPropertyOf :analyses ;
                             owl:inverseOf :isGrammaticalSyllableAnalysedBy ;
                             rdfs:domain :BasicAnalyticalUnit ;
                             rdfs:range :GrammaticalSyllable ;
                             rdfs:label "analyses grammatical syllable"@en .


###  http://postdata.linhd.uned.es/ontology/postdata-poeticAnalysis#analysesMetricalSyllable
:analysesMetricalSyllable rdf:type owl:ObjectProperty ;
                          rdfs:subPropertyOf :analyses ;
                          owl:inverseOf :isMetricalSyllableAnalysedBy ;
                          rdfs:domain :Mora ;
                          rdfs:range :MetricalSyllable ;
                          rdfs:label "analyses metrical syllable"@en .


###  http://postdata.linhd.uned.es/ontology/postdata-poeticAnalysis#analysesWord
:analysesWord rdf:type owl:ObjectProperty ;
              rdfs:subPropertyOf :analyses ;
              owl:inverseOf :isWordAnalysedBy ;
              rdfs:domain :AnalyticalUnit ;
              rdfs:range :Word ;
              rdfs:label "analyses word"@en .


###  http://postdata.linhd.uned.es/ontology/postdata-poeticAnalysis#before
:before rdf:type owl:ObjectProperty ;
        rdfs:domain :Punctuation ;
        rdfs:range :Word ;
        rdfs:comment "This property relates a Punctuation List with its proceeding Word in a Line."@en ;
        rdfs:isDefinedBy "http://postdata.linhd.uned.es/ontology/postdata-poeticAnalysis#" ;
        rdfs:label "before"@en .


###  http://postdata.linhd.uned.es/ontology/postdata-poeticAnalysis#clausula
:clausula rdf:type owl:ObjectProperty ;
          rdfs:domain :Foot ;
          rdfs:range <http://www.w3.org/2004/02/skos/core#Concept> ,
                     [ rdf:type owl:Restriction ;
                       owl:onProperty <http://www.w3.org/2004/02/skos/core#inScheme> ;
                       owl:hasValue <http://postdata.linhd.uned.es/kos/clausula>
                     ] ;
          rdfs:comment """The categorisation of the item according to the rhythmic ending of a line  determined by the number of unstressed syllables following the last stressed one. This property is both valid for accentual and syllabic versification, so possible values include: masculine (zero syllables), femenine (one), dactylic, proparoxitone, etc.

For example, if we consider the final foot of the line from sonnet I by Shakespeare \"From fairest creatures we desire increase\", namely \"|increase|, the clausula is: masculine."""@en ;
          rdfs:isDefinedBy "http://postdata.linhd.uned.es/ontology/postdata-prosodicElements#clausula"@en ;
          rdfs:label "clausula"@en .


###  http://postdata.linhd.uned.es/ontology/postdata-poeticAnalysis#clausulaSchemeType
:clausulaSchemeType rdf:type owl:ObjectProperty ;
                    rdfs:domain :StanzaPattern ;
                    rdfs:range <http://www.w3.org/2004/02/skos/core#Concept> ,
                               [ rdf:type owl:Restriction ;
                                 owl:onProperty <http://www.w3.org/2004/02/skos/core#inScheme> ;
                                 owl:hasValue <http://postdata.linhd.uned.es/kos/clausulaScheme-type>
                               ] ;
                    rdfs:comment """Categorisation of the stanza according to the distribution of clausulae/gender of rhymes (eg. “classic”, “heterogonique”, etc.).

For example, if we consider the first stanza of the sonnet I of Canzoniere by Petrarca, namely: \"Voi ch’ascoltate in rime sparse il suono/ di quei sospiri ond’io nudriva ’l core / in sul mio primo giovenile errore/ quand’era in parte altr’uom da quel ch’i’ sono\" clausulaSchemeType is \"Feminine rhyme\"."""@en ;
                    rdfs:isDefinedBy "http://postdata.linhd.uned.es/ontology/postdata-prosodicElements"@en ;
                    rdfs:label "clausula scheme type"@en .


###  http://postdata.linhd.uned.es/ontology/postdata-poeticAnalysis#employedTechnique
:employedTechnique rdf:type owl:ObjectProperty ;
                   rdfs:domain :ScansionProcess ;
                   rdfs:range <http://www.w3.org/2004/02/skos/core#Concept> ;
                   rdfs:comment "Indicates which methodology or analytical technique has been applied to perform the scansion."@en ;
                   rdfs:label "employed technique"@en .


###  http://postdata.linhd.uned.es/ontology/postdata-poeticAnalysis#employs
:employs rdf:type owl:ObjectProperty ;
         owl:inverseOf :isEmployedIn ;
         rdfs:domain :MetricalEncoding ;
         rdfs:range :Symbol ;
         rdfs:comment """This propery points to a Symbol used in metrical notation being defined.

For example, if we consider the LinePattern \"-+-+-+-+-+\" of the line \"From fairest creatures we desire increase,\" from the first sonnet by Shakespeare, the MetricalEncoding employs the Symbol \"+\" to mark a stressed syllable or metrical position."""@en ;
         rdfs:isDefinedBy "http://postdata.linhd.uned.es/ontology/postdata-prosodicElements"@en ;
         rdfs:label "employs"@en .


###  http://postdata.linhd.uned.es/ontology/postdata-poeticAnalysis#feetType
:feetType rdf:type owl:ObjectProperty ;
          rdfs:domain :LinePattern ;
          rdfs:range <http://www.w3.org/2004/02/skos/core#Concept> ,
                     [ rdf:type owl:Restriction ;
                       owl:onProperty <http://www.w3.org/2004/02/skos/core#inScheme> ;
                       owl:hasValue <http://postdata.linhd.uned.es/kos/feet-type>
                     ] ;
          rdfs:comment """Categorisation of the stanza or line according to the type of feet.

For example, if we consider the first line of the sonnet I by Shakespeare \"From fairest creatures we desire increase\", feetType is \"iamb\"."""@en ;
          rdfs:isDefinedBy "http://postdata.linhd.uned.es/ontology/postdata-prosodicElements"@en ;
          rdfs:label "feet type"@en .


###  http://postdata.linhd.uned.es/ontology/postdata-poeticAnalysis#firstFoot
:firstFoot rdf:type owl:ObjectProperty ;
           rdfs:subPropertyOf <http://purl.org/ontology/olo/core#has_first_slot> ;
           owl:inverseOf :firstFootOf ;
           rdfs:domain :FootList ;
           rdfs:range :Foot ;
           <http://purl.org/dc/elements/1.1/creator> "mluisadiez" ;
           <http://purl.org/dc/elements/1.1/date> "2018-06-16T20:30:43Z"^^xsd:dateTime ;
           rdfs:comment """This property points to the first Foot of the line.

For example, if we consider the first line of the sonnet I by Shakespeare \"From fairest creatures we desire increase\", this has |from fai| as first foot.""" ;
           rdfs:isDefinedBy "http://postdata.linhd.uned.es/ontology/postdata-prosodicElements"@en ;
           rdfs:label "first foot"@en .


###  http://postdata.linhd.uned.es/ontology/postdata-poeticAnalysis#firstFootOf
:firstFootOf rdf:type owl:ObjectProperty ;
             rdfs:subPropertyOf <http://purl.org/ontology/olo/core#is_first_slot_of> ;
             rdfs:domain :Foot ;
             rdfs:range :FootList ;
             rdfs:comment """This property points to the LinePattern whose feet description begins with the current item under analysis.

For example, if we consider the first line of the sonnet I by Shakespeare \"From fairest creatures we desire increase\", |from fai| is its first foot."""@en ;
             rdfs:isDefinedBy "http://postdata.linhd.uned.es/ontology/postdata-prosodicElements"@en ;
             rdfs:label "first foot of"@en .


###  http://postdata.linhd.uned.es/ontology/postdata-poeticAnalysis#firstGrammaticalSyllable
:firstGrammaticalSyllable rdf:type owl:ObjectProperty ;
                          rdfs:subPropertyOf <http://purl.org/ontology/olo/core#has_first_slot> ;
                          owl:inverseOf :firstGrammaticalSyllableOf ;
                          rdfs:domain :GrammaticalSyllableList ;
                          rdfs:range :GrammaticalSyllable ;
                          rdfs:comment """This property points to the first Syllable of a Word.

For instance, the first syllable of the word \"derrota\" is \"der\"."""@en ;
                          rdfs:isDefinedBy "http://postdata.linhd.uned.es/ontology/postdata-poeticAnalysis#" ;
                          rdfs:label "first grammatical syllable"@en .


###  http://postdata.linhd.uned.es/ontology/postdata-poeticAnalysis#firstGrammaticalSyllableOf
:firstGrammaticalSyllableOf rdf:type owl:ObjectProperty ;
                            rdfs:subPropertyOf <http://purl.org/ontology/olo/core#is_first_slot_of> ;
                            rdfs:domain :GrammaticalSyllable ;
                            rdfs:range :GrammaticalSyllableList ;
                            rdfs:comment """This property points to an instance of Word of which a given Syllable is its first element.

For example, \"ar\" isFirstSyllable of the word \"árbol\"."""@en ;
                            rdfs:isDefinedBy "http://postdata.linhd.uned.es/ontology/postdata-poeticAnalysis#" ;
                            rdfs:label "first grammatical syllable of"@en ,
                                       "is first syllable of"@en .


###  http://postdata.linhd.uned.es/ontology/postdata-poeticAnalysis#firstLine
:firstLine rdf:type owl:ObjectProperty ;
           rdfs:subPropertyOf <http://purl.org/ontology/olo/core#has_first_slot> ;
           owl:inverseOf :firstLineOf ;
           rdfs:domain :LineList ;
           rdfs:range :Line ;
           rdfs:comment """This property points to the first Line which forms part of a given Line List.

For example, if we consider the second stanza of the poem \"Calle de Arrabal\" by Dámaso Alonso (i.e. \"A un lado, hay un calvero de solares/ en frente, están las casas alineadas/ porque esperan que de un momento a otro/ la Primavera pasará\"), the first line is \"A un lado, hay un calvero de solares\".""" ;
           rdfs:isDefinedBy "http://postdata.linhd.uned.es/ontology/postdata-poeticAnalysis#" ;
           rdfs:label "first line"@en .


###  http://postdata.linhd.uned.es/ontology/postdata-poeticAnalysis#firstLineOf
:firstLineOf rdf:type owl:ObjectProperty ;
             rdfs:subPropertyOf <http://purl.org/ontology/olo/core#is_first_slot_of> ;
             rdfs:domain :Line ;
             rdfs:range :LineList ;
             rdfs:comment """This property points to the Line List of which the current Line under analysis is its first item.

For example, \"Voi ch'ascoltate in rime sparse il suono\" is the first line of the first stanza of the first sonnet of the \"Canzoniere\" by Francesco Petrarca."""@en ;
             rdfs:isDefinedBy "http://postdata.linhd.uned.es/ontology/postdata-poeticAnalysis#" ;
             rdfs:label "first line of"@en .


###  http://postdata.linhd.uned.es/ontology/postdata-poeticAnalysis#firstMetricalSyllable
:firstMetricalSyllable rdf:type owl:ObjectProperty ;
                       rdfs:subPropertyOf <http://purl.org/ontology/olo/core#has_first_slot> ;
                       owl:inverseOf :firstMetricalSyllableOf ;
                       rdfs:domain :MetricalSyllableList ;
                       rdfs:range :MetricalSyllable ;
                       rdfs:label "first metrical syllable"@en .


###  http://postdata.linhd.uned.es/ontology/postdata-poeticAnalysis#firstMetricalSyllableOf
:firstMetricalSyllableOf rdf:type owl:ObjectProperty ;
                         rdfs:subPropertyOf <http://purl.org/ontology/olo/core#is_first_slot_of> ;
                         rdfs:domain :MetricalSyllable ;
                         rdfs:range :MetricalSyllableList ;
                         rdfs:label "first metrical syllable of"@en .


###  http://postdata.linhd.uned.es/ontology/postdata-poeticAnalysis#firstMora
:firstMora rdf:type owl:ObjectProperty ;
           rdfs:subPropertyOf <http://purl.org/ontology/olo/core#has_first_slot> ;
           owl:inverseOf :firstMoraOf ;
           rdfs:domain :MoraList ;
           rdfs:range :Mora ;
           rdfs:comment """This property points to the firt unit in which the foot is divided (an instance of FootDivision).

For example, if we consider the first foot of the first line of the sonnet I by Shakespeare \"From fairest creatures we desire increase\", namely |from fai|, this foot has \"from\" has its first unit."""@en ;
           rdfs:isDefinedBy "http://postdata.linhd.uned.es/ontology/postdata-prosodicElements"@en ;
           rdfs:label "first mora"@en .


###  http://postdata.linhd.uned.es/ontology/postdata-poeticAnalysis#firstMoraOf
:firstMoraOf rdf:type owl:ObjectProperty ;
             rdfs:subPropertyOf <http://purl.org/ontology/olo/core#is_first_slot_of> ;
             rdfs:domain :Mora ;
             rdfs:range :MoraList ;
             rdfs:comment """This property points to the Foot that contains the item at hand as its first element.

For example, if we consider the first foot of the first line of the sonnet I by Shakespeare \"From fairest creatures we desire increase\", namely |from fai|, its first unit  is \"from\"."""@en ;
             rdfs:isDefinedBy "http://postdata.linhd.uned.es/ontology/postdata-prosodicElements"@en ;
             rdfs:label "first mora of"@en .


###  http://postdata.linhd.uned.es/ontology/postdata-poeticAnalysis#firstPunctuation
:firstPunctuation rdf:type owl:ObjectProperty ;
                  rdfs:subPropertyOf <http://purl.org/ontology/olo/core#has_first_slot> ;
                  owl:inverseOf :firstPunctuationOf ;
                  rdfs:domain :PunctuationList ;
                  rdfs:range :Punctuation ;
                  rdfs:comment "This property points to the first Punctuation which forms part of a given Punctuation List."@en ;
                  rdfs:isDefinedBy "http://postdata.linhd.uned.es/ontology/postdata-poeticAnalysis#" ;
                  rdfs:label "first punctuation"@en .


###  http://postdata.linhd.uned.es/ontology/postdata-poeticAnalysis#firstPunctuationOf
:firstPunctuationOf rdf:type owl:ObjectProperty ;
                    rdfs:subPropertyOf <http://purl.org/ontology/olo/core#is_first_slot_of> ;
                    rdfs:domain :Punctuation ;
                    rdfs:range :PunctuationList ;
                    rdfs:comment "This property points to the Punctuation List for which a given Punctuation is its first element."@en ;
                    rdfs:isDefinedBy "http://postdata.linhd.uned.es/ontology/postdata-poeticAnalysis#" ;
                    rdfs:label "first punctuation of"@en .


###  http://postdata.linhd.uned.es/ontology/postdata-poeticAnalysis#firstStanza
:firstStanza rdf:type owl:ObjectProperty ;
             rdfs:subPropertyOf <http://purl.org/ontology/olo/core#has_first_slot> ;
             owl:inverseOf :firstStanzaOf ;
             rdfs:domain :StanzaList ;
             rdfs:range :Stanza ;
             rdfs:comment """This property points to the first Stanza which forms part of a given Stanza List.

For example, the poem \"Poema 20\" by Pablo Neruda has as first stanza \"Puedo escribir los versos más tristes esta noche. / Escribir, por ejemplo: \"―La noche esta estrellada, / y tiritan, azules, los astros, a lo lejos\"."""@en ;
             rdfs:isDefinedBy "http://postdata.linhd.uned.es/ontology/postdata-poeticAnalysis#" ;
             rdfs:label "first stanza"@en .


###  http://postdata.linhd.uned.es/ontology/postdata-poeticAnalysis#firstStanzaOf
:firstStanzaOf rdf:type owl:ObjectProperty ;
               rdfs:subPropertyOf <http://purl.org/ontology/olo/core#is_first_slot_of> ;
               rdfs:domain :Stanza ;
               rdfs:range :StanzaList ;
               rdfs:comment """This property points to the Stanza List of which the current Stanza under analysis is its first line grouping.

For example, \"Señor Don Juan, quedito, que me enfado:/ besar la mano es mucho atrevimiento; / abrazarme... no, Juan, no lo consiento.  / Cosquillas... ay Juanito... ¿y el pecado?\" is the first stanza of the poem \"El mismo\" by Tomás de Iriarte."""@en ;
               rdfs:isDefinedBy "http://postdata.linhd.uned.es/ontology/postdata-poeticAnalysis#" ;
               rdfs:label "first stanza of"@en .


###  http://postdata.linhd.uned.es/ontology/postdata-poeticAnalysis#firstWord
:firstWord rdf:type owl:ObjectProperty ;
           rdfs:subPropertyOf <http://purl.org/ontology/olo/core#has_first_slot> ;
           owl:inverseOf :firstWordOf ;
           rdfs:domain :WordList ;
           rdfs:range :Word ;
           rdfs:comment """This property points to the first Word of a given Line.

For example, \"voi\" is the first token of the line \"Voi ch'ascoltate in rime sparse il suono\" from the first sonnet of the \"Canzoniere\" by Francesco Petrarca."""@en ;
           rdfs:isDefinedBy "http://postdata.linhd.uned.es/ontology/postdata-poeticAnalysis#" ;
           rdfs:label "first word"@en .


###  http://postdata.linhd.uned.es/ontology/postdata-poeticAnalysis#firstWordOf
:firstWordOf rdf:type owl:ObjectProperty ;
             rdfs:subPropertyOf <http://purl.org/ontology/olo/core#is_first_slot_of> ;
             rdfs:domain :Word ;
             rdfs:range :WordList ;
             rdfs:comment """This property points to an instance of Line of which a given Word is its first element.

For example, if we consider the fifth stanza of the poem \"Ho bisogno di silenzio\" by Alda Merini, \"Chi di parole da me ne ha avute tante\" is the first token.""" ;
             rdfs:isDefinedBy "http://postdata.linhd.uned.es/ontology/postdata-poeticAnalysis#" ;
             rdfs:label "first word of"@en .


###  http://postdata.linhd.uned.es/ontology/postdata-poeticAnalysis#foot
:foot rdf:type owl:ObjectProperty ;
      rdfs:subPropertyOf <http://purl.org/ontology/olo/core#slot> ;
      owl:inverseOf :footList ;
      rdfs:domain :FootList ;
      rdfs:range :Foot ;
      rdfs:label "foot"@en .


###  http://postdata.linhd.uned.es/ontology/postdata-poeticAnalysis#footList
:footList rdf:type owl:ObjectProperty ;
          rdfs:subPropertyOf <http://purl.org/ontology/olo/core#ordered_list> ;
          rdfs:domain :Foot ;
          rdfs:range :FootList ;
          rdfs:label "foot list"@en .


###  http://postdata.linhd.uned.es/ontology/postdata-poeticAnalysis#footType
:footType rdf:type owl:ObjectProperty ;
          rdfs:domain :Foot ;
          rdfs:range <http://www.w3.org/2004/02/skos/core#Concept> ,
                     [ rdf:type owl:Restriction ;
                       owl:onProperty <http://www.w3.org/2004/02/skos/core#inScheme> ;
                       owl:hasValue <http://postdata.linhd.uned.es/kos/foot-type>
                     ] ;
          rdfs:comment """Type of foot (e.g. iamb).

For example, if we consider the final foot of the verse from sonnet I by Shakespeare \"From fairest creatures we desire increase\", namely \"|increase|, footType is \"iamb\"."""@en ;
          rdfs:isDefinedBy "http://postdata.linhd.uned.es/ontology/postdata-prosodicElements"@en ;
          rdfs:label "foot type"@en .


###  http://postdata.linhd.uned.es/ontology/postdata-poeticAnalysis#generated
:generated rdf:type owl:ObjectProperty ;
           owl:inverseOf :isGeneratedBy ;
           rdfs:domain :ScansionProcess ;
           rdfs:range :Scansion .


###  http://postdata.linhd.uned.es/ontology/postdata-poeticAnalysis#grammaticalSyllable
:grammaticalSyllable rdf:type owl:ObjectProperty ;
                     rdfs:subPropertyOf <http://purl.org/ontology/olo/core#slot> ;
                     owl:inverseOf :grammaticalSyllableList ;
                     rdfs:domain :GrammaticalSyllableList ;
                     rdfs:range :GrammaticalSyllable ;
                     rdfs:comment "Syllable of a Word considered as list"@en ;
                     rdfs:isDefinedBy "http://postdata.linhd.uned.es/ontology/postdata-poeticAnalysis#" ;
                     rdfs:label "grammatical syllable"@en .


###  http://postdata.linhd.uned.es/ontology/postdata-poeticAnalysis#grammaticalSyllableList
:grammaticalSyllableList rdf:type owl:ObjectProperty ;
                         rdfs:subPropertyOf <http://purl.org/ontology/olo/core#ordered_list> ;
                         rdfs:domain :GrammaticalSyllable ;
                         rdfs:range :GrammaticalSyllableList ;
                         rdfs:comment """This property refers to the Word a given Syllable belongs to.

For example, the syllable \"ma\" belongs to the word \"Lágrima\"."""@en ;
                         rdfs:isDefinedBy "http://postdata.linhd.uned.es/ontology/postdata-poeticAnalysis#" ;
                         rdfs:label "grammatical syllable list"@en .


###  http://postdata.linhd.uned.es/ontology/postdata-poeticAnalysis#hasAnnotation
:hasAnnotation rdf:type owl:ObjectProperty ;
               owl:inverseOf :isAnnotationOf ;
               rdfs:domain :Scansion ;
               rdfs:label "has annotation"@en .


###  http://postdata.linhd.uned.es/ontology/postdata-poeticAnalysis#hasDeviceAnnotation
:hasDeviceAnnotation rdf:type owl:ObjectProperty ;
                     rdfs:subPropertyOf :hasAnnotation ;
                     owl:inverseOf :isDeviceAnnotationOf ;
                     rdfs:domain :Scansion ;
                     rdfs:range :LiteraryDevice ;
                     rdfs:label "has device annotation"@en .


###  http://postdata.linhd.uned.es/ontology/postdata-poeticAnalysis#hasEndingLine
:hasEndingLine rdf:type owl:ObjectProperty ;
               owl:inverseOf :isEndingLineOf ;
               rdfs:domain <http://postdata.linhd.uned.es/ontology/postdata-core#Excerpt> ;
               rdfs:range :Line ;
               rdfs:label "has ending line"@en .


###  http://postdata.linhd.uned.es/ontology/postdata-poeticAnalysis#hasFoot
:hasFoot rdf:type owl:ObjectProperty ;
         rdfs:subPropertyOf :hasPart ;
         owl:inverseOf :isFootOf ;
         rdfs:domain :Line ;
         rdfs:range :Foot ;
         rdfs:label "has foot"@en .


###  http://postdata.linhd.uned.es/ontology/postdata-poeticAnalysis#hasFootList
:hasFootList rdf:type owl:ObjectProperty ;
             rdfs:subPropertyOf :hasList ;
             owl:inverseOf :isFootListOf ;
             rdfs:domain :LinePattern ;
             rdfs:range :FootList ;
             rdfs:label "has foot list"@en .


###  http://postdata.linhd.uned.es/ontology/postdata-poeticAnalysis#hasGrammaticalSyllable
:hasGrammaticalSyllable rdf:type owl:ObjectProperty ;
                        rdfs:subPropertyOf :hasPart ;
                        owl:inverseOf :isGrammaticalSyllableOf ;
                        rdfs:domain :Line ;
                        rdfs:range :GrammaticalSyllable ;
                        rdfs:label "has grammatical syllable"@en .


###  http://postdata.linhd.uned.es/ontology/postdata-poeticAnalysis#hasGrammaticalSyllableList
:hasGrammaticalSyllableList rdf:type owl:ObjectProperty ;
                            rdfs:subPropertyOf :hasList ;
                            owl:inverseOf :isGrammaticalSyllableListOf ;
                            rdfs:domain :Line ;
                            rdfs:range :GrammaticalSyllableList ;
                            rdfs:label "has grammatical syllable list"@en .


###  http://postdata.linhd.uned.es/ontology/postdata-poeticAnalysis#hasLine
:hasLine rdf:type owl:ObjectProperty ;
         rdfs:subPropertyOf :hasPart ;
         owl:inverseOf :isLineOf ;
         rdfs:domain :Stanza ;
         rdfs:range :Line ;
         rdfs:label "has line"@en .


###  http://postdata.linhd.uned.es/ontology/postdata-poeticAnalysis#hasLineList
:hasLineList rdf:type owl:ObjectProperty ;
             rdfs:subPropertyOf :hasList ;
             owl:inverseOf :isLineListOf ;
             rdfs:domain :Stanza ;
             rdfs:range :LineList ;
             rdfs:comment "This property points to the Line List that conforms a Redaction."@en ;
             rdfs:isDefinedBy "http://postdata.linhd.uned.es/ontology/postdata-poeticAnalysis#" ;
             rdfs:label "has line list"@en .


###  http://postdata.linhd.uned.es/ontology/postdata-poeticAnalysis#hasLinePattern
:hasLinePattern rdf:type owl:ObjectProperty ;
                rdfs:subPropertyOf :hasPattern ;
                owl:inverseOf :isLinePatternOf ;
                rdfs:domain :Line ;
                rdfs:range :LinePattern ;
                rdfs:comment """This property points to an instance of Line about which the item at hand presents analytical information.

For example, the Line Pattern \"---+-+---+-\" analyses the first line of the poem \"Osé y temí, mas pudo la osadía tanto\" by Fernando de Herrera."""@en ;
                rdfs:isDefinedBy "http://postdata.linhd.uned.es/ontology/postdata-prosodicElements"@en ;
                rdfs:label "has line pattern"@en .


###  http://postdata.linhd.uned.es/ontology/postdata-poeticAnalysis#hasList
:hasList rdf:type owl:ObjectProperty ;
         owl:inverseOf :isListOf ;
         rdfs:range <http://purl.org/ontology/olo/core#OrderedList> ;
         rdfs:label "has list"@en .


###  http://postdata.linhd.uned.es/ontology/postdata-poeticAnalysis#hasListAnnotation
:hasListAnnotation rdf:type owl:ObjectProperty ;
                   rdfs:subPropertyOf :hasAnnotation ;
                   owl:inverseOf :isListAnnotationOf ;
                   rdfs:domain :Scansion ;
                   rdfs:range <http://purl.org/ontology/olo/core#OrderedList> ;
                   rdfs:label "has list annotation"@en .


###  http://postdata.linhd.uned.es/ontology/postdata-poeticAnalysis#hasMetricalSyllable
:hasMetricalSyllable rdf:type owl:ObjectProperty ;
                     rdfs:subPropertyOf :hasPart ;
                     owl:inverseOf :isMetricalSyllableOf ;
                     rdfs:domain :Line ;
                     rdfs:range :MetricalSyllable ;
                     rdfs:label "has metrical syllable"@en .


###  http://postdata.linhd.uned.es/ontology/postdata-poeticAnalysis#hasMetricalSyllableList
:hasMetricalSyllableList rdf:type owl:ObjectProperty ;
                         rdfs:subPropertyOf :hasList ;
                         owl:inverseOf :isMetricalSyllableListOf ;
                         rdfs:domain :Line ;
                         rdfs:range :MetricalSyllableList ;
                         rdfs:label "has metrical syllable list"@en .


###  http://postdata.linhd.uned.es/ontology/postdata-poeticAnalysis#hasMora
:hasMora rdf:type owl:ObjectProperty ;
         rdfs:subPropertyOf :hasPart ;
         owl:inverseOf :isMoraOf ;
         rdfs:domain :Line ;
         rdfs:range :Mora ;
         rdfs:label "has mora"@en .


###  http://postdata.linhd.uned.es/ontology/postdata-poeticAnalysis#hasMoraList
:hasMoraList rdf:type owl:ObjectProperty ;
             rdfs:subPropertyOf :hasList ;
             owl:inverseOf :isMoraListOf ;
             rdfs:domain :LinePattern ;
             rdfs:range :MoraList ;
             rdfs:label "has mora list"@en .


###  http://postdata.linhd.uned.es/ontology/postdata-poeticAnalysis#hasPart
:hasPart rdf:type owl:ObjectProperty ;
         owl:inverseOf :isPartOf ;
         rdfs:domain :StructuralUnit ;
         rdfs:range :StructuralUnit ;
         rdfs:label "has part"@en .


###  http://postdata.linhd.uned.es/ontology/postdata-poeticAnalysis#hasPattern
:hasPattern rdf:type owl:ObjectProperty ;
            owl:inverseOf :isPatternOf ;
            rdfs:range :Pattern ;
            rdfs:comment """This property points to an instance of Redaction in which a WorkPattern, StanzaPattern or LinePattern presents analytical information about the work as a whole, the stanzas or the lines, respectively.

For example, all the metrical information contained in the WorkPattern, the StanzaPattern or the LinePattern analyses the poem in its present Redaction. As a result, all this metrical data is bound to change if a different Redaction of the poem is used. For example, if we take Herrera's poem \"Oh soberbia y cruel en tu belleza\", the LinePattern of the nith line in the 1582 version is \"-+-+---+-+-\", while in the 1619 version the line changes and consequently shows a new LinePattern: \"-+---+---+-\"""" ;
            rdfs:isDefinedBy "http://postdata.linhd.uned.es/ontology/postdata-prosodicElements"@en ;
            rdfs:label "has pattern"@en .


###  http://postdata.linhd.uned.es/ontology/postdata-poeticAnalysis#hasPatternAnnotation
:hasPatternAnnotation rdf:type owl:ObjectProperty ;
                      rdfs:subPropertyOf :hasAnnotation ;
                      owl:inverseOf :isPatternAnnotationOf ;
                      rdfs:domain :Scansion ;
                      rdfs:range :Pattern ;
                      rdfs:label "has pattern annotation"@en .


###  http://postdata.linhd.uned.es/ontology/postdata-poeticAnalysis#hasPunctuation
:hasPunctuation rdf:type owl:ObjectProperty ;
                rdfs:subPropertyOf :hasPart ;
                owl:inverseOf :isPunctuationOf ;
                rdfs:domain :Line ;
                rdfs:range :Punctuation ;
                rdfs:label "has punctuation"@en .


###  http://postdata.linhd.uned.es/ontology/postdata-poeticAnalysis#hasPunctuationList
:hasPunctuationList rdf:type owl:ObjectProperty ;
                    rdfs:subPropertyOf :hasList ;
                    owl:inverseOf :isPunctuationListOf ;
                    rdfs:domain :Line ;
                    rdfs:range :PunctuationList ;
                    rdfs:comment "This property points to the Punctuation List containing the punctuations present in a Line."@en ;
                    rdfs:isDefinedBy "http://postdata.linhd.uned.es/ontology/postdata-poeticAnalysis#" ;
                    rdfs:label "has punctuation list"@en .


###  http://postdata.linhd.uned.es/ontology/postdata-poeticAnalysis#hasRedactionPattern
:hasRedactionPattern rdf:type owl:ObjectProperty ;
                     rdfs:subPropertyOf :hasPattern ;
                     owl:inverseOf :isRedactionPatternOf ;
                     rdfs:domain :Scansion ;
                     rdfs:range :RedactionPattern ;
                     rdfs:label "has redaction pattern"@en .


###  http://postdata.linhd.uned.es/ontology/postdata-poeticAnalysis#hasRhyme
:hasRhyme rdf:type owl:ObjectProperty ;
          rdfs:subPropertyOf owl:topObjectProperty ;
          owl:inverseOf :isRhymeOf ;
          rdfs:domain :StructuralUnit ;
          rdfs:range :Rhyme ;
          <http://purl.org/dc/elements/1.1/creator> "mluisadiez" ;
          <http://purl.org/dc/elements/1.1/date> "2018-06-16T20:30:43Z"^^xsd:dateTime ;
          rdfs:comment """This property points to an instance of Rhyme that is contained in the current item under analysis.

Let's take as example the first stanza of the sonnet XXIII by Garcilaso: \"En tanto que de rosa y de azucena\\ se muestra la color en vuestro gesto,\\ y que vuestro mirar ardiente, honesto,\\con clara luz la tempestad serena;\". This stanza presents rhyme between the ending word of the first line and the last word of the fourth line, that is, between \"azucena\" and \"serena\"."""@en ;
          rdfs:isDefinedBy "http://postdata.linhd.uned.es/ontology/postdata-prosodicElements"@en ;
          rdfs:label "has rhyme"@en .


###  http://postdata.linhd.uned.es/ontology/postdata-poeticAnalysis#hasRhymeWord
:hasRhymeWord rdf:type owl:ObjectProperty ;
              rdfs:subPropertyOf owl:topObjectProperty ;
              owl:inverseOf :isRhymeWord ;
              rdfs:domain :Rhyme ;
              rdfs:range :Word ;
              <http://purl.org/dc/elements/1.1/creator> "mluisadiez" ;
              <http://purl.org/dc/elements/1.1/date> "2018-06-16T20:30:43Z"^^xsd:dateTime ;
              rdfs:comment """This property points to the instance of Word for a further linguistic analysis/division by words.

For example, the line \"From fairest creatures we desire increase,\" from the first sonnet by Shakespeare has \"increase\" as rhyming word."""@en ;
              rdfs:isDefinedBy "http://postdata.linhd.uned.es/ontology/postdata-prosodicElements"@en ;
              rdfs:label "has rhyme word"@en .


###  http://postdata.linhd.uned.es/ontology/postdata-poeticAnalysis#hasStanza
:hasStanza rdf:type owl:ObjectProperty ;
           rdfs:subPropertyOf :hasPart ;
           owl:inverseOf :isStanzaOf ;
           rdfs:domain :Scansion ;
           rdfs:range :Stanza ;
           rdfs:label "has stanza"@en .


###  http://postdata.linhd.uned.es/ontology/postdata-poeticAnalysis#hasStanzaList
:hasStanzaList rdf:type owl:ObjectProperty ;
               rdfs:subPropertyOf :hasList ;
               owl:inverseOf :isStanzaListOf ;
               rdfs:domain :Scansion ;
               rdfs:range :StanzaList ;
               rdfs:comment "This property points to the Stanza List that conforms a Redaction."@en ;
               rdfs:isDefinedBy "http://postdata.linhd.uned.es/ontology/postdata-poeticAnalysis#" ;
               rdfs:label "has stanza list"@en .


###  http://postdata.linhd.uned.es/ontology/postdata-poeticAnalysis#hasStanzaPattern
:hasStanzaPattern rdf:type owl:ObjectProperty ;
                  rdfs:subPropertyOf :hasPattern ;
                  owl:inverseOf :isStanzaPatternOf ;
                  rdfs:domain :Stanza ;
                  rdfs:range :StanzaPattern ;
                  rdfs:comment """This property points to an instance of Stanza about which the item at hand presents analytical information.

The Stanza Pattern \"ABBA\" analyses the first stanza of the poem \"Osé y temí, mas pudo la osadía\" by Fernando de Herrera."""@en ;
                  rdfs:isDefinedBy "http://postdata.linhd.uned.es/ontology/postdata-prosodicElements"@en ;
                  rdfs:label "has stanza pattern"@en .


###  http://postdata.linhd.uned.es/ontology/postdata-poeticAnalysis#hasStartingLine
:hasStartingLine rdf:type owl:ObjectProperty ;
                 owl:inverseOf :isStartingLineOf ;
                 rdfs:domain <http://postdata.linhd.uned.es/ontology/postdata-core#Excerpt> ;
                 rdfs:range :Line ;
                 rdfs:comment "This property points to the lines (instance of Line) or word (instance of Word) which contains the current item under analysis"@en ;
                 rdfs:isDefinedBy "http://postdata.linhd.uned.es/ontology/postdata-poeticAnalysis#"@en ;
                 rdfs:label "has starting line"@en .


###  http://postdata.linhd.uned.es/ontology/postdata-poeticAnalysis#hasWord
:hasWord rdf:type owl:ObjectProperty ;
         rdfs:subPropertyOf :hasPart ;
         owl:inverseOf :isWordOf ;
         rdfs:domain :Line ;
         rdfs:range :Word ;
         rdfs:label "has word"@en .


###  http://postdata.linhd.uned.es/ontology/postdata-poeticAnalysis#hasWordList
:hasWordList rdf:type owl:ObjectProperty ;
             rdfs:subPropertyOf :hasList ;
             owl:inverseOf :isWordListOf ;
             rdfs:domain :Line ;
             rdfs:range :WordList ;
             rdfs:label "has word list"@en .


###  http://postdata.linhd.uned.es/ontology/postdata-poeticAnalysis#isAcrosticPresentAt
:isAcrosticPresentAt rdf:type owl:ObjectProperty ;
                     owl:inverseOf :presentsAcrostic ;
                     rdfs:domain :Acrostic ;
                     rdfs:range <http://postdata.linhd.uned.es/ontology/postdata-core#Excerpt> ;
                     rdfs:label "is acrostic present at"@en .


###  http://postdata.linhd.uned.es/ontology/postdata-poeticAnalysis#isAgentMentionedIn
:isAgentMentionedIn rdf:type owl:ObjectProperty ;
                    rdfs:subPropertyOf :isMentionedIn ;
                    owl:inverseOf :mentionsAgent ;
                    rdfs:domain <http://postdata.linhd.uned.es/ontology/postdata-core#Agent> ;
                    rdfs:range <http://postdata.linhd.uned.es/ontology/postdata-core#Excerpt> ;
                    rdfs:label "is agent mentioned in" .


###  http://postdata.linhd.uned.es/ontology/postdata-poeticAnalysis#isAnalysedBy
:isAnalysedBy rdf:type owl:ObjectProperty ;
              rdfs:range :AnalyticalUnit ;
              rdfs:label "is analysed by" .


###  http://postdata.linhd.uned.es/ontology/postdata-poeticAnalysis#isAnnotationOf
:isAnnotationOf rdf:type owl:ObjectProperty ;
                rdfs:domain :Scansion ;
                rdfs:label "is annotation of"@en .


###  http://postdata.linhd.uned.es/ontology/postdata-poeticAnalysis#isCallOf
:isCallOf rdf:type owl:ObjectProperty ;
          rdfs:domain :Word ;
          rdfs:range :Word ;
          rdfs:comment """This property points to a previous Word (call) that rhymes with the current instance of Word.

For example, \"escriba\" is call of \"arriba\", if we consider the lines \"Érase un elefante boca arriba,/
Érase una nariz sayón y escriba\" from the poem \"A un hombre de gran nariz\" by Quevedo."""@en ;
          rdfs:isDefinedBy "http://postdata.linhd.uned.es/ontology/postdata-prosodicElements" ;
          rdfs:label "is call of"@en .


###  http://postdata.linhd.uned.es/ontology/postdata-poeticAnalysis#isDeviceAnnotationOf
:isDeviceAnnotationOf rdf:type owl:ObjectProperty ;
                      rdfs:subPropertyOf :isAnnotationOf ;
                      rdfs:domain :LiteraryDevice ;
                      rdfs:range :Scansion ;
                      rdfs:label "is device annotation of"@en .


###  http://postdata.linhd.uned.es/ontology/postdata-poeticAnalysis#isEchoOf
:isEchoOf rdf:type owl:ObjectProperty ;
          rdfs:domain :Word ;
          rdfs:range :Word ;
          rdfs:comment """This property points to a following Word (echo) that that rhymes with the current instance of Word.

For example, \"arriba\" is echo of \"escriba\", if we consider the lines \"Érase un elefante boca arriba,/ Érase una nariz sayón y escriba,\" from the poem \"A un hombre de gran nariz\" by Quevedo."""@en ;
          rdfs:isDefinedBy "http://postdata.linhd.uned.es/ontology/postdata-prosodicElements"@en ;
          rdfs:label "is echo of"@en .


###  http://postdata.linhd.uned.es/ontology/postdata-poeticAnalysis#isEmployedIn
:isEmployedIn rdf:type owl:ObjectProperty ;
              rdfs:domain :Symbol ;
              rdfs:range :MetricalEncoding ;
              rdfs:comment """This property points to the instance of MetricalEncoding that employs the item at hand.

For example, if we consider the LinePattern \"-+-+-+-+-+\" of the line \"From fairest creatures we desire increase,\" from the first sonnet by Shakespeare,the Symbol \"+\", for example, isEmployed in the MetricalEncoding to indicate stressed syllable."""@en ;
              rdfs:isDefinedBy "http://postdata.linhd.uned.es/ontology/postdata-prosodicElements"@en ;
              rdfs:label "is employed in"@en .


###  http://postdata.linhd.uned.es/ontology/postdata-poeticAnalysis#isEncodingUsedBy
:isEncodingUsedBy rdf:type owl:ObjectProperty ;
                  owl:inverseOf :usesEncoding ;
                  rdfs:domain :MetricalEncoding ;
                  rdfs:range :ScansionProcess ;
                  rdfs:comment """This property points to an instance of LinePattern, StanzaPattern or WorkPattern which uses the convention defined in the current instance of MetricalEncoding.

For example, if we consider the LinePattern \"-+-+-+-+-+\" of the line \"From fairest creatures we desire increase,\" from the first sonnet by Shakespeare, In the first line, the MetricalEncoding using \"+\" and \"-\" symbols for stressed and unstressed syllables, is used for containing the information of the pattern."""@en ;
                  rdfs:isDefinedBy "http://postdata.linhd.uned.es/ontology/postdata-prosodicElements"@en ;
                  rdfs:label "is encoding used by"@en .


###  http://postdata.linhd.uned.es/ontology/postdata-poeticAnalysis#isEndingLineOf
:isEndingLineOf rdf:type owl:ObjectProperty ;
                rdfs:domain :Line ;
                rdfs:range <http://postdata.linhd.uned.es/ontology/postdata-core#Excerpt> ;
                rdfs:label "is ending line of"@en .


###  http://postdata.linhd.uned.es/ontology/postdata-poeticAnalysis#isFigurePresentAt
:isFigurePresentAt rdf:type owl:ObjectProperty ;
                   owl:inverseOf :presentsFigure ;
                   rdfs:domain :FigureOfSpeech ;
                   rdfs:range <http://postdata.linhd.uned.es/ontology/postdata-core#Excerpt> ;
                   rdfs:label "is figure present at"@en .


###  http://postdata.linhd.uned.es/ontology/postdata-poeticAnalysis#isFirstWordAffectedBy
:isFirstWordAffectedBy rdf:type owl:ObjectProperty ;
                       rdfs:domain :Word ;
                       rdfs:range :Metaplasm ;
                       rdfs:label "is first word affected by" .


###  http://postdata.linhd.uned.es/ontology/postdata-poeticAnalysis#isFootAnalysedBy
:isFootAnalysedBy rdf:type owl:ObjectProperty ;
                  rdfs:subPropertyOf :isAnalysedBy ;
                  rdfs:domain :Foot ;
                  rdfs:range :BasicAnalyticalUnit ;
                  rdfs:label "is foot analysed by"@en .


###  http://postdata.linhd.uned.es/ontology/postdata-poeticAnalysis#isFootListOf
:isFootListOf rdf:type owl:ObjectProperty ;
              rdfs:subPropertyOf :isListOf ;
              rdfs:domain :FootList ;
              rdfs:range :LinePattern ;
              rdfs:label "is foot list of"@en .


###  http://postdata.linhd.uned.es/ontology/postdata-poeticAnalysis#isFootOf
:isFootOf rdf:type owl:ObjectProperty ;
          rdfs:subPropertyOf :isPartOf ;
          rdfs:domain :Foot ;
          rdfs:range :Line ;
          rdfs:label "is foot of"@en .


###  http://postdata.linhd.uned.es/ontology/postdata-poeticAnalysis#isGeneratedBy
:isGeneratedBy rdf:type owl:ObjectProperty ;
               rdfs:domain :Scansion ;
               rdfs:range :ScansionProcess ;
               rdfs:label "is generated by"@en .


###  http://postdata.linhd.uned.es/ontology/postdata-poeticAnalysis#isGrammaticalSyllableAnalysedBy
:isGrammaticalSyllableAnalysedBy rdf:type owl:ObjectProperty ;
                                 rdfs:subPropertyOf :isAnalysedBy ;
                                 rdfs:domain :GrammaticalSyllable ;
                                 rdfs:range :BasicAnalyticalUnit ;
                                 rdfs:label "is grammatical syllable analysed by"@en .


###  http://postdata.linhd.uned.es/ontology/postdata-poeticAnalysis#isGrammaticalSyllableListOf
:isGrammaticalSyllableListOf rdf:type owl:ObjectProperty ;
                             rdfs:subPropertyOf :isListOf ;
                             rdfs:domain :GrammaticalSyllableList ;
                             rdfs:range :Line ;
                             rdfs:label "is grammatical syllable list of"@en .


###  http://postdata.linhd.uned.es/ontology/postdata-poeticAnalysis#isGrammaticalSyllableOf
:isGrammaticalSyllableOf rdf:type owl:ObjectProperty ;
                         rdfs:subPropertyOf :isPartOf ;
                         rdfs:domain :GrammaticalSyllable ;
                         rdfs:range :Line ;
                         rdfs:label "is gramamtical syllable of"@en .


###  http://postdata.linhd.uned.es/ontology/postdata-poeticAnalysis#isInflectedForm
:isInflectedForm rdf:type owl:ObjectProperty ;
                 rdfs:subPropertyOf owl:topObjectProperty ;
                 owl:inverseOf :isLemmaOf ;
                 rdfs:domain :Word ;
                 rdfs:range :Word ;
                 rdfs:comment """This property points to the lemma of a Word.

For example, in the poem \"Rojo Sol, que con hacha luminosa\" by Fernando de Herrera, the word \"luminosa\" is inflected from the lemma \"luminoso\"."""@en ;
                 rdfs:isDefinedBy "http://postdata.linhd.uned.es/ontology/postdata-poeticAnalysis#" ;
                 rdfs:label "inflected form"@en .


###  http://postdata.linhd.uned.es/ontology/postdata-poeticAnalysis#isIntertextualityPresentAt
:isIntertextualityPresentAt rdf:type owl:ObjectProperty ;
                            owl:inverseOf :presentsIntertextuality ;
                            rdfs:domain :Intertextuality ;
                            rdfs:range <http://postdata.linhd.uned.es/ontology/postdata-core#Excerpt> ;
                            rdfs:label "is intertextuality present at"@en .


###  http://postdata.linhd.uned.es/ontology/postdata-poeticAnalysis#isLemmaOf
:isLemmaOf rdf:type owl:ObjectProperty ;
           rdfs:domain :Word ;
           rdfs:range :Word ;
           rdfs:comment """This property points to one of the inflected forms (an instance of Word) of the current headword (the Word at hand).

For example, \"tampoco\" isLemma in the line \"Si no eres par, tampoco le has tenido\" from the sonnet \"Orlando Furioso a Don Quijote de la Mancha\" by Miguel Cervantes."""@en ;
           rdfs:isDefinedBy "http://postdata.linhd.uned.es/ontology/postdata-poeticAnalysis#" ;
           rdfs:label "is lemma of"@en .


###  http://postdata.linhd.uned.es/ontology/postdata-poeticAnalysis#isLineAffectedBy
:isLineAffectedBy rdf:type owl:ObjectProperty ;
                  rdfs:domain :Line ;
                  rdfs:range :Enjambment ;
                  rdfs:label "is line affected by"@en .


###  http://postdata.linhd.uned.es/ontology/postdata-poeticAnalysis#isLineListOf
:isLineListOf rdf:type owl:ObjectProperty ;
              rdfs:subPropertyOf :isListOf ;
              rdfs:domain :LineList ;
              rdfs:range :Stanza ;
              rdfs:comment "This property relates a Line List with the Redaction it breaks down into lines."@en ;
              rdfs:isDefinedBy "http://postdata.linhd.uned.es/ontology/postdata-poeticAnalysis#" ;
              rdfs:label "is line list of"@en .


###  http://postdata.linhd.uned.es/ontology/postdata-poeticAnalysis#isLineOf
:isLineOf rdf:type owl:ObjectProperty ;
          rdfs:subPropertyOf :isPartOf ;
          rdfs:domain :Line ;
          rdfs:range :Stanza ;
          rdfs:label "is line of"@en .


###  http://postdata.linhd.uned.es/ontology/postdata-poeticAnalysis#isLinePatternOf
:isLinePatternOf rdf:type owl:ObjectProperty ;
                 rdfs:subPropertyOf :isPatternOf ;
                 rdfs:domain :LinePattern ;
                 rdfs:range :Line ;
                 rdfs:label "is line pattern of"@en .


###  http://postdata.linhd.uned.es/ontology/postdata-poeticAnalysis#isListAnnotationOf
:isListAnnotationOf rdf:type owl:ObjectProperty ;
                    rdfs:subPropertyOf :isAnnotationOf ;
                    rdfs:domain <http://purl.org/ontology/olo/core#OrderedList> ;
                    rdfs:range :Scansion ;
                    rdfs:label "is list annotation of"@en .


###  http://postdata.linhd.uned.es/ontology/postdata-poeticAnalysis#isListOf
:isListOf rdf:type owl:ObjectProperty ;
          rdfs:domain <http://purl.org/ontology/olo/core#OrderedList> ;
          rdfs:label "is list of"@en .


###  http://postdata.linhd.uned.es/ontology/postdata-poeticAnalysis#isMentionedIn
:isMentionedIn rdf:type owl:ObjectProperty ;
               owl:inverseOf :mentions ;
               rdfs:range <http://postdata.linhd.uned.es/ontology/postdata-core#Excerpt> ;
               rdfs:label "is mentioned in" .


###  http://postdata.linhd.uned.es/ontology/postdata-poeticAnalysis#isMetaplasmPresentedAt
:isMetaplasmPresentedAt rdf:type owl:ObjectProperty ;
                        owl:inverseOf :presentsMetaplasm ;
                        rdfs:domain :Metaplasm ;
                        rdfs:range :Line ;
                        rdfs:label "is metaplasm presented at"@en .


###  http://postdata.linhd.uned.es/ontology/postdata-poeticAnalysis#isMetricalSyllableAnalysedBy
:isMetricalSyllableAnalysedBy rdf:type owl:ObjectProperty ;
                              rdfs:subPropertyOf :isAnalysedBy ;
                              rdfs:domain :MetricalSyllable ;
                              rdfs:range :Mora ;
                              rdfs:label "is metrical syllable analysed by"@en .


###  http://postdata.linhd.uned.es/ontology/postdata-poeticAnalysis#isMetricalSyllableListOf
:isMetricalSyllableListOf rdf:type owl:ObjectProperty ;
                          rdfs:subPropertyOf :isListOf ;
                          rdfs:domain :MetricalSyllableList ;
                          rdfs:range :Line ;
                          rdfs:label "is metrical syllable list of"@en .


###  http://postdata.linhd.uned.es/ontology/postdata-poeticAnalysis#isMetricalSyllableOf
:isMetricalSyllableOf rdf:type owl:ObjectProperty ;
                      rdfs:subPropertyOf :isPartOf ;
                      rdfs:domain :MetricalSyllable ;
                      rdfs:range :Line ;
                      rdfs:label "is metrical syllable of"@en .


###  http://postdata.linhd.uned.es/ontology/postdata-poeticAnalysis#isMoraListOf
:isMoraListOf rdf:type owl:ObjectProperty ;
              rdfs:subPropertyOf :isListOf ;
              rdfs:domain :MoraList ;
              rdfs:range :LinePattern ;
              rdfs:label "is mora list of"@en .


###  http://postdata.linhd.uned.es/ontology/postdata-poeticAnalysis#isMoraOf
:isMoraOf rdf:type owl:ObjectProperty ;
          rdfs:subPropertyOf :isPartOf ;
          rdfs:domain :Mora ;
          rdfs:range :Line ;
          rdfs:label "is mora of"@en .


###  http://postdata.linhd.uned.es/ontology/postdata-poeticAnalysis#isPartOf
:isPartOf rdf:type owl:ObjectProperty ;
          rdfs:domain <http://purl.org/ontology/olo/core#Slot> ;
          rdfs:range <http://purl.org/ontology/olo/core#Slot> ;
          rdfs:label "is part of"@en .


###  http://postdata.linhd.uned.es/ontology/postdata-poeticAnalysis#isPatternAnnotationOf
:isPatternAnnotationOf rdf:type owl:ObjectProperty ;
                       rdfs:subPropertyOf :isAnnotationOf ;
                       rdfs:domain :Pattern ;
                       rdfs:range :Scansion ;
                       rdfs:label "is pattern annotation of"@en .


###  http://postdata.linhd.uned.es/ontology/postdata-poeticAnalysis#isPatternOf
:isPatternOf rdf:type owl:ObjectProperty ;
             rdfs:subPropertyOf owl:topObjectProperty ;
             rdfs:domain :Pattern ;
             <http://purl.org/dc/elements/1.1/creator> "mluisadiez" ;
             <http://purl.org/dc/elements/1.1/date> "2018-06-16T20:30:43Z"^^xsd:dateTime ;
             rdfs:comment """This property points to an item (Pattern) that contains analytical content about the current instance of Redaction or about its stanzas or lines.

For example, the metrical Pattern of the poem \"Amadís de Gaula a don Quijote de La Mancha\" by Cervantes can be analysed, for instance, using the Redaction provided by the Corpus of Golden-Age Spanish Sonnets."""@en ;
             rdfs:label "is pattern of"@en .


###  http://postdata.linhd.uned.es/ontology/postdata-poeticAnalysis#isPlaceMentionedIn
:isPlaceMentionedIn rdf:type owl:ObjectProperty ;
                    rdfs:subPropertyOf :isMentionedIn ;
                    owl:inverseOf :mentionsPlace ;
                    rdfs:domain <http://postdata.linhd.uned.es/ontology/postdata-core#Place> ;
                    rdfs:range <http://postdata.linhd.uned.es/ontology/postdata-core#Excerpt> ;
                    rdfs:label "is place mentioned in" .


###  http://postdata.linhd.uned.es/ontology/postdata-poeticAnalysis#isPunctuationListOf
:isPunctuationListOf rdf:type owl:ObjectProperty ;
                     rdfs:subPropertyOf :isListOf ;
                     rdfs:domain :PunctuationList ;
                     rdfs:range :Line ;
                     rdfs:comment "This property relates a Punctuation List with the Line that presents the punctuations."@en ;
                     rdfs:isDefinedBy "http://postdata.linhd.uned.es/ontology/postdata-poeticAnalysis#" ;
                     rdfs:label "is punctuation list of"@en .


###  http://postdata.linhd.uned.es/ontology/postdata-poeticAnalysis#isPunctuationOf
:isPunctuationOf rdf:type owl:ObjectProperty ;
                 rdfs:subPropertyOf :isPartOf ;
                 rdfs:domain :Punctuation ;
                 rdfs:range :Line ;
                 rdfs:label "is punctuation of"@en .


###  http://postdata.linhd.uned.es/ontology/postdata-poeticAnalysis#isRedactionPatternOf
:isRedactionPatternOf rdf:type owl:ObjectProperty ;
                      rdfs:subPropertyOf :isPatternOf ;
                      rdfs:domain :RedactionPattern ;
                      rdfs:range :Scansion ;
                      rdfs:label "is redaction pattern of"@en .


###  http://postdata.linhd.uned.es/ontology/postdata-poeticAnalysis#isRhymeOf
:isRhymeOf rdf:type owl:ObjectProperty ;
           rdfs:domain :Rhyme ;
           rdfs:range :StructuralUnit ;
           rdfs:comment """This property points to the text (instance of Redaction, Line or Stanza) which contains the current item under analysis.

For example, if we consider the poem \"Elegía a Ramón Sijé\" by Miguel Hernández, the rhyme \"ento\" isPresentIn the seventh and ninth lines of the poem."""@en ;
           rdfs:isDefinedBy "http://postdata.linhd.uned.es/ontology/postdata-prosodicElements"@en ;
           rdfs:label "is rhyme of"@en .


###  http://postdata.linhd.uned.es/ontology/postdata-poeticAnalysis#isRhymeWord
:isRhymeWord rdf:type owl:ObjectProperty ;
             rdfs:domain :Word ;
             rdfs:range :Rhyme ;
             rdfs:comment """This property points to the instance of Rhyme that contains the item at hand as its rhyme word.

For example, if we consider the poem \"Elegía a Ramón Sijé\" by Miguel Hernández, in the first line, the word \"hortelano\" isRhymeWord. \"Hortelano\" rhymes with \"temprano\" in the third line."""@en ;
             rdfs:isDefinedBy "http://postdata.linhd.uned.es/ontology/postdata-prosodicElements"@en ;
             rdfs:label "is rhyme word"@en .


###  http://postdata.linhd.uned.es/ontology/postdata-poeticAnalysis#isSchemePresentAt
:isSchemePresentAt rdf:type owl:ObjectProperty ;
                   rdfs:subPropertyOf :isFigurePresentAt ;
                   owl:inverseOf :presentsScheme ;
                   rdfs:domain :Scheme ;
                   rdfs:label "is scheme present at"@en .


###  http://postdata.linhd.uned.es/ontology/postdata-poeticAnalysis#isStanzaListOf
:isStanzaListOf rdf:type owl:ObjectProperty ;
                rdfs:subPropertyOf :isListOf ;
                rdfs:domain :StanzaList ;
                rdfs:range :Scansion ;
                rdfs:comment "This property relates a given Stanza List with the Redaction it breaks down into stanzas."@en ;
                rdfs:isDefinedBy "http://postdata.linhd.uned.es/ontology/postdata-poeticAnalysis#" ;
                rdfs:label "is stanza list of"@en .


###  http://postdata.linhd.uned.es/ontology/postdata-poeticAnalysis#isStanzaOf
:isStanzaOf rdf:type owl:ObjectProperty ;
            rdfs:subPropertyOf :isPartOf ;
            rdfs:domain :Stanza ;
            rdfs:range :Scansion ;
            rdfs:label "is stanza of"@en .


###  http://postdata.linhd.uned.es/ontology/postdata-poeticAnalysis#isStanzaPatternOf
:isStanzaPatternOf rdf:type owl:ObjectProperty ;
                   rdfs:subPropertyOf :isPatternOf ;
                   rdfs:domain :StanzaPattern ;
                   rdfs:range :Stanza ;
                   rdfs:label "is stanza pattern of"@en .


###  http://postdata.linhd.uned.es/ontology/postdata-poeticAnalysis#isStartingLineOf
:isStartingLineOf rdf:type owl:ObjectProperty ;
                  rdfs:domain :Line ;
                  rdfs:range <http://postdata.linhd.uned.es/ontology/postdata-core#Excerpt> ;
                  rdfs:label "is starting line of"@en .


###  http://postdata.linhd.uned.es/ontology/postdata-poeticAnalysis#isTropePresentAt
:isTropePresentAt rdf:type owl:ObjectProperty ;
                  rdfs:subPropertyOf :isFigurePresentAt ;
                  owl:inverseOf :presentsTrope ;
                  rdfs:domain :Trope ;
                  rdfs:range <http://postdata.linhd.uned.es/ontology/postdata-core#Excerpt> ;
                  rdfs:label "is trope present at"@en .


###  http://postdata.linhd.uned.es/ontology/postdata-poeticAnalysis#isUsedRedactionIn
:isUsedRedactionIn rdf:type owl:ObjectProperty ;
                   owl:inverseOf :usedAsRedaction ;
                   rdfs:domain <http://postdata.linhd.uned.es/ontology/postdata-core#Redaction> ;
                   rdfs:range :Intertextuality ;
                   rdfs:comment "This property points to a cultural product (Intertextuality) which was based on the work under analysis"@en ;
                   rdfs:isDefinedBy "http://postdata.linhd.uned.es/ontology/postdata-poeticAnalysis#"@en ;
                   rdfs:label "is used redaction in"@en .


###  http://postdata.linhd.uned.es/ontology/postdata-poeticAnalysis#isUsedSourceIn
:isUsedSourceIn rdf:type owl:ObjectProperty ;
                owl:inverseOf :usesAsSource ;
                rdfs:domain <http://postdata.linhd.uned.es/ontology/postdata-transmission#Manifestation> ;
                rdfs:range :Intertextuality ;
                rdfs:comment "This property points to the text under analysis (Redaction) from which the current cultural product has derived"@en ;
                rdfs:isDefinedBy "http://postdata.linhd.uned.es/ontology/postdata-poeticAnalysis#"@en ;
                rdfs:label "is used source in"@en .


###  http://postdata.linhd.uned.es/ontology/postdata-poeticAnalysis#isWordAnalysedBy
:isWordAnalysedBy rdf:type owl:ObjectProperty ;
                  rdfs:subPropertyOf :isAnalysedBy ;
                  rdfs:domain :Word ;
                  rdfs:range :AnalyticalUnit ;
                  rdfs:label "is word analysed by"@en .


###  http://postdata.linhd.uned.es/ontology/postdata-poeticAnalysis#isWordListOf
:isWordListOf rdf:type owl:ObjectProperty ;
              rdfs:subPropertyOf :isListOf ;
              rdfs:domain :WordList ;
              rdfs:range :Line ;
              rdfs:label "is word list of"@en .


###  http://postdata.linhd.uned.es/ontology/postdata-poeticAnalysis#isWordOf
:isWordOf rdf:type owl:ObjectProperty ;
          rdfs:subPropertyOf :isPartOf ;
          rdfs:domain :Word ;
          rdfs:range :Line ;
          rdfs:label "is word of"@en .


###  http://postdata.linhd.uned.es/ontology/postdata-poeticAnalysis#lastFoot
:lastFoot rdf:type owl:ObjectProperty ;
          rdfs:subPropertyOf <http://purl.org/ontology/olo/core#has_last_slot> ;
          owl:inverseOf :lastFootOf ;
          rdfs:domain :FootList ;
          rdfs:range :Foot ;
          rdfs:label "last foot"@en .


###  http://postdata.linhd.uned.es/ontology/postdata-poeticAnalysis#lastFootOf
:lastFootOf rdf:type owl:ObjectProperty ;
            rdfs:subPropertyOf <http://purl.org/ontology/olo/core#is_last_slot_of> ;
            rdfs:domain :Foot ;
            rdfs:range :FootList ;
            rdfs:label "last foot of"@en .


###  http://postdata.linhd.uned.es/ontology/postdata-poeticAnalysis#lastGrammaticalSyllable
:lastGrammaticalSyllable rdf:type owl:ObjectProperty ;
                         rdfs:subPropertyOf <http://purl.org/ontology/olo/core#has_last_slot> ;
                         owl:inverseOf :lastGrammaticalSyllableOf ;
                         rdfs:domain :GrammaticalSyllableList ;
                         rdfs:range :GrammaticalSyllable ;
                         rdfs:comment """This property points to the last Syllable which forms part of a given Word.

For example, if we consider the word \"amor\", the last syllable is \"mor\"."""@en ;
                         rdfs:isDefinedBy "http://postdata.linhd.uned.es/ontology/postdata-poeticAnalysis#" ;
                         rdfs:label "last grammatical syllable"@en .


###  http://postdata.linhd.uned.es/ontology/postdata-poeticAnalysis#lastGrammaticalSyllableOf
:lastGrammaticalSyllableOf rdf:type owl:ObjectProperty ;
                           rdfs:subPropertyOf <http://purl.org/ontology/olo/core#is_last_slot_of> ;
                           rdfs:domain :GrammaticalSyllable ;
                           rdfs:range :GrammaticalSyllableList ;
                           rdfs:comment """This property points to Word of which the current Syllable under analysis is its last item.

For example, \"bla\" is the last syllable of the word \"niebla\"."""@en ;
                           rdfs:isDefinedBy "http://postdata.linhd.uned.es/ontology/postdata-poeticAnalysis#" ;
                           rdfs:label "last grammatical syllable of"@en .


###  http://postdata.linhd.uned.es/ontology/postdata-poeticAnalysis#lastLine
:lastLine rdf:type owl:ObjectProperty ;
          rdfs:subPropertyOf <http://purl.org/ontology/olo/core#has_last_slot> ;
          owl:inverseOf :lastLineOf ;
          rdfs:domain :LineList ;
          rdfs:range :Line ;
          rdfs:comment """This property points to the last Line which forms part of a given Line List.

For example, for the poem \"Fábula de Polifemo y Galatea\", last line would be \"yerno lo saludó, lo aclamó río\"."""@en ;
          rdfs:isDefinedBy "http://postdata.linhd.uned.es/ontology/postdata-poeticAnalysis#" ;
          rdfs:label "last line"@en .


###  http://postdata.linhd.uned.es/ontology/postdata-poeticAnalysis#lastLineOf
:lastLineOf rdf:type owl:ObjectProperty ;
            rdfs:subPropertyOf <http://purl.org/ontology/olo/core#is_last_slot_of> ;
            rdfs:domain :Line ;
            rdfs:range :LineList ;
            rdfs:comment """This property points to the Line List of which the current Line under analysis is its last item.

For example, \"Attaccato alla vita\" is the last line of the poem \"Veglia\" by Giuseppe Ungaretti."""@en ;
            rdfs:isDefinedBy "http://postdata.linhd.uned.es/ontology/postdata-poeticAnalysis#" ;
            rdfs:label "last line of"@en .


###  http://postdata.linhd.uned.es/ontology/postdata-poeticAnalysis#lastMetricalSyllable
:lastMetricalSyllable rdf:type owl:ObjectProperty ;
                      rdfs:subPropertyOf <http://purl.org/ontology/olo/core#has_last_slot> ;
                      owl:inverseOf :lastMetricalSyllableOf ;
                      rdfs:domain :MetricalSyllableList ;
                      rdfs:range :MetricalSyllable ;
                      rdfs:label "last metrical syllable"@en .


###  http://postdata.linhd.uned.es/ontology/postdata-poeticAnalysis#lastMetricalSyllableOf
:lastMetricalSyllableOf rdf:type owl:ObjectProperty ;
                        rdfs:subPropertyOf <http://purl.org/ontology/olo/core#is_last_slot_of> ;
                        rdfs:domain :MetricalSyllable ;
                        rdfs:range :MetricalSyllableList ;
                        rdfs:label "last metrical syllable of"@en .


###  http://postdata.linhd.uned.es/ontology/postdata-poeticAnalysis#lastMora
:lastMora rdf:type owl:ObjectProperty ;
          rdfs:subPropertyOf <http://purl.org/ontology/olo/core#has_last_slot> ;
          owl:inverseOf :lastMoraOf ;
          rdfs:domain :MoraList ;
          rdfs:range :Mora ;
          rdfs:label "last mora"@en .


###  http://postdata.linhd.uned.es/ontology/postdata-poeticAnalysis#lastMoraOf
:lastMoraOf rdf:type owl:ObjectProperty ;
            rdfs:subPropertyOf <http://purl.org/ontology/olo/core#is_last_slot_of> ;
            rdfs:domain :Mora ;
            rdfs:range :MoraList ;
            rdfs:label "last mora of"@en .


###  http://postdata.linhd.uned.es/ontology/postdata-poeticAnalysis#lastPunctuation
:lastPunctuation rdf:type owl:ObjectProperty ;
                 rdfs:subPropertyOf <http://purl.org/ontology/olo/core#has_last_slot> ;
                 owl:inverseOf :lastPunctuationOf ;
                 rdfs:domain :PunctuationList ;
                 rdfs:range :Punctuation ;
                 rdfs:comment "This property points to the last Punctuation which forms part of a given Punctuation List."@en ;
                 rdfs:isDefinedBy "http://postdata.linhd.uned.es/ontology/postdata-poeticAnalysis#" ;
                 rdfs:label "last punctuation"@en .


###  http://postdata.linhd.uned.es/ontology/postdata-poeticAnalysis#lastPunctuationOf
:lastPunctuationOf rdf:type owl:ObjectProperty ;
                   rdfs:subPropertyOf <http://purl.org/ontology/olo/core#is_last_slot_of> ;
                   rdfs:domain :Punctuation ;
                   rdfs:range :PunctuationList ;
                   rdfs:comment "This property points to the Punctuation List for which a given Punctuation is its last element."@en ;
                   rdfs:isDefinedBy "http://postdata.linhd.uned.es/ontology/postdata-poeticAnalysis#" ;
                   rdfs:label "last punctuation of"@en .


###  http://postdata.linhd.uned.es/ontology/postdata-poeticAnalysis#lastStanza
:lastStanza rdf:type owl:ObjectProperty ;
            rdfs:subPropertyOf <http://purl.org/ontology/olo/core#has_last_slot> ;
            owl:inverseOf :lastStanzaOf ;
            rdfs:domain :StanzaList ;
            rdfs:range :Stanza ;
            rdfs:comment """This property points to the last Stanza which forms part of the current Stanza List.

For example, The last stanza of el poema \"Diamante\" by Federico García Lorca is \"Se agitan en mi recuerdo /Dos palomas campesinas /Y en el horizonte, lejos, Se hunde el arcaduz del día. /¡Terrible noria del tiempo!\"."""@en ;
            rdfs:isDefinedBy "http://postdata.linhd.uned.es/ontology/postdata-poeticAnalysis#" ;
            rdfs:label "last stanza"@en .


###  http://postdata.linhd.uned.es/ontology/postdata-poeticAnalysis#lastStanzaOf
:lastStanzaOf rdf:type owl:ObjectProperty ;
              rdfs:subPropertyOf <http://purl.org/ontology/olo/core#is_last_slot_of> ;
              rdfs:domain :Stanza ;
              rdfs:range :StanzaList ;
              rdfs:comment """This property points to the Stanza List of which the current Stanza under analysis is its last item.

For example, if we take the poem \"Un soneto me manda hacer Violante\" by Lope de Vega, the fourth stanza (\"Ya estoy en el segundo, y aún sospecho / que voy los trece versos acabando; / contad si son catorce, y está hecho.\") is the last stanza."""@en ;
              rdfs:isDefinedBy "http://postdata.linhd.uned.es/ontology/postdata-poeticAnalysis#" ;
              rdfs:label "last stanza of"@en .


###  http://postdata.linhd.uned.es/ontology/postdata-poeticAnalysis#lastWord
:lastWord rdf:type owl:ObjectProperty ;
          rdfs:subPropertyOf <http://purl.org/ontology/olo/core#has_last_slot> ;
          owl:inverseOf :lastWordOf ;
          rdfs:domain :WordList ;
          rdfs:range :Word ;
          rdfs:comment """This property points to the last Word which form part of a given Line.

For example, \"suono\" is the last token of the line \"Voi ch'ascoltate in rime sparse il suono\" from the first sonnet of the \"Canzoniere\" by Francesco Petrarca."""@en ;
          rdfs:isDefinedBy "http://postdata.linhd.uned.es/ontology/postdata-poeticAnalysis#" ;
          rdfs:label "last word"@en .


###  http://postdata.linhd.uned.es/ontology/postdata-poeticAnalysis#lastWordOf
:lastWordOf rdf:type owl:ObjectProperty ;
            rdfs:subPropertyOf <http://purl.org/ontology/olo/core#is_last_slot_of> ;
            rdfs:domain :Word ;
            rdfs:range :WordList ;
            rdfs:comment """This property points to Line of which the current Word is its last element.

For example, the token \"breeding\" is the last token of the line \"April is the cruellest month, breeding\" from the poem \"The Waste Land\" by T. S. Eliot."""@en ;
            rdfs:isDefinedBy "http://postdata.linhd.uned.es/ontology/postdata-poeticAnalysis#" ;
            rdfs:label "last word of"@en .


###  http://postdata.linhd.uned.es/ontology/postdata-poeticAnalysis#line
:line rdf:type owl:ObjectProperty ;
      rdfs:subPropertyOf <http://purl.org/ontology/olo/core#slot> ;
      owl:inverseOf :lineList ;
      rdfs:domain :LineList ;
      rdfs:range :Line ;
      rdfs:comment """Line of a Line List.

For example, the poem \"Non chiederci la parola che squadri da ogni lato\" by Eugenio Montale has the line \"Ah l’uomo che se ne va sicuro,\"  as the first line of the second stanza."""@en ;
      rdfs:isDefinedBy "http://postdata.linhd.uned.es/ontology/postdata-poeticAnalysis#" ;
      rdfs:label "line"@en .


###  http://postdata.linhd.uned.es/ontology/postdata-poeticAnalysis#lineList
:lineList rdf:type owl:ObjectProperty ;
          rdfs:subPropertyOf <http://purl.org/ontology/olo/core#ordered_list> ;
          rdfs:domain :Line ;
          rdfs:range :LineList ;
          rdfs:comment """This property refers to the Line List a given Line belongs to.

For example, in the poem \"Mientras por competir por tu cabello\", the line \"en tierra, en humo, en polvo, en sombra, en nada\" belongs to the fourth stanza (\"no sólo en plata o vïola troncada / se vuelva, mas tú y ello, juntamente, / en tierra, en humo, en polvo, en sombra, en nada.\")"""@en ;
          rdfs:isDefinedBy "http://postdata.linhd.uned.es/ontology/postdata-poeticAnalysis#" ;
          rdfs:label "line list"@en .


###  http://postdata.linhd.uned.es/ontology/postdata-poeticAnalysis#mentions
:mentions rdf:type owl:ObjectProperty ;
          rdfs:domain <http://postdata.linhd.uned.es/ontology/postdata-core#Excerpt> ;
          rdfs:comment """Agent or Place that is mentioned on the line

Example: The line from the poem \"Piedra negra sobre una piedra blanca\" by César Vallejo \"Me moriré en París con aguacero,\" has mention to the Place \"Paris\""""@en ;
          rdfs:isDefinedBy "http://postdata.linhd.uned.es/ontology/postdata-poeticAnalysis#"@en ;
          rdfs:label "mentions"@en .


###  http://postdata.linhd.uned.es/ontology/postdata-poeticAnalysis#mentionsAgent
:mentionsAgent rdf:type owl:ObjectProperty ;
               rdfs:subPropertyOf :mentions ;
               rdfs:domain <http://postdata.linhd.uned.es/ontology/postdata-core#Excerpt> ;
               rdfs:range <http://postdata.linhd.uned.es/ontology/postdata-core#Agent> ;
               rdfs:comment """This property points to the Place that is mentioned in a given Line.

Example: The following line from the Purgatorio of Divina Commedia by Dante Alighieri contains mention to the Agent \"Dante\": \"Dante, perché Virgilio se ne vada\""""@en ;
               rdfs:isDefinedBy "http://postdata.linhd.uned.es/ontology/postdata-poeticAnalysis#" ;
               rdfs:label "mentions agent"@en .


###  http://postdata.linhd.uned.es/ontology/postdata-poeticAnalysis#mentionsPlace
:mentionsPlace rdf:type owl:ObjectProperty ;
               rdfs:subPropertyOf :mentions ;
               rdfs:domain <http://postdata.linhd.uned.es/ontology/postdata-core#Excerpt> ;
               rdfs:range <http://postdata.linhd.uned.es/ontology/postdata-core#Place> ;
               rdfs:comment """This property points to the Place that is mentioned in a given Line.

Example: For example, the line \"Granada, calle de Elvira,\" from the poem \"Granada\" by Federico García Lorca, contains mention to the place \"Granada\"."""@en ;
               rdfs:isDefinedBy "http://postdata.linhd.uned.es/ontology/postdata-poeticAnalysis#" ;
               rdfs:label "mentions place"@en .


###  http://postdata.linhd.uned.es/ontology/postdata-poeticAnalysis#metricalCategory
:metricalCategory rdf:type owl:ObjectProperty ;
                  rdfs:domain :RedactionPattern ;
                  rdfs:range <http://www.w3.org/2004/02/skos/core#Concept> ,
                             [ rdf:type owl:Restriction ;
                               owl:onProperty <http://www.w3.org/2004/02/skos/core#inScheme> ;
                               owl:hasValue <http://postdata.linhd.uned.es/kos/metrical-category>
                             ] ;
                  rdfs:comment """Major category to identify the metrical type (e.g. fixed forms vs strophic).

For example, if we consider the sonnet by Garcilaso \"Soneto XVII\", metricalCatehory is Strophic."""@en ;
                  rdfs:isDefinedBy "http://postdata.linhd.uned.es/ontology/postdata-prosodicElements"@en ;
                  rdfs:label "metrical category"@en .


###  http://postdata.linhd.uned.es/ontology/postdata-poeticAnalysis#metricalComplexity
:metricalComplexity rdf:type owl:ObjectProperty ;
                    rdfs:domain :RedactionPattern ;
                    rdfs:range <http://www.w3.org/2004/02/skos/core#Concept> ,
                               [ rdf:type owl:Restriction ;
                                 owl:onProperty <http://www.w3.org/2004/02/skos/core#inScheme> ;
                                 owl:hasValue <http://postdata.linhd.uned.es/kos/metrical-complexity>
                               ] ;
                    rdfs:comment """Categorisation depending on the number of syllables: usually, less or more than eight.

For example, if we consider the sonnet by Garcilaso \"Soneto XVII\", metricalComplexity is \"verso de arte mayor\" because all lines are hendecasyllables."""@en ;
                    rdfs:isDefinedBy "http://postdata.linhd.uned.es/ontology/postdata-prosodicElements"@en ;
                    rdfs:label "metrical complexity"@en .


###  http://postdata.linhd.uned.es/ontology/postdata-poeticAnalysis#metricalContext
:metricalContext rdf:type owl:ObjectProperty ;
                 rdfs:domain :RedactionPattern ;
                 rdfs:range <http://www.w3.org/2004/02/skos/core#Concept> ,
                            [ rdf:type owl:Restriction ;
                              owl:onProperty <http://www.w3.org/2004/02/skos/core#inScheme> ;
                              owl:hasValue <http://postdata.linhd.uned.es/kos/metrical-context>
                            ] ;
                 rdfs:comment """Categorisation depending on whether all lines have the same number of syllables.

For example, if we consider the sonnet by Garcilaso \"Soneto XVII\", metricalContext is \"Isosyllabic\" because all lines are hendecasyllables, hence, exhibit the same metrical length."""@en ;
                 rdfs:isDefinedBy "http://postdata.linhd.uned.es/ontology/postdata-prosodicElements"@en ;
                 rdfs:label "metrical context"@en .


###  http://postdata.linhd.uned.es/ontology/postdata-poeticAnalysis#metricalSyllable
:metricalSyllable rdf:type owl:ObjectProperty ;
                  rdfs:subPropertyOf <http://purl.org/ontology/olo/core#slot> ;
                  owl:inverseOf :metricalSyllableList ;
                  rdfs:domain :MetricalSyllableList ;
                  rdfs:range :MetricalSyllable ;
                  rdfs:label "metrical syllable"@en .


###  http://postdata.linhd.uned.es/ontology/postdata-poeticAnalysis#metricalSyllableList
:metricalSyllableList rdf:type owl:ObjectProperty ;
                      rdfs:subPropertyOf <http://purl.org/ontology/olo/core#ordered_list> ;
                      rdfs:domain :MetricalSyllable ;
                      rdfs:range :MetricalSyllableList ;
                      rdfs:label "metrical syllable list"@en .


###  http://postdata.linhd.uned.es/ontology/postdata-poeticAnalysis#metricalType
:metricalType rdf:type owl:ObjectProperty ;
              rdfs:domain :StanzaPattern ;
              rdfs:range <http://www.w3.org/2004/02/skos/core#Concept> ,
                         [ rdf:type owl:Restriction ;
                           owl:onProperty <http://www.w3.org/2004/02/skos/core#inScheme> ;
                           owl:hasValue <http://postdata.linhd.uned.es/kos/metrical-type>
                         ] ;
              rdfs:comment """Categorisation of the stanza/line  grouping or work according to metrics. E.g. “sapphic stanza”.

For example, \"By taking as example the poem \"La torre de Monterrey a la luz de la luna\" by Miguel de Unamuno:  \"Torre de Monterrey, \\ cuadrada torre, que miras desfilar hombres y días,\\ tú me hablas del pasado y del futuro \\ Renacimiento.\". In this case, metricalType is \"sapphic stanza\"."""@en ;
              rdfs:isDefinedBy "http://postdata.linhd.uned.es/ontology/postdata-prosodicElements"@en ;
              rdfs:label "metrical type"@en .


###  http://postdata.linhd.uned.es/ontology/postdata-poeticAnalysis#mora
:mora rdf:type owl:ObjectProperty ;
      rdfs:subPropertyOf <http://purl.org/ontology/olo/core#slot> ;
      owl:inverseOf :moraList ;
      rdfs:domain :MoraList ;
      rdfs:range :Mora ;
      rdfs:label "mora"@en .


###  http://postdata.linhd.uned.es/ontology/postdata-poeticAnalysis#moraList
:moraList rdf:type owl:ObjectProperty ;
          rdfs:subPropertyOf <http://purl.org/ontology/olo/core#ordered_list> ;
          owl:inverseOf <http://purl.org/ontology/olo/core#slot> ;
          rdfs:domain :Mora ;
          rdfs:range :MoraList ;
          rdfs:label "mora list"@en .


###  http://postdata.linhd.uned.es/ontology/postdata-poeticAnalysis#nextFoot
:nextFoot rdf:type owl:ObjectProperty ;
          rdfs:subPropertyOf <http://purl.org/ontology/olo/core#next> ;
          owl:inverseOf :previousFoot ;
          rdfs:domain :Foot ;
          rdfs:range :Foot ;
          <http://purl.org/dc/elements/1.1/creator> "mluisadiez" ;
          <http://purl.org/dc/elements/1.1/date> "2018-06-16T20:30:43Z"^^xsd:dateTime ;
          rdfs:comment """This property points to the next instance of Foot.

For example, if we consider the first foot of the first line of the sonnet I by Shakespeare \"From fairest creatures we desire increase\", namely |from fai|, nextFoot is |rest crea|"""@en ;
          rdfs:isDefinedBy "http://postdata.linhd.uned.es/ontology/postdata-prosodicElements"@en ;
          rdfs:label "next foot"@en .


###  http://postdata.linhd.uned.es/ontology/postdata-poeticAnalysis#nextFootAfterCaesura
:nextFootAfterCaesura rdf:type owl:ObjectProperty ;
                      rdfs:subPropertyOf owl:topObjectProperty ;
                      owl:inverseOf :previousFootBeforeCaesura ;
                      rdfs:domain :Foot ;
                      rdfs:range :Foot ;
                      <http://purl.org/dc/elements/1.1/creator> "mluisadiez" ;
                      <http://purl.org/dc/elements/1.1/date> "2018-06-16T20:30:43Z"^^xsd:dateTime ;
                      rdfs:comment """This property points to the next instance of Foot when this is positioned after a caesura.

For example, consider the first line of the sonnet by the Dutch Renaissance poet P.C. Hooft \"Leitsterren van mijn hoop, planeten van mijn jeucht\". Given that this iambic alexandrine is divided into six feet (noted here as I) and exhibits a caesura (noted here as ||) after the first three feet as follows: |Leitster| ren van| mijn hoop||, plane| ten van| mijn jeucht|. In this case, previousFootBeforeCaesura is \"plane\"."""@en ;
                      rdfs:isDefinedBy "http://postdata.linhd.uned.es/ontology/postdata-prosodicElements"@en ;
                      rdfs:label "next foot after caesura"@en .


###  http://postdata.linhd.uned.es/ontology/postdata-poeticAnalysis#nextGrammaticalSyllable
:nextGrammaticalSyllable rdf:type owl:ObjectProperty ;
                         rdfs:subPropertyOf <http://purl.org/ontology/olo/core#next> ;
                         owl:inverseOf :previousGrammaticalSyllable ;
                         rdfs:domain :GrammaticalSyllable ;
                         rdfs:range :GrammaticalSyllable ;
                         rdfs:comment """This property points to the Syllable that follows the Syllable under analysis in a Word.

For example, if we consider the syllable \"can\" in the word \"cansado\", the next syllable is \"sa\"."""@en ;
                         rdfs:isDefinedBy "http://postdata.linhd.uned.es/ontology/postdata-poeticAnalysis#" ;
                         rdfs:label "next grammatical syllable"@en .


###  http://postdata.linhd.uned.es/ontology/postdata-poeticAnalysis#nextLine
:nextLine rdf:type owl:ObjectProperty ;
          rdfs:subPropertyOf <http://purl.org/ontology/olo/core#next> ;
          owl:inverseOf :previousLine ;
          rdfs:domain :Line ;
          rdfs:range :Line ;
          rdfs:comment """This property points to following Line of the Line under analysis in a Line List.

For example, if we consider the line \"April is the cruellest most\" from the poem \"The Waste Land\" by T.S. Eliot, \"Lilacs out of the dead land, mixing\" is the next line."""@en ;
          rdfs:isDefinedBy "http://postdata.linhd.uned.es/ontology/postdata-poeticAnalysis#" ;
          rdfs:label "next line"@en .


###  http://postdata.linhd.uned.es/ontology/postdata-poeticAnalysis#nextMetricalSyllable
:nextMetricalSyllable rdf:type owl:ObjectProperty ;
                      rdfs:subPropertyOf <http://purl.org/ontology/olo/core#next> ;
                      owl:inverseOf :previousMetricalSyllable ;
                      rdfs:domain :MetricalSyllable ;
                      rdfs:range :MetricalSyllable ;
                      rdfs:label "next metrical syllable"@en .


###  http://postdata.linhd.uned.es/ontology/postdata-poeticAnalysis#nextMora
:nextMora rdf:type owl:ObjectProperty ;
          rdfs:subPropertyOf <http://purl.org/ontology/olo/core#next> ;
          owl:inverseOf :previousMora ;
          rdfs:domain :Mora ;
          rdfs:range :Mora ;
          rdfs:comment """This property points to the next unit that forms the foot (an instance of FootDivision).

For example, if we consider the unit \"rest\" of the second foot of the first line of the sonnet I by Shakespeare (\"From fairest creatures we desire increase\") , namely |rest crea|, nextUnit in the foot is \"crea\"."""@en ;
          rdfs:isDefinedBy "http://postdata.linhd.uned.es/ontology/postdata-prosodicElements"@en ;
          rdfs:label "next mora"@en .


###  http://postdata.linhd.uned.es/ontology/postdata-poeticAnalysis#nextPunctuation
:nextPunctuation rdf:type owl:ObjectProperty ;
                 rdfs:subPropertyOf <http://purl.org/ontology/olo/core#next> ;
                 owl:inverseOf :previousPunctuation ;
                 rdfs:domain :Punctuation ;
                 rdfs:range :Punctuation ;
                 rdfs:comment "This property points to the following Punctuation of a given Punctuation in a Punctuation List."@en ;
                 rdfs:isDefinedBy "http://postdata.linhd.uned.es/ontology/postdata-poeticAnalysis#" ;
                 rdfs:label "next punctuation"@en .


###  http://postdata.linhd.uned.es/ontology/postdata-poeticAnalysis#nextStanza
:nextStanza rdf:type owl:ObjectProperty ;
            rdfs:subPropertyOf <http://purl.org/ontology/olo/core#next> ;
            owl:inverseOf :previousStanza ;
            rdfs:domain :Stanza ;
            rdfs:range :Stanza ;
            rdfs:comment """This property points to the Stanza that follows the Stanza under analysis in a Stanza List.

For example, in the poem \"SONETO XIII\" by Garcilaso de la Vega, if we are analysing the first stanza, next stanza would be \"De áspera corteza se cubrían / los tiernos miembros que aún bullendo estaban; / los blancos pies en tierra se hincaban, /Y en torcidas raíces se volvían.\""""@en ;
            rdfs:isDefinedBy "http://postdata.linhd.uned.es/ontology/postdata-poeticAnalysis#" ;
            rdfs:label "next stanza"@en .


###  http://postdata.linhd.uned.es/ontology/postdata-poeticAnalysis#nextWord
:nextWord rdf:type owl:ObjectProperty ;
          rdfs:subPropertyOf <http://purl.org/ontology/olo/core#next> ;
          owl:inverseOf :previousWord ;
          rdfs:domain :Word ;
          rdfs:range :Word ;
          rdfs:comment """This property points to a Word that follows the current Word under analysis in a Line.

For example, if the poem under analysis is \"Romance sonámbulo\" and we have already analyse the first token (\"verde\"), next token would be \"que\"."""@en ;
          rdfs:isDefinedBy "http://postdata.linhd.uned.es/ontology/postdata-poeticAnalysis#" ;
          rdfs:label "next word"@en .


###  http://postdata.linhd.uned.es/ontology/postdata-poeticAnalysis#partOfSpeech
:partOfSpeech rdf:type owl:ObjectProperty ;
              rdfs:subPropertyOf owl:topObjectProperty ;
              rdfs:domain :Word ;
              rdfs:range <http://www.w3.org/2004/02/skos/core#Concept> ,
                         [ rdf:type owl:Restriction ;
                           owl:onProperty <http://www.w3.org/2004/02/skos/core#inScheme> ;
                           owl:hasValue <http://postdata.linhd.uned.es/kos/part-of-speech>
                         ] ;
              rdfs:comment """The category or type of a Word. Words in the same category (or, more generally, of lexical items) have similar grammatical properties. Commonly listed  parts of speech are noun, verb, adjective, adverb, pronoun, preposition, conjunction, interjection, and sometimes numeral, article, or determiner. We exclude punctuations from the possible values as we employ the Punctuation class for this purpose

For example, if we take the poem \"Autorretrato\" by Antonio Machado, the word \"infancia\" has noun as its Part of Speech."""@en ;
              rdfs:isDefinedBy "http://postdata.linhd.uned.es/ontology/postdata-poeticAnalysis#/" ;
              rdfs:label "part of speech"@en .


###  http://postdata.linhd.uned.es/ontology/postdata-poeticAnalysis#presentsAcrostic
:presentsAcrostic rdf:type owl:ObjectProperty ;
                  rdfs:domain <http://postdata.linhd.uned.es/ontology/postdata-core#Excerpt> ;
                  rdfs:range :Acrostic ;
                  rdfs:label "presents acrostic"@en .


###  http://postdata.linhd.uned.es/ontology/postdata-poeticAnalysis#presentsFigure
:presentsFigure rdf:type owl:ObjectProperty ;
                rdfs:domain <http://postdata.linhd.uned.es/ontology/postdata-core#Excerpt> ;
                rdfs:range :FigureOfSpeech ;
                rdfs:label "presents figure"@en .


###  http://postdata.linhd.uned.es/ontology/postdata-poeticAnalysis#presentsIntertextuality
:presentsIntertextuality rdf:type owl:ObjectProperty ;
                         rdfs:domain <http://postdata.linhd.uned.es/ontology/postdata-core#Excerpt> ;
                         rdfs:range :Intertextuality ;
                         rdfs:label "presents intertextuality"@en .


###  http://postdata.linhd.uned.es/ontology/postdata-poeticAnalysis#presentsMetaplasm
:presentsMetaplasm rdf:type owl:ObjectProperty ;
                   rdfs:domain :Line ;
                   rdfs:range :Metaplasm ;
                   rdfs:comment """A metaplasm is presented in Line.

For example, the line from the sonnet I from the Canzoniere by Petrarca, namely \"Voi ch'ascoltate in rime sparse il suono\", presentsMetaplasm, because synaloepha occurs between \"-te\" (\"ascoltate\") and \"in\" and \"-se\" (\"sparse\") and \"il\"."""@en ;
                   rdfs:label "presents metaplasm"@en .


###  http://postdata.linhd.uned.es/ontology/postdata-poeticAnalysis#presentsScheme
:presentsScheme rdf:type owl:ObjectProperty ;
                rdfs:subPropertyOf :presentsFigure ;
                rdfs:domain <http://postdata.linhd.uned.es/ontology/postdata-core#Excerpt> ;
                rdfs:range :Scheme ;
                rdfs:label "presents scheme"@en .


###  http://postdata.linhd.uned.es/ontology/postdata-poeticAnalysis#presentsTrope
:presentsTrope rdf:type owl:ObjectProperty ;
               rdfs:subPropertyOf :presentsFigure ;
               rdfs:domain <http://postdata.linhd.uned.es/ontology/postdata-core#Excerpt> ;
               rdfs:range :Trope ;
               rdfs:label "presents trope"@en .


###  http://postdata.linhd.uned.es/ontology/postdata-poeticAnalysis#previousFoot
:previousFoot rdf:type owl:ObjectProperty ;
              rdfs:subPropertyOf <http://purl.org/ontology/olo/core#previous> ;
              rdfs:domain :Foot ;
              rdfs:range :Foot ;
              rdfs:comment """This property points to the previous instance of Foot.

For example, if we consider the second foot of the first line of the sonnet I by Shakespeare \"From fairest creatures we desire increase\", namely |rest crea|, previousFoot is |from fai|"""@en ;
              rdfs:isDefinedBy "http://postdata.linhd.uned.es/ontology/postdata-prosodicElements"@en ;
              rdfs:label "previous foot"@en .


###  http://postdata.linhd.uned.es/ontology/postdata-poeticAnalysis#previousFootBeforeCaesura
:previousFootBeforeCaesura rdf:type owl:ObjectProperty ;
                           rdfs:domain :Foot ;
                           rdfs:range :Foot ;
                           rdfs:comment """This property points to the previous instance of Foot when this is positioned before a caesura.

For example, consider  the first line of the sonnet by the Dutch Renaissance poet P.C. Hooft \"Leitsterren van mijn hoop, planeten van mijn jeucht\". Given that this iambic alexandrine is divided into six feet (noted here as I) and exhibits a caesura (noted here as ||) after the first three feet as follows: |Leitster| ren van| mijn hoop||, plane| ten van| mijn jeucht|. In this case, previousFootBeforeCaesura is \"mijn hoop\"."""@en ;
                           rdfs:isDefinedBy "http://postdata.linhd.uned.es/ontology/postdata-prosodicElements"@en ;
                           rdfs:label "previous foot before caesura"@en .


###  http://postdata.linhd.uned.es/ontology/postdata-poeticAnalysis#previousGrammaticalSyllable
:previousGrammaticalSyllable rdf:type owl:ObjectProperty ;
                             rdfs:subPropertyOf <http://purl.org/ontology/olo/core#previous> ;
                             rdfs:domain :GrammaticalSyllable ;
                             rdfs:range :GrammaticalSyllable ;
                             rdfs:comment """This property relates a given Syllable to its preceeding Syllable in a Word.

For example, if we consider the syllable \"lor\" in the word \"color\", \"previousSyllable\" is \"co\"."""@en ;
                             rdfs:isDefinedBy "http://postdata.linhd.uned.es/ontology/postdata-poeticAnalysis#" ;
                             rdfs:label "previous grammatical syllable"@en .


###  http://postdata.linhd.uned.es/ontology/postdata-poeticAnalysis#previousLine
:previousLine rdf:type owl:ObjectProperty ;
              rdfs:subPropertyOf <http://purl.org/ontology/olo/core#previous> ;
              rdfs:domain :Line ;
              rdfs:range :Line ;
              rdfs:comment """This property points to the previous item of a list that contains an instance of Line.

For example, \"Aunque es verdad que he escrito algunos miles\" is the previous line of the line \"de versos, si no buenos, tales cuales\" of the poem \"Aunque es verdad\" by Tomás de Iriarte."""@en ;
              rdfs:isDefinedBy "http://postdata.linhd.uned.es/ontology/postdata-poeticAnalysis#" ;
              rdfs:label "previous line"@en .


###  http://postdata.linhd.uned.es/ontology/postdata-poeticAnalysis#previousMetricalSyllable
:previousMetricalSyllable rdf:type owl:ObjectProperty ;
                          rdfs:subPropertyOf <http://purl.org/ontology/olo/core#previous> ;
                          rdfs:domain :MetricalSyllable ;
                          rdfs:range :MetricalSyllable ;
                          rdfs:label "previous metrical syllable"@en .


###  http://postdata.linhd.uned.es/ontology/postdata-poeticAnalysis#previousMora
:previousMora rdf:type owl:ObjectProperty ;
              rdfs:subPropertyOf <http://purl.org/ontology/olo/core#previous> ;
              rdfs:domain :Mora ;
              rdfs:range :Mora ;
              rdfs:comment """This property points to the previous unit that forms the foot (an instance of FootDivision).

For example, if we consider the unit \"crea\" of the second foot of the first line of the sonnet I by Shakespeare (\"From fairest creatures we desire increase\") , namely |rest crea|, previousUnit in the foot is \"rest\"."""@en ;
              rdfs:isDefinedBy "http://postdata.linhd.uned.es/ontology/postdata-prosodicElements"@en ;
              rdfs:label "previous mora"@en .


###  http://postdata.linhd.uned.es/ontology/postdata-poeticAnalysis#previousPunctuation
:previousPunctuation rdf:type owl:ObjectProperty ;
                     rdfs:subPropertyOf <http://purl.org/ontology/olo/core#previous> ;
                     rdfs:domain :Punctuation ;
                     rdfs:range :Punctuation ;
                     rdfs:comment "This property points to the preceeding Punctuation of a Punctuation List."@en ;
                     rdfs:isDefinedBy "http://postdata.linhd.uned.es/ontology/postdata-poeticAnalysis#" ;
                     rdfs:label "previous punctuation"@en .


###  http://postdata.linhd.uned.es/ontology/postdata-poeticAnalysis#previousStanza
:previousStanza rdf:type owl:ObjectProperty ;
                rdfs:subPropertyOf <http://purl.org/ontology/olo/core#previous> ;
                rdfs:domain :Stanza ;
                rdfs:range :Stanza ;
                rdfs:comment """This property points to previous Stanza of the Stanza under analysis in a Stanza List.

For example, in the poem \"Why I Am Not A Painter\" by Frank O'Hara, previous stanza to the second one is the first (\"I am not a painter. I am a poet / Why? I think I would rather be / a painter, but I am not. Well,\")"""@en ;
                rdfs:isDefinedBy "http://postdata.linhd.uned.es/ontology/postdata-poeticAnalysis#" ;
                rdfs:label "previous stanza"@en .


###  http://postdata.linhd.uned.es/ontology/postdata-poeticAnalysis#previousWord
:previousWord rdf:type owl:ObjectProperty ;
              rdfs:subPropertyOf <http://purl.org/ontology/olo/core#previous> ;
              rdfs:domain :Word ;
              rdfs:range :Word ;
              rdfs:comment """This property relates a given Word to its preceeding Word in a Line.

For example, if we consider the token \"month\", the line \"April is the cruellest month, breeding\" from the poem \"The Waste Land\" by T. S. Eliot, the previous token is \"cruellest\".""" ;
              rdfs:isDefinedBy "http://postdata.linhd.uned.es/ontology/postdata-poeticAnalysis#" ;
              rdfs:label "previous word"@en .


###  http://postdata.linhd.uned.es/ontology/postdata-poeticAnalysis#punctuation
:punctuation rdf:type owl:ObjectProperty ;
             rdfs:subPropertyOf <http://purl.org/ontology/olo/core#slot> ;
             owl:inverseOf :punctuationList ;
             rdfs:domain :PunctuationList ;
             rdfs:range :Punctuation ;
             rdfs:comment "This property points to a Punctuation that is contained in a given Punctuation List."@en ;
             rdfs:isDefinedBy "http://postdata.linhd.uned.es/ontology/postdata-poeticAnalysis#" ;
             rdfs:label "punctuation"@en .


###  http://postdata.linhd.uned.es/ontology/postdata-poeticAnalysis#punctuationList
:punctuationList rdf:type owl:ObjectProperty ;
                 rdfs:subPropertyOf <http://purl.org/ontology/olo/core#ordered_list> ;
                 rdfs:domain :Punctuation ;
                 rdfs:range :PunctuationList ;
                 rdfs:comment "This property refers to the Punctuation List that a Punctuation belongs to."@en ;
                 rdfs:isDefinedBy "http://postdata.linhd.uned.es/ontology/postdata-poeticAnalysis#" ;
                 rdfs:label "punctuation list"@en .


###  http://postdata.linhd.uned.es/ontology/postdata-poeticAnalysis#rhetoricalOperation
:rhetoricalOperation rdf:type owl:ObjectProperty ;
                     rdfs:domain :FigureOfSpeech ;
                     rdfs:range <http://www.w3.org/2004/02/skos/core#Concept> ,
                                [ rdf:type owl:Restriction ;
                                  owl:onProperty <http://www.w3.org/2004/02/skos/core#inScheme> ;
                                  owl:hasValue <http://postdata.linhd.uned.es/kos/rhetorical-operation>
                                ] ;
                     rdfs:comment "Classification categories of speech figures in relation to rhetorical operations: addition, omission, transposition and permutation"@en ;
                     rdfs:isDefinedBy "http://postdata.linhd.uned.es/ontology/postdata-poeticAnalysis#"@en ;
                     rdfs:label "rethorical operation"@en .


###  http://postdata.linhd.uned.es/ontology/postdata-poeticAnalysis#rhymeDispositionType
:rhymeDispositionType rdf:type owl:ObjectProperty ;
                      rdfs:domain :StanzaPattern ;
                      rdfs:range <http://www.w3.org/2004/02/skos/core#Concept> ,
                                 [ rdf:type owl:Restriction ;
                                   owl:onProperty <http://www.w3.org/2004/02/skos/core#inScheme> ;
                                   owl:hasValue <http://postdata.linhd.uned.es/kos/rhymeDisposition-type>
                                 ] ;
                      rdfs:comment """Categorisation of the stanza according to the diposition of the rhymes (eg. “cross”, “pair”).

For example, if we consider the first stanza of the sonnet XXIII by Garcilaso: \"En tanto que de rosa y de azucena\\ se muestra la color en vuestro gesto,\\ y que vuestro mirar ardiente, honesto,\\con clara luz la tempestad serena;\" rhymeDisposition is \"enclosed\"."""@en ;
                      rdfs:isDefinedBy "http://postdata.linhd.uned.es/ontology/postdata-prosodicElements"@en ;
                      rdfs:label "rhyme disposition type"@en .


###  http://postdata.linhd.uned.es/ontology/postdata-poeticAnalysis#rhymeMatchingType
:rhymeMatchingType rdf:type owl:ObjectProperty ;
                   rdfs:domain :StructuralUnit ;
                   rdfs:range <http://www.w3.org/2004/02/skos/core#Concept> ,
                              [ rdf:type owl:Restriction ;
                                owl:onProperty <http://www.w3.org/2004/02/skos/core#inScheme> ;
                                owl:hasValue <http://postdata.linhd.uned.es/kos/rhymeMatching-type>
                              ] ;
                   rdfs:comment """Categorisation of the stanza or  work according to the degree in which the different rhyming sounds match (e.g. assonant, consonant...).

For example, if we consider the first stanza of the sonnet XXIII by Garcilaso: \"En tanto que de rosa y de azucena\\ se muestra la color en vuestro gesto,\\ y que vuestro mirar ardiente, honesto,\\con clara luz la tempestad serena;\" rhymeMatching is \"perfect rhyme\"."""@en ;
                   rdfs:isDefinedBy "http://postdata.linhd.uned.es/ontology/postdata-prosodicElements"@en ;
                   rdfs:label "presents rhyme matching"@en .


###  http://postdata.linhd.uned.es/ontology/postdata-poeticAnalysis#rhymesWith
:rhymesWith rdf:type owl:ObjectProperty ,
                     owl:ReflexiveProperty ;
            rdfs:domain :StructuralUnit ;
            rdfs:range :StructuralUnit ;
            rdfs:comment """This property points to an instance of Line that rhymes with the current Line under analysis.

For example, if we consider the line in the sonnet III from Petrarch's \"Canzoniere\", \"Era il giorno ch’al sol si scoloraro\", rhymesWith is the line \"ché i be' vostr'occhi, Donna, mi legaro\"."""@en ;
            rdfs:isDefinedBy "http://postdata.linhd.uned.es/ontology/postdata-prosodicElements"@en ;
            rdfs:label "rhymes with"@en .


###  http://postdata.linhd.uned.es/ontology/postdata-poeticAnalysis#stanza
:stanza rdf:type owl:ObjectProperty ;
        rdfs:subPropertyOf <http://purl.org/ontology/olo/core#slot> ;
        owl:inverseOf :stanzaList ;
        rdfs:domain :StanzaList ;
        rdfs:range :Stanza ;
        rdfs:comment """Stanza associated with the Stanza List that breaks down a Redaction.

For instance, the redaction of Divina Commedia edited by Raffaele Andreoli published by Barbèra Editore, Florence, in 1879, has the stanza \"Veramente, però ch'a questo segno/ Molto si mira e poco si discerne,/Dirò perchè tal modo fu più degno.\""""@en ;
        rdfs:isDefinedBy "http://postdata.linhd.uned.es/ontology/postdata-poeticAnalysis#" ;
        rdfs:label "stanza"@en .


###  http://postdata.linhd.uned.es/ontology/postdata-poeticAnalysis#stanzaList
:stanzaList rdf:type owl:ObjectProperty ;
            rdfs:subPropertyOf <http://purl.org/ontology/olo/core#ordered_list> ;
            rdfs:domain :Stanza ;
            rdfs:range :StanzaList ;
            rdfs:comment """This property refers to the Stanza List that a Stanza belongs to.

For example, the line \"veo llegar la corta vida mía\" from the poem \"A la pequeña luz del breve dia\" by Fernando de Herrera belongs to the Redaction of the poem in Algunas obras (1582)."""@en ;
            rdfs:isDefinedBy "http://postdata.linhd.uned.es/ontology/postdata-poeticAnalysis#" ;
            rdfs:label "stanza list"@en .


###  http://postdata.linhd.uned.es/ontology/postdata-poeticAnalysis#typeOfAcrostic
:typeOfAcrostic rdf:type owl:ObjectProperty ;
                rdfs:domain :Acrostic ;
                rdfs:range <http://www.w3.org/2004/02/skos/core#Concept> ,
                           [ rdf:type owl:Restriction ;
                             owl:onProperty <http://www.w3.org/2004/02/skos/core#inScheme> ;
                             owl:hasValue <http://postdata.linhd.uned.es/kos/type-of-acrostic>
                           ] ;
                rdfs:label "type of acrostic"@en .


###  http://postdata.linhd.uned.es/ontology/postdata-poeticAnalysis#typeOfEnjambment
:typeOfEnjambment rdf:type owl:ObjectProperty ;
                  rdfs:domain :Enjambment ;
                  rdfs:range <http://www.w3.org/2004/02/skos/core#Concept> ,
                             [ rdf:type owl:Restriction ;
                               owl:onProperty <http://www.w3.org/2004/02/skos/core#inScheme> ;
                               owl:hasValue :type-of-enjambment
                             ] ;
                  rdfs:label "type of enjambment" .


###  http://postdata.linhd.uned.es/ontology/postdata-poeticAnalysis#typeOfIntertextuality
:typeOfIntertextuality rdf:type owl:ObjectProperty ;
                       rdfs:domain :Intertextuality ;
                       rdfs:range <http://www.w3.org/2004/02/skos/core#Concept> ,
                                  [ rdf:type owl:Restriction ;
                                    owl:onProperty <http://www.w3.org/2004/02/skos/core#inScheme> ;
                                    owl:hasValue <http://postdata.linhd.uned.es/kos/type-of-intertextuality>
                                  ] ;
                       rdfs:comment "Categorisation of the work under analysis depending on the relationship between this work and other texts. E.g. “contrafactum”, “de seguir”, etc."@en ;
                       rdfs:isDefinedBy "http://postdata.linhd.uned.es/ontology/postdata-poeticAnalysis#"@en ;
                       rdfs:label "type of intertextuality"@en .


###  http://postdata.linhd.uned.es/ontology/postdata-poeticAnalysis#typeOfMetaplasm
:typeOfMetaplasm rdf:type owl:ObjectProperty ;
                 rdfs:domain :Metaplasm ;
                 rdfs:range <http://www.w3.org/2004/02/skos/core#Concept> ,
                            [ rdf:type owl:Restriction ;
                              owl:onProperty <http://www.w3.org/2004/02/skos/core#inScheme> ;
                              owl:hasValue <http://postdata.linhd.uned.es/kos/metaplasm-type>
                            ] ;
                 rdfs:comment """Type of Metaplasm.

For example, if we consider the two words \"sparse il\" in the line from the sonnet I from the Canzoniere by Petrarca, namely \"Voi ch'ascoltate in rime sparse il suono\", the typeOfMetaplasm taking place across the two words is \"synaloepha\"."""@en ;
                 rdfs:label "type of metaplasm"@en .


###  http://postdata.linhd.uned.es/ontology/postdata-poeticAnalysis#typeOfNucleus
:typeOfNucleus rdf:type owl:ObjectProperty ;
               rdfs:domain :GrammaticalSyllable ;
               rdfs:range <http://www.w3.org/2004/02/skos/core#Concept> ,
                          [ rdf:type owl:Restriction ;
                            owl:onProperty <http://www.w3.org/2004/02/skos/core#inScheme> ;
                            owl:hasValue <http://postdata.linhd.uned.es/kos/nucleus-type>
                          ] ;
               rdfs:comment """Type of syllabic nucleus (linguistic typology).

For example, if we consider the first syllable of the word \"boca\" (i.e. \"bo\"), \"nucleusType\" is \"vowel\"."""@en ;
               rdfs:isDefinedBy "http://postdata.linhd.uned.es/ontology/postdata-poeticAnalysis#" ;
               rdfs:label "type of nucleus"@en .


###  http://postdata.linhd.uned.es/ontology/postdata-poeticAnalysis#typeOfRhymeMatching
:typeOfRhymeMatching rdf:type owl:ObjectProperty ;
                     rdfs:domain :Rhyme ;
                     rdfs:range <http://www.w3.org/2004/02/skos/core#Concept> ,
                                [ rdf:type owl:Restriction ;
                                  owl:onProperty <http://www.w3.org/2004/02/skos/core#inScheme> ;
                                  owl:hasValue <http://postdata.linhd.uned.es/kos/rhymeMatching-type>
                                ] ;
                     rdfs:comment """Explain the degree in which the different rhyming sounds match (e.g. assonant, consonant, perfect, imperfect, half-rhyme...).

For example, if we consider the rhyme \"scoloraro-legaro\" in the sonnet III from Petrarch's \"Canzoniere\", typeofRhymeMatching is \"perfect rhyme\". See the example lines:  \"Era il giorno ch’al sol si scoloraro \\ per la pietà del suo factore i rai,\\ quando i' fui preso, et non me ne guardai, \\ché i be' vostr'occhi, Donna, mi legaro\"."""@en ;
                     rdfs:isDefinedBy "http://postdata.linhd.uned.es/ontology/postdata-prosodicElements"@en ;
                     rdfs:label "type of rhyme matching"@en .


###  http://postdata.linhd.uned.es/ontology/postdata-poeticAnalysis#typeOfScansion
:typeOfScansion rdf:type owl:ObjectProperty ;
                rdfs:domain :Scansion ;
                rdfs:range <http://www.w3.org/2004/02/skos/core#Concept> ,
                           [ rdf:type owl:Restriction ;
                             owl:onProperty <http://www.w3.org/2004/02/skos/core#inScheme> ;
                             owl:hasValue :scansion-type
                           ] ;
                rdfs:comment "Specifies if the annotation is manual or automatic." ;
                rdfs:label "type of scansion" .


###  http://postdata.linhd.uned.es/ontology/postdata-poeticAnalysis#typeOfScheme
:typeOfScheme rdf:type owl:ObjectProperty ;
              rdfs:domain :Scheme ;
              rdfs:range <http://www.w3.org/2004/02/skos/core#Concept> ,
                         [ rdf:type owl:Restriction ;
                           owl:onProperty <http://www.w3.org/2004/02/skos/core#inScheme> ;
                           owl:hasValue <http://postdata.linhd.uned.es/kos/type-of-scheme>
                         ] ;
              rdfs:label "type of scheme"@en .


###  http://postdata.linhd.uned.es/ontology/postdata-poeticAnalysis#typeOfStanza
:typeOfStanza rdf:type owl:ObjectProperty ;
              rdfs:domain :Stanza ;
              rdfs:range <http://www.w3.org/2004/02/skos/core#Concept> ,
                         [ rdf:type owl:Restriction ;
                           owl:onProperty <http://www.w3.org/2004/02/skos/core#inScheme> ;
                           owl:hasValue <http://postdata.linhd.uned.es/kos/stanza-type>
                         ] ;
              rdfs:comment """Type of Stanza, but not in relation to its metrics. E.g. tornada, refrain.

For instance, the stanza \"Bailada, ten ta carrera/ e digues a la tan bella/ que heu m' i seray en breu\" from the anonymous poem \"Na dolça res, be m’es greu\" is a \"tornada\"."""@en ;
              rdfs:isDefinedBy "http://postdata.linhd.uned.es/ontology/postdata-poeticAnalysis#" ;
              rdfs:label "type of stanza"@en .


###  http://postdata.linhd.uned.es/ontology/postdata-poeticAnalysis#typeOfStanzaEdition
:typeOfStanzaEdition rdf:type owl:ObjectProperty ;
                     rdfs:domain :Stanza ;
                     rdfs:range <http://www.w3.org/2004/02/skos/core#Concept> ,
                                [ rdf:type owl:Restriction ;
                                  owl:onProperty <http://www.w3.org/2004/02/skos/core#inScheme> ;
                                  owl:hasValue <http://postdata.linhd.uned.es/kos/stanzaEdition-type>
                                ] ;
                     rdfs:comment """The type of the text provided in the Stanza. 
Eg.: Diplomatic edition, critical edition, translation

For instance, if we consider the first stanza of the Inferno of the Divina Commedia (i.e. \"Nel mezzo del cammin di nostra vita/ mi ritrovai per una selva oscura/ ché la diritta via era smarrita.\") from the critical edition \"La Divina Commedia. Inferno\" edited by A.M. Chiavacci Leonardi, the type of Stanza Edition will be \"critical edition\"."""@en ;
                     rdfs:isDefinedBy "http://postdata.linhd.uned.es/ontology/postdata-poeticAnalysis#" ;
                     rdfs:label "type of stanza edition"@en .


###  http://postdata.linhd.uned.es/ontology/postdata-poeticAnalysis#typeOfTrope
:typeOfTrope rdf:type owl:ObjectProperty ;
             rdfs:domain :Trope ;
             rdfs:range <http://www.w3.org/2004/02/skos/core#Concept> ,
                        [ rdf:type owl:Restriction ;
                          owl:onProperty <http://www.w3.org/2004/02/skos/core#inScheme> ;
                          owl:hasValue <http://postdata.linhd.uned.es/kos/type-of-trope>
                        ] ;
             rdfs:label "type of trope"@en .


###  http://postdata.linhd.uned.es/ontology/postdata-poeticAnalysis#usedAsInput
:usedAsInput rdf:type owl:ObjectProperty ;
             owl:inverseOf :wasInputFor ;
             rdfs:domain :ScansionProcess ;
             rdfs:range <http://postdata.linhd.uned.es/ontology/postdata-core#Redaction> ;
             rdfs:label "used as input" .


###  http://postdata.linhd.uned.es/ontology/postdata-poeticAnalysis#usedAsRedaction
:usedAsRedaction rdf:type owl:ObjectProperty ;
                 rdfs:domain :Intertextuality ;
                 rdfs:range <http://postdata.linhd.uned.es/ontology/postdata-core#Redaction> ;
                 rdfs:comment "This property points to the text under analysis (Redaction) which has been a source for the current cultural product"@en ;
                 rdfs:isDefinedBy "http://postdata.linhd.uned.es/ontology/postdata-poeticAnalysis#"@en ;
                 rdfs:label "used as redaction"@en .


###  http://postdata.linhd.uned.es/ontology/postdata-poeticAnalysis#usesAsSource
:usesAsSource rdf:type owl:ObjectProperty ;
              rdfs:domain :Intertextuality ;
              rdfs:range <http://postdata.linhd.uned.es/ontology/postdata-transmission#Manifestation> ;
              rdfs:comment "This property points to a cultural product (Intertextuality) which was a source for the work under analysis"@en ;
              rdfs:isDefinedBy "http://postdata.linhd.uned.es/ontology/postdata-poeticAnalysis#"@en ;
              rdfs:label "used as source"@en .


###  http://postdata.linhd.uned.es/ontology/postdata-poeticAnalysis#usesEncoding
:usesEncoding rdf:type owl:ObjectProperty ;
              rdfs:subPropertyOf owl:topObjectProperty ;
              rdfs:domain :ScansionProcess ;
              rdfs:range :MetricalEncoding ;
              <http://purl.org/dc/elements/1.1/creator> "mluisadiez" ;
              <http://purl.org/dc/elements/1.1/date> "2018-06-16T20:30:43Z"^^xsd:dateTime ;
              rdfs:comment """This property points to the instance of MetricalEncoding in which the conventions implemented in the item at hand are explained.

For example, in the poem \"Amadís de Gaula a don Quijote de La Mancha\", the presented metrical Pattern uses the following MetricalEncoding: the symbol \"+\" for stressed syllables and the symbol \"-\" for unstressed ones.""" ;
              rdfs:isDefinedBy "http://postdata.linhd.uned.es/ontology/postdata-prosodicElements"@en ;
              rdfs:label "uses encoding"@en .


###  http://postdata.linhd.uned.es/ontology/postdata-poeticAnalysis#versificationType
:versificationType rdf:type owl:ObjectProperty ;
                   rdfs:domain :RedactionPattern ;
                   rdfs:range <http://www.w3.org/2004/02/skos/core#Concept> ,
                              [ rdf:type owl:Restriction ;
                                owl:onProperty <http://www.w3.org/2004/02/skos/core#inScheme> ;
                                owl:hasValue <http://postdata.linhd.uned.es/kos/versification-type>
                              ] ;
                   rdfs:comment """Type of metre: accentual verse, accentual-syllabic verse, syllabic verse, quantitative verse, etc.

For example, if we consider the sonnet I from \"L'olive\" by Du Bellay, versificationType is \"syllabic verse\" because its type of versification is based on the number of syllables per line only."""@en ;
                   rdfs:isDefinedBy "http://postdata.linhd.uned.es/ontology/postdata-prosodicElements"@en ;
                   rdfs:label "versification type"@en .


###  http://postdata.linhd.uned.es/ontology/postdata-poeticAnalysis#wasInputFor
:wasInputFor rdf:type owl:ObjectProperty ;
             rdfs:domain <http://postdata.linhd.uned.es/ontology/postdata-core#Redaction> ;
             rdfs:range :ScansionProcess ;
             rdfs:label "was input for" .


###  http://postdata.linhd.uned.es/ontology/postdata-poeticAnalysis#word
:word rdf:type owl:ObjectProperty ;
      rdfs:subPropertyOf <http://purl.org/ontology/olo/core#slot> ;
      owl:inverseOf :wordList ;
      rdfs:domain :WordList ;
      rdfs:range :Word ;
      rdfs:comment """Word of a Line.

For example, the line \"Bruscamente la tarde se ha aclarado\" from the poem \"La lluvia\" by Jorge Luis Borges, has \"bruscamente\" as a token."""@en ;
      rdfs:isDefinedBy "http://postdata.linhd.uned.es/ontology/postdata-poeticAnalysis#" ;
      rdfs:label "word"@en .


###  http://postdata.linhd.uned.es/ontology/postdata-poeticAnalysis#wordList
:wordList rdf:type owl:ObjectProperty ;
          rdfs:subPropertyOf <http://purl.org/ontology/olo/core#ordered_list> ;
          rdfs:domain :Word ;
          rdfs:range :WordList ;
          rdfs:comment """This property refers to the Line that contains a given Word.

For example, the token \"April\" belongs to the line \"April is the cruellest month, breeding\" from the poem \"The Waste Land\" by T. S. Eliot."""@en ;
          rdfs:isDefinedBy "http://postdata.linhd.uned.es/ontology/postdata-poeticAnalysis#" ;
          rdfs:label "word list"@en .


###  http://purl.org/ontology/olo/core#has_first_slot
<http://purl.org/ontology/olo/core#has_first_slot> rdf:type owl:ObjectProperty ;
                                                   rdfs:domain <http://purl.org/ontology/olo/core#OrderedList> ;
                                                   rdfs:range <http://purl.org/ontology/olo/core#Slot> .


###  http://purl.org/ontology/olo/core#has_last_slot
<http://purl.org/ontology/olo/core#has_last_slot> rdf:type owl:ObjectProperty ;
                                                  rdfs:domain <http://purl.org/ontology/olo/core#OrderedList> ;
                                                  rdfs:range <http://purl.org/ontology/olo/core#Slot> .


###  http://purl.org/ontology/olo/core#is_first_slot_of
<http://purl.org/ontology/olo/core#is_first_slot_of> rdf:type owl:ObjectProperty ;
                                                     rdfs:domain <http://purl.org/ontology/olo/core#Slot> ;
                                                     rdfs:range <http://purl.org/ontology/olo/core#OrderedList> .


###  http://purl.org/ontology/olo/core#is_last_slot_of
<http://purl.org/ontology/olo/core#is_last_slot_of> rdf:type owl:ObjectProperty ;
                                                    rdfs:domain <http://purl.org/ontology/olo/core#Slot> ;
                                                    rdfs:range <http://purl.org/ontology/olo/core#OrderedList> .


###  http://purl.org/ontology/olo/core#next
<http://purl.org/ontology/olo/core#next> rdf:type owl:ObjectProperty ;
                                         rdfs:domain <http://purl.org/ontology/olo/core#Slot> ;
                                         rdfs:range <http://purl.org/ontology/olo/core#Slot> .


###  http://purl.org/ontology/olo/core#ordered_list
<http://purl.org/ontology/olo/core#ordered_list> rdf:type owl:ObjectProperty ;
                                                 rdfs:domain <http://purl.org/ontology/olo/core#Slot> ;
                                                 rdfs:range <http://purl.org/ontology/olo/core#OrderedList> .


###  http://purl.org/ontology/olo/core#previous
<http://purl.org/ontology/olo/core#previous> rdf:type owl:ObjectProperty ;
                                             rdfs:domain <http://purl.org/ontology/olo/core#Slot> ;
                                             rdfs:range <http://purl.org/ontology/olo/core#Slot> .


###  http://purl.org/ontology/olo/core#slot
<http://purl.org/ontology/olo/core#slot> rdf:type owl:ObjectProperty ;
                                         rdfs:domain <http://purl.org/ontology/olo/core#OrderedList> ;
                                         rdfs:range <http://purl.org/ontology/olo/core#Slot> .


###  http://www.w3.org/2002/07/owl#topObjectProperty
owl:topObjectProperty rdfs:domain owl:Thing .


###  http://www.w3.org/2004/02/skos/core#inScheme
<http://www.w3.org/2004/02/skos/core#inScheme> rdf:type owl:ObjectProperty .


#################################################################
#    Data properties
#################################################################

###  http://postdata.linhd.uned.es/ontology/postdata-core#text
<http://postdata.linhd.uned.es/ontology/postdata-core#text> rdf:type owl:DatatypeProperty ;
                                                            rdfs:domain <http://postdata.linhd.uned.es/ontology/postdata-core#LinguisticObject> ;
                                                            rdfs:range xsd:string ;
                                                            rdfs:comment "Full content of the literary resource. For example, the content of the  acrostic is  the letters that compose it." .


###  http://postdata.linhd.uned.es/ontology/postdata-poeticAnalysis#absoluteLineNumber
:absoluteLineNumber rdf:type owl:DatatypeProperty ;
                    rdfs:subPropertyOf <http://purl.org/ontology/olo/core#index> ;
                    rdfs:domain :Line ;
                    rdfs:range xsd:positiveInteger ;
                    rdfs:comment """Number of the Line (verse) in the Redaction.

For example, if we take the line \"segura playa i peligroso puerto\" of the poem \"Ô cara perdicion, ô dulce engaño\" by Fernando de Herrera, the absolute line number is 10."""@en ;
                    rdfs:isDefinedBy "http://postdata.linhd.uned.es/ontology/postdata-poeticAnalysis#" ;
                    rdfs:label "absolute line number"@en .


###  http://postdata.linhd.uned.es/ontology/postdata-poeticAnalysis#accentedVowels
:accentedVowels rdf:type owl:DatatypeProperty ;
                rdfs:subPropertyOf owl:topDataProperty ;
                rdfs:domain :LinePattern ;
                rdfs:range xsd:string ;
                <http://purl.org/dc/elements/1.1/creator> "mluisadiez" ;
                rdfs:comment """Stressed vowels in the order in which they occur in the text.

If we consider, for example, the line \"Suspiros y risas, colores y notas.\", from the first of the \"Rimas\" by Bécquer, the accentedVowels are: i i e o."""@en ;
                rdfs:isDefinedBy "http://postdata.linhd.uned.es/ontology/postdata-prosodicElements"@en ;
                rdfs:label "accented vowels"@en .


###  http://postdata.linhd.uned.es/ontology/postdata-poeticAnalysis#accentedVowelsPattern
:accentedVowelsPattern rdf:type owl:DatatypeProperty ;
                       rdfs:subPropertyOf owl:topDataProperty ;
                       rdfs:domain :LinePattern ;
                       rdfs:range xsd:string ;
                       <http://purl.org/dc/elements/1.1/creator> "mluisadiez" ;
                       rdfs:comment """Stressed vowels in a line, in alphabetical order to show sound repetitions.

For instance, if we consider the line from the 12th of the \"Rimas\" by Bécquer, namely \"Verdes como el mar, te quejas;\", accentedVowelsPattern is: a a e e e e e o o."""@en ;
                       rdfs:isDefinedBy "http://postdata.linhd.uned.es/ontology/postdata-prosodicElements"@en ;
                       rdfs:label "accented vowels pattern"@en .


###  http://postdata.linhd.uned.es/ontology/postdata-poeticAnalysis#altMoraeMetricalScheme
:altMoraeMetricalScheme rdf:type owl:DatatypeProperty ;
                        rdfs:domain :LinePattern ;
                        rdfs:range xsd:string ;
                        rdfs:comment """Alternative morae metrical schemaes.

For example, in the corpus of Middle High German, the line \"ein ritter sô gelêer was\" of the poem \"Der arme Heinrich\" by Hartmann von Aue has its morae metrical scheme presented in a different way from the system used in MoraeMetricalScheme, resulting the following altMoraeMetricalScheme: ein/MORA WBY rit/MORA_HAUPT ter/MORA WBY/WBY sô/MORA_HAUPT WBY/WBY ge/MORA lê/MORA_HAUPT er/MORA WBY/WBY was/MORA_HAUPT."""@en ;
                        rdfs:isDefinedBy "http://postdata.linhd.uned.es/ontology/postdata-prosodicElements" ;
                        rdfs:label "alt morae metrical scheme"@en .


###  http://postdata.linhd.uned.es/ontology/postdata-poeticAnalysis#altPatterningMetricalScheme
:altPatterningMetricalScheme rdf:type owl:DatatypeProperty ;
                             rdfs:subPropertyOf owl:topDataProperty ;
                             rdfs:domain :LinePattern ;
                             rdfs:range xsd:string ;
                             <http://purl.org/dc/elements/1.1/creator> "mluisadiez" ;
                             rdfs:comment """Distribution of stresses/long syllables, but, for instance, with the addition of punctuation marks to present word boundaries in the line.

For example, if we consider the line \"From fairest creatures we desire increase,\" from the first sonnet by Shakespeare, altPatterningMetricalScheme is \"-.+|-.+|-.+|.-+|.-+\" in which full stop indicates word boundary and \"|\" foot boundary.""" ;
                             rdfs:label "alt patterning metrical scheme"@en .


###  http://postdata.linhd.uned.es/ontology/postdata-poeticAnalysis#altRhymeScheme
:altRhymeScheme rdf:type owl:DatatypeProperty ;
                rdfs:subPropertyOf owl:topDataProperty ;
                rdfs:domain :StanzaPattern ;
                rdfs:range xsd:string ;
                <http://purl.org/dc/elements/1.1/creator> "mluisadiez" ;
                rdfs:comment """An alternative rhyme scheme (usually in relation with an alternative metrical scheme).

If we take as example the fourth stanza of the poem \"A mal estrany es la pena estranya\" by Ausiàs March (\"Envers alguns aço miracle par,\\ mas si·ns membram de Arnau Daniell\\ e de aquells que la terra·ls es vel, \\ sabrem Amor vers nos que pot mostrar.\\ Cella que am en egual de la vida, \\ mostre ’vorrir en fets y en continent:\\ quant li so prop, e d’ella sbayment,\\ ab continent de aver l’avorrida.\") we can use an altRhymeScheme which uses capitalisation to indicate femenine rhymes: abbaCddC.""" ;
                rdfs:isDefinedBy "http://postdata.linhd.uned.es/ontology/postdata-prosodicElements"@en ;
                rdfs:label "alt rhyme scheme"@en .


###  http://postdata.linhd.uned.es/ontology/postdata-poeticAnalysis#altSyllabicMetricalScheme
:altSyllabicMetricalScheme rdf:type owl:DatatypeProperty ;
                           rdfs:subPropertyOf owl:topDataProperty ;
                           rdfs:domain :LinePattern ;
                           rdfs:range xsd:string ;
                           <http://purl.org/dc/elements/1.1/creator> "mluisadiez" ;
                           rdfs:comment """Alternative syllabic metrical schemes (e.g. long lines with caesura opposite to short lines).

If we consider, for instance, the second line of the poem \"Te recuerdo como eras en el último otoño\" by Pablo Neruda, that is, \"Eras la boina gris y el corazón en calma\", this line has an altCountingMetricalScheme considering a caesura after \"gris\". As a result, altCountingMetricalScheme would be 7+7= 14, instead of 15."""@en ;
                           rdfs:isDefinedBy "http://postdata.linhd.uned.es/ontology/postdata-prosodicElements"@en ;
                           rdfs:label "alt syllabic metrical scheme"@en .


###  http://postdata.linhd.uned.es/ontology/postdata-poeticAnalysis#clausulaScheme
:clausulaScheme rdf:type owl:DatatypeProperty ;
                rdfs:subPropertyOf owl:topDataProperty ;
                rdfs:domain :StanzaPattern ;
                rdfs:range xsd:string ;
                <http://purl.org/dc/elements/1.1/creator> "mluisadiez" ;
                rdfs:comment """Pattern of clausulae, that is, the ending of a line determined by the number of unstressed syllables following the last stressed one.

For example, if we consider the second stanza from the poem \"Acaso...\" by Antonio Machado: \"Brotaban verdes hojas \\ de las hinchadas yemas del ramaje, \\ y flores amarillas, blancas, rojas, /\\alegraban la mancha del paisaje.\"the clausulaScheme is: 4 feminine endings."""@en ;
                rdfs:isDefinedBy "http://postdata.linhd.uned.es/ontology/postdata-prosodicElements"@en ;
                rdfs:label "clausula scheme"@en .


###  http://postdata.linhd.uned.es/ontology/postdata-poeticAnalysis#coda
:coda rdf:type owl:DatatypeProperty ;
      rdfs:subPropertyOf owl:topDataProperty ;
      rdfs:domain :GrammaticalSyllable ;
      rdfs:range xsd:string ;
      rdfs:comment """Sound or sounds that follow the nucleus.

For example in the word \"mar\" in Spanish, the coda of the syllable is \"r\".""" ;
      rdfs:isDefinedBy "http://postdata.linhd.uned.es/ontology/postdata-poeticAnalysis#" ;
      rdfs:label "coda"@en .


###  http://postdata.linhd.uned.es/ontology/postdata-poeticAnalysis#content
:content rdf:type owl:DatatypeProperty ;
         rdfs:subPropertyOf owl:topDataProperty ;
         rdfs:domain :StructuralUnit ;
         rdfs:range xsd:string ;
         rdfs:comment "Full textual content of a structural element (Redaction, Line, Stanza, Word or Syllable)"@en ;
         rdfs:isDefinedBy "http://postdata.linhd.uned.es/ontology/postdata-poeticAnalysis#" ;
         rdfs:label "content"@en .


###  http://postdata.linhd.uned.es/ontology/postdata-poeticAnalysis#ending
:ending rdf:type owl:DatatypeProperty ;
        rdfs:subPropertyOf owl:topDataProperty ;
        rdfs:domain :Rhyme ;
        rdfs:range xsd:string ;
        <http://purl.org/dc/elements/1.1/creator> "mluisadiez" ;
        <http://purl.org/dc/elements/1.1/date> "2018-06-16T18:39:21Z"^^xsd:dateTime ;
        rdfs:comment """Contents from the last stressed vowel of the rhyme to its end.

For instance, if we consider the rhyme word \"vida\" from the poem \"Morir soñando\" by Unamuno, ending is \"ida\"."""@en ;
        rdfs:isDefinedBy "http://postdata.linhd.uned.es/ontology/postdata-prosodicElements"@en ;
        rdfs:label "ending"@en .


###  http://postdata.linhd.uned.es/ontology/postdata-poeticAnalysis#finalConsonant
:finalConsonant rdf:type owl:DatatypeProperty ;
                rdfs:subPropertyOf owl:topDataProperty ;
                rdfs:domain :Rhyme ;
                rdfs:range xsd:string ;
                <http://purl.org/dc/elements/1.1/creator> "mluisadiez" ;
                <http://purl.org/dc/elements/1.1/date> "2018-06-16T18:39:21Z"^^xsd:dateTime ;
                rdfs:comment """Last consonant of rhyming word.

For example, if we consider the rhyming word \"infinito\" in the poem by Quevedo \"A un hombre de gran nariz\", which rhymes with \"frito\", the final consonant of the rhyming word is \"t\".""" ;
                rdfs:isDefinedBy "http://postdata.linhd.uned.es/ontology/postdata-prosodicElements"@en ;
                rdfs:label "final consonant"@en .


###  http://postdata.linhd.uned.es/ontology/postdata-poeticAnalysis#firstHemistich
:firstHemistich rdf:type owl:DatatypeProperty ;
                rdfs:domain :Line ;
                rdfs:range xsd:string ;
                rdfs:comment """This property points to the first division of a Line (an instance of Line) that forms  the first hemistich.

For example, if we consider the line \"Sous le flambeau d’Amour, des éternelles nuits\" from the sonnet \"Afin que pour jamais une marque demeure\" by Jean Antoine de Baïf, the \"firstHemistich\" of the line is \"Sous le flambeau d'Amour\"."""@en ;
                rdfs:isDefinedBy "http://postdata.linhd.uned.es/ontology/postdata-poeticAnalysis#" ;
                rdfs:label "first hemistich"@en .


###  http://postdata.linhd.uned.es/ontology/postdata-poeticAnalysis#footNumber
:footNumber rdf:type owl:DatatypeProperty ;
            rdfs:subPropertyOf <http://purl.org/ontology/olo/core#index> ;
            rdfs:domain :Foot ;
            rdfs:range xsd:nonNegativeInteger ;
            rdfs:label "foot number"@en .


###  http://postdata.linhd.uned.es/ontology/postdata-poeticAnalysis#grammaticalStressPattern
:grammaticalStressPattern rdf:type owl:DatatypeProperty ;
                          rdfs:subPropertyOf owl:topDataProperty ;
                          rdfs:domain :LinePattern ;
                          rdfs:range xsd:string ;
                          <http://purl.org/dc/elements/1.1/creator> "mluisadiez" ;
                          rdfs:comment """Pattern based on disposition of the expected stresses according to grammar rules. This includes the distribution of weak and strong positions.

For instance, if we consider the line \"Piedra soy en sufrir pena y cuidado\" from the homonym poem by Quevedo, grammaticalStressPattern is \"+-+--++---+-\" (while the metrical pattern would be +-+--+--+-, e.g. in the grammatical pattern both \"sufrir\" and \"pena\" have a stressed syllables, while in the metrical pattern \"sufrir\" is not stressed).""" ;
                          rdfs:isDefinedBy "http://postdata.linhd.uned.es/ontology/postdata-prosodicElements"@en ;
                          rdfs:label "grammatical stress pattern"@en .


###  http://postdata.linhd.uned.es/ontology/postdata-poeticAnalysis#grammaticalSyllableNumber
:grammaticalSyllableNumber rdf:type owl:DatatypeProperty ;
                           rdfs:subPropertyOf <http://purl.org/ontology/olo/core#index> ;
                           rdfs:domain :GrammaticalSyllable ;
                           rdfs:range xsd:positiveInteger ;
                           rdfs:comment """Position of the Syllable in the Word 

Eg.: 3/4 (= third syllable in a four-syllable word).
For example, in the Spanish word \"recordar\", the syllable \"cor\" is the second syllable of the word, so this field should be filled with 2/3."""@en ;
                           rdfs:isDefinedBy "http://postdata.linhd.uned.es/ontology/postdata-poeticAnalysis#" ;
                           rdfs:label "gramamtical syllable number"@en .


###  http://postdata.linhd.uned.es/ontology/postdata-poeticAnalysis#hasAnacrusis
:hasAnacrusis rdf:type owl:DatatypeProperty ;
              rdfs:subPropertyOf owl:topDataProperty ;
              rdfs:domain :LinePattern ;
              rdfs:range xsd:boolean ;
              <http://purl.org/dc/elements/1.1/creator> "mluisadiez" ;
              <http://purl.org/dc/elements/1.1/date> "2018-06-16T18:39:21Z"^^xsd:dateTime ;
              rdfs:comment """If the line has one or more unstressed syllables at the beginning of a line of verse, before the reckoning of the normal meter begins.

For instance, if we consider the line \"El que alaba la vida de la Corte\" from the sonnet by Cristóbal de Mesa, has Anacrusis is \"Yes\".""" ;
              rdfs:isDefinedBy "http://postdata.linhd.uned.es/ontology/postdata-prosodicElements"@en ;
              rdfs:label "has anacrusis"@en .


###  http://postdata.linhd.uned.es/ontology/postdata-poeticAnalysis#hasCaesura
:hasCaesura rdf:type owl:DatatypeProperty ;
            rdfs:subPropertyOf owl:topDataProperty ;
            rdfs:domain :LinePattern ;
            rdfs:range xsd:boolean ;
            <http://purl.org/dc/elements/1.1/creator> "mluisadiez" ;
            rdfs:comment """Whether it contains any lines with a pause/break near its middle.

If we consider, for example, the line \"Suspiros y risas, colores y notas.\", from the first of the \"Rimas\" by Bécquer, hasCaesura is negative because the line has no caesura.""" ;
            rdfs:isDefinedBy "http://postdata.linhd.uned.es/ontology/postdata-prosodicElements"@en ;
            rdfs:label "has caesura"@en .


###  http://postdata.linhd.uned.es/ontology/postdata-poeticAnalysis#hasMetaplasm
:hasMetaplasm rdf:type owl:DatatypeProperty ;
              rdfs:subPropertyOf owl:topDataProperty ;
              rdfs:domain :LinePattern ;
              rdfs:range xsd:boolean ;
              rdfs:comment """If the line, word or syllable is affected by a metaplasm.

If we consider, for example, the line from the first sonnet from the \"Canzoniere\" by Petrarca, namely \"Voi ch'ascoltate in rime sparse il suono\", hasMetaplasm is \"Yes\" because synaloepha occurs between \"-te\" (\"ascoltate\") and \"in\" and \"-se\" (\"sparse\") and \"il\"."""@en ;
              rdfs:isDefinedBy "http://postdata.linhd.uned.es/ontology/postdata-prosodicElements"@en ;
              rdfs:label "has metaplasm"@en .


###  http://postdata.linhd.uned.es/ontology/postdata-poeticAnalysis#hasRefrain
:hasRefrain rdf:type owl:DatatypeProperty ;
            rdfs:subPropertyOf owl:topDataProperty ;
            rdfs:domain :RedactionPattern ;
            rdfs:range xsd:boolean ;
            <http://purl.org/dc/elements/1.1/creator> "mluisadiez" ;
            <http://purl.org/dc/elements/1.1/date> "2018-06-16T18:39:21Z"^^xsd:dateTime ;
            rdfs:comment """Whether the work has a refrain.

For instance, if we consider the poem \"Señora de hermosura\" by Juan del Encina, hasRefrain would be affirmative, since it has a refrain.""" ;
            rdfs:label "has refrain"@en .


###  http://postdata.linhd.uned.es/ontology/postdata-poeticAnalysis#initialPhonemesPattern
:initialPhonemesPattern rdf:type owl:DatatypeProperty ;
                        rdfs:subPropertyOf owl:topDataProperty ;
                        rdfs:domain :LinePattern ;
                        rdfs:range xsd:string ;
                        <http://purl.org/dc/elements/1.1/creator> "mluisadiez" ;
                        rdfs:comment """Initial phonemes of each word in a line, in alphabetical order to show sound repetitions.

If we consider, for example, the line \"Suspiros y risas, colores y notas.\", from the first of the \"Rimas\" by Bécquer, initialPhonemesPattern is: [k ii n r s]."""@en ;
                        rdfs:isDefinedBy "http://postdata.linhd.uned.es/ontology/postdata-prosodicElements"@en ;
                        rdfs:label "initial phonemes pattern"@en .


###  http://postdata.linhd.uned.es/ontology/postdata-poeticAnalysis#initialPhonemesPatternByManner
:initialPhonemesPatternByManner rdf:type owl:DatatypeProperty ;
                                rdfs:domain :LinePattern ,
                                            [ rdf:type owl:Restriction ;
                                              owl:onProperty :initialPhonemesPatternByManner ;
                                              owl:maxQualifiedCardinality "1"^^xsd:nonNegativeInteger ;
                                              owl:onDataRange xsd:string
                                            ] ;
                                rdfs:range xsd:string ;
                                rdfs:comment """Initial phonemes of each word in a line represented by manner, in alphabetical order to show sound repetitions.

If we consider, for example, the line \"Suspiros y risas, colores y notas.\", from the first of the \"Rimas\" by Bécquer, initialPhonemesPatternByManner is: fricative, front vowel, front vowel, stop, stop."""@en ;
                                rdfs:isDefinedBy "http://postdata.linhd.uned.es/ontology/postdata-prosodicElements"@en ;
                                rdfs:label "initial phonemes pattern by manner"@en .


###  http://postdata.linhd.uned.es/ontology/postdata-poeticAnalysis#interStrophicRelations
:interStrophicRelations rdf:type owl:DatatypeProperty ;
                        rdfs:subPropertyOf owl:topDataProperty ;
                        rdfs:domain :RedactionPattern ;
                        rdfs:range xsd:string ;
                        <http://purl.org/dc/elements/1.1/creator> "mluisadiez" ;
                        <http://purl.org/dc/elements/1.1/date> "2018-06-16T18:39:21Z"^^xsd:dateTime ;
                        rdfs:comment """Type of technique used to related stanzas by the repetition of sounds.

For instance, the tercets of the Sonnet XI by Garcilaso are \"tercetos encadenados\", therefore their interStrophicRelations is \"rhyme: terza rima\".""" ;
                        rdfs:isDefinedBy "http://postdata.linhd.uned.es/ontology/postdata-prosodicElements"@en ;
                        rdfs:label "inter strophic relations"@en .


###  http://postdata.linhd.uned.es/ontology/postdata-poeticAnalysis#isCatalectic
:isCatalectic rdf:type owl:DatatypeProperty ;
              rdfs:subPropertyOf owl:topDataProperty ;
              rdfs:domain :Foot ;
              rdfs:range xsd:boolean ;
              <http://purl.org/dc/elements/1.1/creator> "mluisadiez" ;
              rdfs:comment """Whether the instance at hand is the last foot of the line or hemistich and is lacking one syllable.

If we consider, for instance, the foot \"shed\" of the line \"Stood a lowly cattle shed\" from the poem \"Once in Royal David's city\" by Cecil Frances Alexander, isCatalectic is \"Yes\" because the foot lacks one syllable. In fact, the line would be expected to be of eight syllables, as the previous line, and instead has one syllable missing. Compare the two lines: \"Once in Royal David's city\" (8 syllables) / \"Stood a lowly cattle shed,\" (7 syllables)."""@en ;
              rdfs:isDefinedBy "http://postdata.linhd.uned.es/ontology/postdata-prosodicElements"@en ;
              rdfs:label "is catalectic"@en .


###  http://postdata.linhd.uned.es/ontology/postdata-poeticAnalysis#isEcho
:isEcho rdf:type owl:DatatypeProperty ;
        rdfs:subPropertyOf owl:topDataProperty ;
        rdfs:domain :Rhyme ;
        rdfs:range xsd:boolean ;
        <http://purl.org/dc/elements/1.1/creator> "mluisadiez" ;
        <http://purl.org/dc/elements/1.1/date> "2018-06-16T18:39:21Z"^^xsd:dateTime ;
        rdfs:comment """Whether the word in a rhyming pair under analysis is the first one (false) or the second (true).

If we consider, for instance, the word \"scoloraro\" in the first line of the sonnet III from Petrarch's \"Canzoniere\", isEcho is \"False\". In fact, the echo would be \"legaro\", as can be observed in the following lines: \"Era il giorno ch’al sol si scoloraro/ per la pietà del suo factore i rai,/ quando i' fui preso, et non me ne guardai,/ché i be' vostr'occhi, Donna, mi legaro\"."""@en ;
        rdfs:isDefinedBy "http://postdata.linhd.uned.es/ontology/postdata-prosodicElements"@en ;
        rdfs:label "is echo"@en .


###  http://postdata.linhd.uned.es/ontology/postdata-poeticAnalysis#isHypermetre
:isHypermetre rdf:type owl:DatatypeProperty ;
              rdfs:subPropertyOf owl:topDataProperty ;
              rdfs:domain :LinePattern ;
              rdfs:range xsd:boolean ;
              <http://purl.org/dc/elements/1.1/creator> "mluisadiez" ;
              <http://purl.org/dc/elements/1.1/date> "2018-06-16T18:39:21Z"^^xsd:dateTime ;
              rdfs:comment """It has one or more syllables in addition to those found in a standard metrical unit or line of verse.

For instance, if we consider the line \"intorno la croce.\" from the poem \"La figlia maggiore\" by Pascoli, isHypermetre is \"Yes\" because the line should have five syllables and instead has six syllables."""@en ;
              rdfs:isDefinedBy "http://postdata.linhd.uned.es/ontology/postdata-prosodicElements"@en ;
              rdfs:label "is hypermetre"@en .


###  http://postdata.linhd.uned.es/ontology/postdata-poeticAnalysis#isHypermetrical
:isHypermetrical rdf:type owl:DatatypeProperty ;
                 rdfs:subPropertyOf owl:topDataProperty ;
                 rdfs:domain :Foot ;
                 rdfs:range xsd:boolean ;
                 <http://purl.org/dc/elements/1.1/creator> "mluisadiez" ;
                 rdfs:comment """Whether the instance at hand is the last foot of the line or hemistich and it contains extra syllables.

If we consider, for instance, the foot \"From fai\" in the line \"From fairest creatures we desire increase,\" from the first sonnet by Shakespeare, isHypermetrical is \"No\" because that foot is part of the metrical pattern of the line: from FAI | rest CREA | tures WE | deSIRE | inCREASE."""@en ;
                 rdfs:isDefinedBy "http://postdata.linhd.uned.es/ontology/postdata-prosodicElements"@en ;
                 rdfs:label "is hypermetrical"@en .


###  http://postdata.linhd.uned.es/ontology/postdata-poeticAnalysis#isHypometre
:isHypometre rdf:type owl:DatatypeProperty ;
             rdfs:subPropertyOf owl:topDataProperty ;
             rdfs:domain :LinePattern ;
             rdfs:range xsd:boolean ;
             <http://purl.org/dc/elements/1.1/creator> "mluisadiez" ;
             <http://purl.org/dc/elements/1.1/date> "2018-06-16T18:39:21Z"^^xsd:dateTime ;
             rdfs:comment """It has one or more syllables less than to those found in a standard metrical unit or line of verse.

For instance, if we consider the line \"e benedico quel dolce varco\" from the sonnet \"Sonecto d’amore di misser Guliermo maramauro de Napoli\" by Marmaldo, isHypometre is \"Yes\"  because the line is one syllable shorter (i.e. 9 syllables) than the other lines in the poems which are all hendecasyllables. This can be observed by comparing the syllable length of the surrounding lines: \"Io benedico il duro ferro e l’arco (10) / col qual mi fo passato in prima il core, (10)/ e sempre benedico e lodo Amore (10)/ che m’à del suo piacer si forte carco; (10)/ e benedico quel dolce varco (9)\"."""@en ;
             rdfs:isDefinedBy "http://postdata.linhd.uned.es/ontology/postdata-prosodicElements"@en ;
             rdfs:label "is hypometre"@en .


###  http://postdata.linhd.uned.es/ontology/postdata-poeticAnalysis#isIrregular
:isIrregular rdf:type owl:DatatypeProperty ;
             rdfs:subPropertyOf owl:topDataProperty ;
             rdfs:domain :Foot ;
             rdfs:range xsd:boolean ;
             <http://purl.org/dc/elements/1.1/creator> "mluisadiez" ;
             rdfs:comment """Whether in comparison to the other lines, the current foot breaks a regular pattern.

If we consider, for instance, the first foot of the line \"Pity the world, or else this glutton be,\" from the first sonnet by Shakespeare, isIrregular is \"Yes\" because the sonnet is in iambic pentameters but the first foot of this line, namely \"Pity\", is a trochee. The metrical scansion of the line is: PIty | the WORLD | or ELSE | this GLUT | ton Be."""@en ;
             rdfs:isDefinedBy "http://postdata.linhd.uned.es/ontology/postdata-prosodicElements"@en ;
             rdfs:label "is irregular"@en .


###  http://postdata.linhd.uned.es/ontology/postdata-poeticAnalysis#isIsometric
:isIsometric rdf:type owl:DatatypeProperty ;
             rdfs:subPropertyOf owl:topDataProperty ;
             rdfs:domain :RedactionPattern ;
             rdfs:range xsd:boolean ;
             <http://purl.org/dc/elements/1.1/creator> "mluisadiez" ;
             <http://purl.org/dc/elements/1.1/date> "2018-06-16T18:39:21Z"^^xsd:dateTime ;
             rdfs:comment """Whether the work is monometric, that is, if all lines have the same metrical analysis.

If we consider, for example, the sonnet III from the \"Canzoniere\" by Petrarca, isIsometric is \"Yes\" because all lines are hendecasyllables, hence, they have the same metrical analysis.""" ;
             rdfs:isDefinedBy "http://postdata.linhd.uned.es/ontology/postdata-prosodicElements"@en ;
             rdfs:label "is isometric"@en .


###  http://postdata.linhd.uned.es/ontology/postdata-poeticAnalysis#isIsostrophic
:isIsostrophic rdf:type owl:DatatypeProperty ;
               rdfs:subPropertyOf owl:topDataProperty ;
               rdfs:domain :RedactionPattern ;
               rdfs:range xsd:boolean ;
               <http://purl.org/dc/elements/1.1/creator> "mluisadiez" ;
               <http://purl.org/dc/elements/1.1/date> "2018-06-16T18:39:21Z"^^xsd:dateTime ;
               rdfs:comment """Whether all stanzas are metrically equivalent.

If we consider for example the poem \"Canción de otoño en primavera\" by Rubén Darío, isIsostrophic is \"Yes\" because all stanzas of the poem have the same length and the same metrical characteristics.""" ;
               rdfs:isDefinedBy "http://postdata.linhd.uned.es/ontology/postdata-prosodicElements"@en ;
               rdfs:label "is isotrophic"@en .


###  http://postdata.linhd.uned.es/ontology/postdata-poeticAnalysis#isMetricStanza
:isMetricStanza rdf:type owl:DatatypeProperty ;
                rdfs:subPropertyOf owl:topDataProperty ;
                rdfs:domain :Stanza ;
                rdfs:range xsd:boolean ;
                rdfs:comment """If Stanza is a metrical unit, then this should be True. Otherwise (e.g. a section, a lai, a refrain, etc) it should be set to False.

If we consider, for example, the first stanza of the poem \"Caracola\" by Federico García Lorca, this property would be False because that stanza is a refrain, hence, it does not have a specific metrical scheme."""@en ;
                rdfs:isDefinedBy "http://postdata.linhd.uned.es/ontology/postdata-poeticAnalysis#" ;
                rdfs:label "is metric stanza"@en .


###  http://postdata.linhd.uned.es/ontology/postdata-poeticAnalysis#isRefrain
:isRefrain rdf:type owl:DatatypeProperty ;
           rdfs:domain :Line ;
           rdfs:range xsd:boolean ;
           rdfs:comment """Whether a Line contains or is part of a refrain.

If we consider, for example, the first stanza of the poem \"Caracola\" by Federico Garcia Lorca, \"iSNotMetricStanza\" would be True because that stanza is a refrain."""@en ;
           rdfs:isDefinedBy "http://postdata.linhd.uned.es/ontology/postdata-poeticAnalysis#" ;
           rdfs:label "is refrain"@en .


###  http://postdata.linhd.uned.es/ontology/postdata-poeticAnalysis#isRegular
:isRegular rdf:type owl:DatatypeProperty ;
           rdfs:subPropertyOf owl:topDataProperty ;
           rdfs:domain :LinePattern ;
           rdfs:range xsd:boolean ;
           <http://purl.org/dc/elements/1.1/creator> "mluisadiez" ;
           <http://purl.org/dc/elements/1.1/date> "2018-06-16T18:39:21Z"^^xsd:dateTime ;
           rdfs:comment """Regular metrics.

For example, if we take as example the poem \"Osé y temí mas pudo la osadía\" by Fernando de Herrera, LinePattern isRegular since it is a sonnet and all the lines are hendecasyllables."""@en ;
           rdfs:isDefinedBy "http://postdata.linhd.uned.es/ontology/postdata-prosodicElements"@en ;
           rdfs:label "is regular"@en .


###  http://postdata.linhd.uned.es/ontology/postdata-poeticAnalysis#isStressed
:isStressed rdf:type owl:DatatypeProperty ;
            rdfs:subPropertyOf owl:topDataProperty ;
            rdfs:domain :MetricalSyllable ;
            rdfs:range xsd:boolean ;
            rdfs:comment """If the syllable has accent.

For example, if we take the syllable \"-ñar\" word \"soñar\" in the line \"Soñar la muerte no es matar el sueño\" from the poem \"Morir soñando\" by Unamuno, isStressed is \"Yes\"."""@en ;
            rdfs:isDefinedBy "http://postdata.linhd.uned.es/ontology/postdata-prosodicElements"@en ;
            rdfs:label "is stressed"@en .


###  http://postdata.linhd.uned.es/ontology/postdata-poeticAnalysis#isUnissonant
:isUnissonant rdf:type owl:DatatypeProperty ;
              rdfs:subPropertyOf owl:topDataProperty ;
              rdfs:domain :RedactionPattern ;
              rdfs:range xsd:boolean ;
              <http://purl.org/dc/elements/1.1/creator> "mluisadiez" ;
              <http://purl.org/dc/elements/1.1/date> "2018-06-16T18:39:21Z"^^xsd:dateTime ;
              rdfs:comment """Whether all stanzas have the same rhyme.

If we take as example the poem \"Cortesamen vuoill comensar\" by the trobador Marcabru, isUnissonant is true, since all the stanzas have the same rhyme.""" ;
              rdfs:isDefinedBy "http://postdata.linhd.uned.es/ontology/postdata-prosodicElements"@en ;
              rdfs:label "is unissonant"@en .


###  http://postdata.linhd.uned.es/ontology/postdata-poeticAnalysis#lemma
:lemma rdf:type owl:DatatypeProperty ;
       rdfs:subPropertyOf owl:topDataProperty ;
       rdfs:domain :Word ;
       rdfs:range xsd:string ;
       rdfs:comment """A lemma is a Word that stands at the head of a definition in a dictionary. All the head words in a dictionary are lemmas. Technically, it is \"a base Word and its inflections\".

For example, for the verbal forms \"querer\", \"querremos\" and \"quería\", the lemma is \"querer\"."""@en ;
       rdfs:isDefinedBy "http://postdata.linhd.uned.es/ontology/postdata-poeticAnalysis#" ;
       rdfs:label "lemma"@en ;
       rdfs:seeAlso "https://simple.wikipedia.org/wiki/Lemma_(linguistics)" .


###  http://postdata.linhd.uned.es/ontology/postdata-poeticAnalysis#metricalNotes
:metricalNotes rdf:type owl:DatatypeProperty ;
               rdfs:subPropertyOf owl:topDataProperty ;
               rdfs:domain :Pattern ;
               rdfs:range xsd:string ;
               <http://purl.org/dc/elements/1.1/creator> "mluisadiez" ;
               <http://purl.org/dc/elements/1.1/date> "2018-06-16T18:39:21Z"^^xsd:dateTime ;
               rdfs:comment """Metrical commentary.

For example, the poem \"A creer devemos que todo pecado\" contains the following metrical commentary in the Cantigas de Santa María for Singers Database: \"Synaeresis, which is common in forms of the verb veer (= \"to see\"), is required here to reduce viía to two metrical syllables (contrast line 24 where it has its natural three). The compressed syllable vii- benefits from a long note  in the music, however\"""" ;
               rdfs:isDefinedBy "http://postdata.linhd.uned.es/ontology/postdata-prosodicElements"@en ;
               rdfs:label "metrical notes"@en .


###  http://postdata.linhd.uned.es/ontology/postdata-poeticAnalysis#metricalSyllableNumber
:metricalSyllableNumber rdf:type owl:DatatypeProperty ;
                        rdfs:subPropertyOf <http://purl.org/ontology/olo/core#index> ;
                        rdfs:domain :MetricalSyllable ;
                        rdfs:range xsd:nonNegativeInteger ;
                        rdfs:label "metrical syllable number"@en .


###  http://postdata.linhd.uned.es/ontology/postdata-poeticAnalysis#metricalSymbol
:metricalSymbol rdf:type owl:DatatypeProperty ;
                rdfs:domain :Symbol ;
                rdfs:range xsd:string ;
                rdfs:comment """Symbol use to define a feature in a metrical pattern.

For example, the symbol \"+\" is used as metricalSymbol of an stressed syllable."""@en ;
                rdfs:isDefinedBy "http://postdata.linhd.uned.es/ontology/postdata-prosodicElements"@en ;
                rdfs:label "metrical symbol"@en .


###  http://postdata.linhd.uned.es/ontology/postdata-poeticAnalysis#moraNumber
:moraNumber rdf:type owl:DatatypeProperty ;
            rdfs:subPropertyOf <http://purl.org/ontology/olo/core#index> ;
            rdfs:domain :Mora ;
            rdfs:range xsd:nonNegativeInteger ;
            rdfs:label "mora number"@en .


###  http://postdata.linhd.uned.es/ontology/postdata-poeticAnalysis#moraeMetricalScheme
:moraeMetricalScheme rdf:type owl:DatatypeProperty ;
                     rdfs:domain :LinePattern ;
                     rdfs:range xsd:string ;
                     rdfs:comment """Metrical scheme according to the number of morae.

For instance, the metrical analysis of the 616th line of the Bacchae by Euripides is: 
(—x. . x.)   (. x. . x.) (. x. . x.)(x. x. . x.) (the transliterated text is \"ta ́u.ta ka`ı ka.thu ́b.ris’ au.to ́n ho ́.te me des.meu ́.ein do.ko ́on\")."""@en ;
                     rdfs:isDefinedBy "http://postdata.linhd.uned.es/ontology/postdata-prosodicElements" ;
                     rdfs:label "morae metrical scheme"@en .


###  http://postdata.linhd.uned.es/ontology/postdata-poeticAnalysis#morphologicalAnnotation
:morphologicalAnnotation rdf:type owl:DatatypeProperty ;
                         rdfs:subPropertyOf owl:topDataProperty ;
                         rdfs:domain :Word ;
                         rdfs:range xsd:string ;
                         rdfs:comment """Any type of morphological analysis (from POS to morpheme composition).

For example, for the word \"rojos\" , the morphological composition is the following: \"roj\" is the stem, \"o\" is the inflectional morpheme indicating masculine and \"s\" in the inflectional morpheme indicating plural."""@en ;
                         rdfs:isDefinedBy "http://postdata.linhd.uned.es/ontology/postdata-poeticAnalysis#" ;
                         rdfs:label "morphological annotation"@en .


###  http://postdata.linhd.uned.es/ontology/postdata-poeticAnalysis#nucleus
:nucleus rdf:type owl:DatatypeProperty ;
         rdfs:domain :GrammaticalSyllable ;
         rdfs:range xsd:string ;
         rdfs:label "nucleus"@en .


###  http://postdata.linhd.uned.es/ontology/postdata-poeticAnalysis#numberOfFeet
:numberOfFeet rdf:type owl:DatatypeProperty ;
              rdfs:subPropertyOf <http://purl.org/ontology/olo/core#length> ;
              rdfs:domain :FootList ;
              rdfs:range xsd:positiveInteger ;
              <http://purl.org/dc/elements/1.1/creator> "mluisadiez" ;
              <http://purl.org/dc/elements/1.1/date> "2018-06-16T18:39:21Z"^^xsd:dateTime ;
              rdfs:comment """Number of feet.

If we consider the first line of the first sonnet by Shakespeare, namely \"From fairest creatures we desire increase,\" the numberOfFeet is: 5"""@en ;
              rdfs:isDefinedBy "http://postdata.linhd.uned.es/ontology/postdata-prosodicElements"@en ;
              rdfs:label "number of feet"@en .


###  http://postdata.linhd.uned.es/ontology/postdata-poeticAnalysis#numberOfGrammaticalSyllables
:numberOfGrammaticalSyllables rdf:type owl:DatatypeProperty ;
                              rdfs:subPropertyOf <http://purl.org/ontology/olo/core#length> ,
                                                 owl:topDataProperty ;
                              rdfs:domain :GrammaticalSyllableList ;
                              rdfs:range xsd:positiveInteger ;
                              <http://purl.org/dc/elements/1.1/creator> "mluisadiez" ;
                              <http://purl.org/dc/elements/1.1/date> "2018-06-16T18:39:21Z"^^xsd:dateTime ;
                              rdfs:comment "The exact number of syllables of a Word, that is, without paying attention to any metrical phenomena that may affect the counting"@en ,
                                           """The exact number of syllables, that is, without paying attention to any metrical phenomena that may affect the counting.

If we consider the first hendecasyllable line of the sonnet I by Petrarca, namely \"Voi ch'ascoltate in rime sparse il suono\", and disregard any metrical phenomena (e.g. synaloepha), numberOfSyllables is: 13."""@en ;
                              rdfs:isDefinedBy "http://postdata.linhd.uned.es/ontology/postdata-prosodicElements"@en ,
                                               "http://postdata.linhd.uned.es/ontology/postdata-poeticAnalysis#" ;
                              rdfs:label "number of grammatical syllables"@en .


###  http://postdata.linhd.uned.es/ontology/postdata-poeticAnalysis#numberOfLines
:numberOfLines rdf:type owl:DatatypeProperty ;
               rdfs:subPropertyOf <http://purl.org/ontology/olo/core#length> ;
               rdfs:domain :LineList ;
               rdfs:range xsd:positiveInteger ;
               <http://purl.org/dc/elements/1.1/creator> "mluisadiez" ;
               <http://purl.org/dc/elements/1.1/date> "2018-06-16T18:39:21Z"^^xsd:dateTime ;
               rdfs:comment "The total number of lines of a Line List"@en ,
                            """Number of lines in item.

If we consider the second stanza from the poem \"Acaso...\" by Antonio Machado:     \"Brotaban verdes hojas \\ de las hinchadas yemas del ramaje, \\ y flores amarillas, blancas, rojas, /\\alegraban la mancha del paisaje.\" numberOFLines is: 4.""" ;
               rdfs:isDefinedBy "http://postdata.linhd.uned.es/ontology/postdata-prosodicElements"@en ,
                                "http://postdata.linhd.uned.es/ontology/postdata-poeticAnalysis#" ;
               rdfs:label "number of lines"@en .


###  http://postdata.linhd.uned.es/ontology/postdata-poeticAnalysis#numberOfMetricalSyllables
:numberOfMetricalSyllables rdf:type owl:DatatypeProperty ;
                           rdfs:subPropertyOf <http://purl.org/ontology/olo/core#length> ;
                           rdfs:domain :MetricalSyllableList ;
                           rdfs:range xsd:positiveInteger ;
                           rdfs:label "number of metrical syllables"@en .


###  http://postdata.linhd.uned.es/ontology/postdata-poeticAnalysis#numberOfMorae
:numberOfMorae rdf:type owl:DatatypeProperty ;
               rdfs:subPropertyOf <http://purl.org/ontology/olo/core#length> ;
               rdfs:domain :MoraList ;
               rdfs:range xsd:positiveInteger ;
               <http://purl.org/dc/elements/1.1/creator> "mluisadiez" ;
               rdfs:comment """The number of morae the foot contains.

If we consider first dactylic foot of the line 51 from Ovid's Tristia: \"Vergilium vidi tantum, nec avara Tibullo\" (Vergĭlĭ | um vī | dī tan | tum, nĕc ă | māră Tĭ | bullō), namely \"Vergili\", numberOfMorae is: 4."""@en ;
               rdfs:isDefinedBy "http://postdata.linhd.uned.es/ontology/postdata-prosodicElements"@en ;
               rdfs:label "number of morae"@en .


###  http://postdata.linhd.uned.es/ontology/postdata-poeticAnalysis#numberOfPunctuations
:numberOfPunctuations rdf:type owl:DatatypeProperty ;
                      rdfs:subPropertyOf <http://purl.org/ontology/olo/core#length> ;
                      rdfs:domain :PunctuationList ;
                      rdfs:range xsd:positiveInteger ;
                      rdfs:comment "Total number of punctuation in a Punctuation List."@en ;
                      rdfs:isDefinedBy "http://postdata.linhd.uned.es/ontology/postdata-poeticAnalysis#" ;
                      rdfs:label "number of punctuations" .


###  http://postdata.linhd.uned.es/ontology/postdata-poeticAnalysis#numberOfStanzas
:numberOfStanzas rdf:type owl:DatatypeProperty ;
                 rdfs:subPropertyOf <http://purl.org/ontology/olo/core#length> ;
                 rdfs:domain :StanzaList ;
                 rdfs:range xsd:positiveInteger ;
                 <http://purl.org/dc/elements/1.1/creator> "mluisadiez" ;
                 <http://purl.org/dc/elements/1.1/date> "2018-06-16T18:39:21Z"^^xsd:dateTime ;
                 rdfs:comment "The total number of stanzas of a Stanza List"@en ,
                              """Number of stanzas.

\"If we consider the poem \"Acaso...\" by Antonio Machado: \"Como atento no más a mi quimera \\ no reparaba en torno mío, un día  \\ me sorprendió la fértil primavera \\ que en todo el ancho campo sonreía. 

Brotaban verdes hojas  \\ de las hinchadas \\ yemas del ramaje, \\ y flores amarillas, blancas, rojas, \\ alegraban la mancha del paisaje. 

Y era una lluvia de saetas de oro, \\ el sol sobre las frondas juveniles; \\ del amplio río en el caudal sonoro \\ se miraban los álamos gentiles. 

Tras de tanto camino es la primera \\ vez que miro brotar la primavera, \\ dije, y después, declamatoriamente: 

¿¡Cuán tarde ya para la dicha mía!? \\ Y luego, al caminar, como quien siente \\ alas de otra ilusión: Y todavía \\ ¡yo alcanzaré mi juventud un día!\" Number of stanza is: 5.""" ;
                 rdfs:isDefinedBy "http://postdata.linhd.uned.es/ontology/postdata-prosodicElements"@en ,
                                  "http://postdata.linhd.uned.es/ontology/postdata-poeticAnalysis#" ;
                 rdfs:label "number of stanzas"@en .


###  http://postdata.linhd.uned.es/ontology/postdata-poeticAnalysis#numberOfWords
:numberOfWords rdf:type owl:DatatypeProperty ;
               rdfs:subPropertyOf <http://purl.org/ontology/olo/core#length> ;
               rdfs:domain :WordList ;
               rdfs:range xsd:positiveInteger ;
               rdfs:comment "The total number of words of a Line"@en ;
               rdfs:isDefinedBy "http://postdata.linhd.uned.es/ontology/postdata-poeticAnalysis#" ;
               rdfs:label "number of words"@en .


###  http://postdata.linhd.uned.es/ontology/postdata-poeticAnalysis#onset
:onset rdf:type owl:DatatypeProperty ;
       rdfs:subPropertyOf owl:topDataProperty ;
       rdfs:domain :GrammaticalSyllable ;
       rdfs:range xsd:string ;
       rdfs:comment """Sound or sounds occurring before the nucleus, a consonant or consonant cluster.

For example, in the word \"mar\" in Spanish, the syllable onset is \"m\"."""@en ;
       rdfs:isDefinedBy "http://postdata.linhd.uned.es/ontology/postdata-poeticAnalysis#" ;
       rdfs:label "onset"@en .


###  http://postdata.linhd.uned.es/ontology/postdata-poeticAnalysis#paraphrasis
:paraphrasis rdf:type owl:DatatypeProperty ;
             rdfs:subPropertyOf owl:topDataProperty ;
             rdfs:domain :Stanza ;
             rdfs:range xsd:string ;
             rdfs:comment """The recasting of the contents in words different from that originally used, whether in the same language or in a translation.

For example, a possible paraphrasis of the famous first tercet of Dante's \"Divina Commedia\" is:\"A metà del nostro cammino di vita terrena mi trovai in un bosco scuro e buio poiché avevo perso la retta via\"."""@en ;
             rdfs:isDefinedBy "http://postdata.linhd.uned.es/ontology/postdata-poeticAnalysis#" ;
             rdfs:label "paraphrasis"@en .


###  http://postdata.linhd.uned.es/ontology/postdata-poeticAnalysis#patterningMetricalScheme
:patterningMetricalScheme rdf:type owl:DatatypeProperty ;
                          rdfs:subPropertyOf owl:topDataProperty ;
                          rdfs:domain :LinePattern ;
                          rdfs:range xsd:string ;
                          <http://purl.org/dc/elements/1.1/creator> "mluisadiez" ;
                          <http://purl.org/dc/elements/1.1/date> "2018-06-16T18:39:21Z"^^xsd:dateTime ;
                          rdfs:comment """Metrical scheme for quantitative, tonal, accentual or accentual-syllabic metre.

If we consider the line \"From fairest creatures we desire increase,\" from the first sonnet by Shakespeare, patterningMetricalScheme is: -+-+-+-+-+""" ;
                          rdfs:isDefinedBy "http://postdata.linhd.uned.es/ontology/postdata-prosodicElements"@en ;
                          rdfs:label "patterning metrical scheme"@en .


###  http://postdata.linhd.uned.es/ontology/postdata-poeticAnalysis#phonemePattern
:phonemePattern rdf:type owl:DatatypeProperty ;
                rdfs:subPropertyOf owl:topDataProperty ;
                rdfs:domain :LinePattern ;
                rdfs:range xsd:string ;
                <http://purl.org/dc/elements/1.1/creator> "mluisadiez" ;
                <http://purl.org/dc/elements/1.1/date> "2018-06-16T18:39:21Z"^^xsd:dateTime ;
                rdfs:comment """All phonemes in a line represented by their nearest written equivalents. They could be arranged in alphabetical order to show sound repetitions.

If we take, for example, the line \"Si quejas y lamentos pueden tanto,\" from the sonnet \"Si quejas y lamentos puedan tanto\" by Garcilaso, the phonemePattern is \"aaa d eeee ii k l m nnn oo p sss ttt w x\""""@en ;
                rdfs:isDefinedBy "http://postdata.linhd.uned.es/ontology/postdata-prosodicElements"@en ;
                rdfs:label "phoneme pattern"@en .


###  http://postdata.linhd.uned.es/ontology/postdata-poeticAnalysis#phonemePatternByManner
:phonemePatternByManner rdf:type owl:DatatypeProperty ;
                        rdfs:subPropertyOf owl:topDataProperty ;
                        rdfs:domain :LinePattern ;
                        rdfs:range xsd:string ;
                        <http://purl.org/dc/elements/1.1/creator> "mluisadiez" ;
                        <http://purl.org/dc/elements/1.1/date> "2018-06-16T18:39:21Z"^^xsd:dateTime ;
                        rdfs:comment """All phonemes in a line represented by manner of articulation. They could be arranged in alphabetical order to show sound repetitions. The coding scheme presented in one of the databases stands for the different manners of articulation of consonants, and at the same time groups together front and back vowels.

If we take, for example, the line \"Si quejas y lamentos pueden tanto,\" from the sonnet \"Si quejas y lamentos puedan tanto\" by Garcilaso, the phonemePatternByManner is: fricative, front vowel, stop, front vowel, fricative, front vowel, fricative, front vowel, liquid, front vowel, stop, front vowel, stop, stop, back vowel, fricative, stop, back vowel, front vowel, fricative, front vowel, nasal, stop, front vowel, stop, stop, back vowel."""@en ;
                        rdfs:isDefinedBy "http://postdata.linhd.uned.es/ontology/postdata-prosodicElements"@en ;
                        rdfs:label "phoneme pattern by manner"@en .


###  http://postdata.linhd.uned.es/ontology/postdata-poeticAnalysis#phoneticTranscription
:phoneticTranscription rdf:type owl:DatatypeProperty ;
                       rdfs:subPropertyOf owl:topDataProperty ;
                       rdfs:domain :AnalyticalUnit ;
                       rdfs:range xsd:string ;
                       <http://purl.org/dc/elements/1.1/creator> "mluisadiez" ;
                       <http://purl.org/dc/elements/1.1/date> "2018-06-16T18:39:21Z"^^xsd:dateTime ;
                       rdfs:comment """Phonetic transcription

For example, in the case of the Spanish word \"novio\", the phonetic transcription is ['nɔ.βjo]."""@en ,
                                    """Phonetic transcription.

If we consider, as an example, the line \"Soñar la muerte no es matar el sueño\" from the poem \"Morir soñando\" by Unamuno, phoneticTranscription is: /so'ɲar la 'mwerte no es ma'tar el 'sweɲo/."""@en ;
                       rdfs:isDefinedBy "http://postdata.linhd.uned.es/ontology/postdata-prosodicElements"@en ,
                                        "http://postdata.linhd.uned.es/ontology/postdata-poeticAnalysis#" ;
                       rdfs:label "phonetic transcription"@en .


###  http://postdata.linhd.uned.es/ontology/postdata-poeticAnalysis#prefinalConsonants
:prefinalConsonants rdf:type owl:DatatypeProperty ;
                    rdfs:subPropertyOf owl:topDataProperty ;
                    rdfs:domain :Rhyme ;
                    rdfs:range xsd:string ;
                    <http://purl.org/dc/elements/1.1/creator> "mluisadiez" ;
                    <http://purl.org/dc/elements/1.1/date> "2018-06-16T18:39:21Z"^^xsd:dateTime ;
                    rdfs:comment """Consonants between the stressed vowel and the last consonant.

For example, in the rhyme \"doliente-accidente\" (rhyme between the first and the fourth line) from the sonnet XXXVIII by Fernando de Herrera, the prefinalConsonant is \"n\"."""@en ;
                    rdfs:isDefinedBy "http://postdata.linhd.uned.es/ontology/postdata-prosodicElements"@en ;
                    rdfs:label "prefinal consonants"@en .


###  http://postdata.linhd.uned.es/ontology/postdata-poeticAnalysis#punctuationNumber
:punctuationNumber rdf:type owl:DatatypeProperty ;
                   rdfs:subPropertyOf <http://purl.org/ontology/olo/core#index> ;
                   rdfs:domain :Punctuation ;
                   rdfs:range xsd:positiveInteger ;
                   rdfs:isDefinedBy "http://postdata.linhd.uned.es/ontology/postdata-poeticAnalysis#" ;
                   rdfs:label "The position of a Punctuation in a Punctuation List."@en ,
                              "punctuation number"@en .


###  http://postdata.linhd.uned.es/ontology/postdata-poeticAnalysis#relativeLineNumber
:relativeLineNumber rdf:type owl:DatatypeProperty ;
                    rdfs:domain :Line ;
                    rdfs:range xsd:positiveInteger ;
                    rdfs:comment "Index of a Line (verse) in the Stanza it belongs to."@en ;
                    rdfs:isDefinedBy "http://postdata.linhd.uned.es/ontology/postdata-poeticAnalysis#" ;
                    rdfs:label "relative line number"@en .


###  http://postdata.linhd.uned.es/ontology/postdata-poeticAnalysis#rhymeGrapheme
:rhymeGrapheme rdf:type owl:DatatypeProperty ;
               rdfs:subPropertyOf owl:topDataProperty ;
               rdfs:domain :Rhyme ;
               rdfs:range xsd:string ;
               <http://purl.org/dc/elements/1.1/creator> "mluisadiez" ;
               <http://purl.org/dc/elements/1.1/date> "2018-06-16T18:39:21Z"^^xsd:dateTime ;
               rdfs:comment """Grapheme that represents the rhyming sounds.

If we consider, as an example, the rhyme \"infinito-frito\" in the poem by Quevedo \"A un hombre de gran nariz\", rhyme grapheme is \"ito\"."""@en ;
               rdfs:isDefinedBy "http://postdata.linhd.uned.es/ontology/postdata-prosodicElements"@en ;
               rdfs:label "rhyme grapheme"@en .


###  http://postdata.linhd.uned.es/ontology/postdata-poeticAnalysis#rhymeLabel
:rhymeLabel rdf:type owl:DatatypeProperty ;
            rdfs:subPropertyOf owl:topDataProperty ;
            rdfs:domain :Rhyme ;
            rdfs:range xsd:string ;
            <http://purl.org/dc/elements/1.1/creator> "mluisadiez" ;
            <http://purl.org/dc/elements/1.1/date> "2018-06-16T18:39:21Z"^^xsd:dateTime ;
            rdfs:comment """String used to identify the item at hand (usually, “a”, “b”, “c”, etc.).

For instance, \"A\" is the label used to mark the rhyme between the first and fourth line of the first stanza of the sonnet III from Petrarcha's \"Canzoniere\", namely \"Era il giorno ch’al sol si scoloraro/ [...] /ché i be’ vostr’occhi, donna, mi legaro.\"."""@en ;
            rdfs:isDefinedBy "http://postdata.linhd.uned.es/ontology/postdata-prosodicElements"@en ;
            rdfs:label "rhyme label"@en .


###  http://postdata.linhd.uned.es/ontology/postdata-poeticAnalysis#rhymePhoneme
:rhymePhoneme rdf:type owl:DatatypeProperty ;
              rdfs:subPropertyOf owl:topDataProperty ;
              rdfs:domain :Rhyme ;
              rdfs:range xsd:string ;
              <http://purl.org/dc/elements/1.1/creator> "mluisadiez" ;
              <http://purl.org/dc/elements/1.1/date> "2018-06-16T18:39:21Z"^^xsd:dateTime ;
              rdfs:comment """Phonetic transcription of the rhyming sounds.

For instance, if we consider the rhyme \"strife-life\" from the 55th Psalm by Mary Alcock, rhymePhoneme is /aɪf/."""@en ;
              rdfs:isDefinedBy "http://postdata.linhd.uned.es/ontology/postdata-prosodicElements"@en ;
              rdfs:label "rhyme phoneme"@en .


###  http://postdata.linhd.uned.es/ontology/postdata-poeticAnalysis#rhymeScheme
:rhymeScheme rdf:type owl:DatatypeProperty ;
             rdfs:subPropertyOf owl:topDataProperty ;
             rdfs:domain :StanzaPattern ;
             rdfs:range xsd:string ;
             <http://purl.org/dc/elements/1.1/creator> "mluisadiez" ;
             <http://purl.org/dc/elements/1.1/date> "2018-06-16T18:39:21Z"^^xsd:dateTime ;
             rdfs:comment """A rhyme scheme is the pattern of rhymes at the end of each line of a poem or song. It is usually referred to by using letters to indicate which lines rhyme; lines designated with the same letter all rhyme with each other.

If we consider the first stanza of the sonnet III from Petrarcha's \"Canzoniere\", namely \"Era il giorno ch’al sol si scoloraro / per la pietà del suo factore i rai, / quando i’ fui preso, et non me ne guardai, /ché i be’ vostr’occhi, donna, mi legaro.\". rhymeScheme is: \"ABBA\".""" ;
             rdfs:isDefinedBy "http://postdata.linhd.uned.es/ontology/postdata-prosodicElements"@en ;
             rdfs:label "rhyme scheme"@en .


###  http://postdata.linhd.uned.es/ontology/postdata-poeticAnalysis#rhymeTypeProportion
:rhymeTypeProportion rdf:type owl:DatatypeProperty ;
                     rdfs:subPropertyOf owl:topDataProperty ;
                     rdfs:domain :RedactionPattern ;
                     rdfs:range xsd:string ;
                     <http://purl.org/dc/elements/1.1/creator> "mluisadiez" ;
                     <http://purl.org/dc/elements/1.1/date> "2018-06-16T18:39:21Z"^^xsd:dateTime ;
                     rdfs:comment """Proportion of the feminine/masculine rhymes of the poem.

If we consider, as an example, the sonnet I by Shakespeare, all rhymes are masculine rhymes: \"From fairest creatures we desire increase,/ That thereby beauty's rose might never die, /But as the riper should by time decease, /His tender heir might bear his memory:/ But thou contracted to thine own bright eyes,/ Feed'st thy light's flame with self-substantial fuel,/ Making a famine where abundance lies,/ Thy self thy foe, to thy sweet self too cruel:/ Thou that art now the world's fresh ornament,/ And only herald to the gaudy spring,/ Within thine own bud buriest thy content,/ And, tender churl, mak'st waste in niggarding:/  Pity the world, or else this glutton be,/ To eat the world's due, by the grave and thee.\". Consequently, the rhymeTypeProportion will be \"100% masculine rhymes\".""" ;
                     rdfs:isDefinedBy "http://postdata.linhd.uned.es/ontology/postdata-prosodicElements"@en ;
                     rdfs:label "rhyme type proportion"@en .


###  http://postdata.linhd.uned.es/ontology/postdata-poeticAnalysis#scannedLine
:scannedLine rdf:type owl:DatatypeProperty ;
             rdfs:subPropertyOf owl:topDataProperty ;
             rdfs:domain :LinePattern ;
             rdfs:range xsd:string ;
             <http://purl.org/dc/elements/1.1/creator> "mluisadiez" ;
             <http://purl.org/dc/elements/1.1/date> "2018-06-16T18:39:21Z"^^xsd:dateTime ;
             rdfs:comment """A line metrically analysed, marked up in terms of syllable division and accent.

If we consider, as an example, the line \"From fairest creatures we desire increase,\" from the first sonnet by Shakespeare, scannedLine is \"from FAI.|rest. CREA.|tures. WE.| de.SIRE.| in.CREASE.\""""@en ;
             rdfs:isDefinedBy "http://postdata.linhd.uned.es/ontology/postdata-prosodicElements"@en ;
             rdfs:label "scanned line"@en .


###  http://postdata.linhd.uned.es/ontology/postdata-poeticAnalysis#scheme
:scheme rdf:type owl:DatatypeProperty ;
        rdfs:domain :Foot ;
        rdfs:range xsd:string ;
        rdfs:comment """Abstraction that represents the outline of the unit through a pattern. E.g. “ox(o)“ to represent the type of syllables.

If we consider, as an example, the fist foot of  the line \"From fairest creatures we desire increase,\" from the first sonnet by Shakespeare, namely |From fai|, scheme is \"-+\"."""@en ;
        rdfs:isDefinedBy "http://postdata.linhd.uned.es/ontology/postdata-prosodicElements"@en ;
        rdfs:label "scheme"@en .


###  http://postdata.linhd.uned.es/ontology/postdata-poeticAnalysis#secondHemistich
:secondHemistich rdf:type owl:DatatypeProperty ;
                 rdfs:domain :Line ;
                 rdfs:range xsd:string ;
                 rdfs:comment """This property points to the second division of the line (an instance of Line) that forms the second hemistich.

For example, if we consider the line \"Sous le flambeau d’Amour, des éternelles nuits\" from the sonnet \"Afin que pour jamais une marque demeure\" by Jean Antoine de Baïf, the \"secondHemistich\" is the line \"des éternelles nuits\"."""@en ;
                 rdfs:isDefinedBy "http://postdata.linhd.uned.es/ontology/postdata-poeticAnalysis#" ;
                 rdfs:label "second hemistich"@en .


###  http://postdata.linhd.uned.es/ontology/postdata-poeticAnalysis#stanzaNumber
:stanzaNumber rdf:type owl:DatatypeProperty ;
              rdfs:subPropertyOf <http://purl.org/ontology/olo/core#index> ;
              rdfs:domain :Stanza ;
              rdfs:range xsd:positiveInteger ;
              rdfs:comment """Position of the Stanza inside the Redaction.

For example, if we take the first stanza of the Sonnet XIII by Garcilaso de la Vega, that is \"A Dafne ya los brazos le crecían, / y en luengos ramos vueltos se mostraban; / en verdes hojas vi que se tornaban / los cabellos que'l oro escurecían\", the position of this stanza inside the Redaction is 1."""@en ;
              rdfs:isDefinedBy "http://postdata.linhd.uned.es/ontology/postdata-poeticAnalysis#" ;
              rdfs:label "stanza number"@en .


###  http://postdata.linhd.uned.es/ontology/postdata-poeticAnalysis#stressPosition
:stressPosition rdf:type owl:DatatypeProperty ;
                rdfs:domain :MetricalSyllable ;
                rdfs:range xsd:integer ;
                rdfs:comment """Position of the stressed syllable from the end of the word.ç

If we take, for instance, the word \"esperanza\", stressPosition is 2, because stress in on the second syllable of the word."""@en ;
                rdfs:isDefinedBy "http://postdata.linhd.uned.es/ontology/postdata-prosodicElements"@en ;
                rdfs:label "stress position"@en .


###  http://postdata.linhd.uned.es/ontology/postdata-poeticAnalysis#syllabicMetricalScheme
:syllabicMetricalScheme rdf:type owl:DatatypeProperty ;
                        rdfs:subPropertyOf owl:topDataProperty ;
                        rdfs:domain :LinePattern ;
                        rdfs:range xsd:string ;
                        <http://purl.org/dc/elements/1.1/creator> "mluisadiez" ;
                        rdfs:comment """Metrical scheme according to the number of syllables.

For instance, if we consider the line \"From fairest creatures we desire increase,\" from the first sonnet by Shakespeare and analyse them only in terms of number of syllables, syllabicMetricalScheme is: 10 syllables."""@en ;
                        rdfs:isDefinedBy "http://postdata.linhd.uned.es/ontology/postdata-prosodicElements"@en ;
                        rdfs:label "syllabic metrical scheme"@en .


###  http://postdata.linhd.uned.es/ontology/postdata-poeticAnalysis#symbolExplanation
:symbolExplanation rdf:type owl:DatatypeProperty ;
                   rdfs:domain :Symbol ;
                   rdfs:range xsd:string ;
                   rdfs:comment """Meaning of the symbol used in a metrical pattern.

In the metrical pattern description of the line he line \"From fairest creatures we desire increase,\" from the first sonnet by Shakespeare, that is -+-+-+-+-+, + indicates stressed syllables and - unstressed syllables."""@en ;
                   rdfs:isDefinedBy "http://postdata.linhd.uned.es/ontology/postdata-prosodicElements"@en ;
                   rdfs:label "symbol explanation"@en .


###  http://postdata.linhd.uned.es/ontology/postdata-poeticAnalysis#translation
:translation rdf:type owl:DatatypeProperty ;
             rdfs:subPropertyOf owl:topDataProperty ;
             rdfs:domain :Word ;
             rdfs:range xsd:string ;
             rdfs:comment """Translation of a Word

For instance, if we take the Spanish word \"viaje\" the English translation would be \"journey\"."""@en ;
             rdfs:isDefinedBy "http://postdata.linhd.uned.es/ontology/postdata-poeticAnalysis#" ;
             rdfs:label "translation"@en .


###  http://postdata.linhd.uned.es/ontology/postdata-poeticAnalysis#vowelTypeScheme
:vowelTypeScheme rdf:type owl:DatatypeProperty ;
                 rdfs:subPropertyOf owl:topDataProperty ;
                 rdfs:domain :LinePattern ;
                 rdfs:range xsd:string ;
                 <http://purl.org/dc/elements/1.1/creator> "mluisadiez" ;
                 <http://purl.org/dc/elements/1.1/date> "2018-06-16T18:39:21Z"^^xsd:dateTime ;
                 rdfs:comment """Linguistic properties of the vowels of the line.

If we consider, for instance, the line \"Morir soñando, sí, mas si se sueña\" from the poem \"Morir soñando\" by Unamuno, vowelTypeScheme is: monophthong back close-mid, monophthong front close, monophthong back close-mid, monophthong front open, monophthong back close-mid, monophthong front close, monophthong front open, monophthong front close, monophthong front close-mid, diphthong labio-velar approximant + front close-mid vowel, monophthong front open."""@en ;
                 rdfs:isDefinedBy "http://postdata.linhd.uned.es/ontology/postdata-prosodicElements"@en ;
                 rdfs:label "vowel type scheme"@en .


###  http://postdata.linhd.uned.es/ontology/postdata-poeticAnalysis#weight
:weight rdf:type owl:DatatypeProperty ;
        rdfs:subPropertyOf owl:topDataProperty ;
        rdfs:domain :MetricalSyllable ;
        rdfs:range xsd:string ;
        rdfs:comment """Pattern according to the number and/or duration of segments in the syllabic rime, that is, the nucleus and coda.

For example, in Latin the first syllable of the word 'Arma' (i.e. 'ar') is heavy because it contains a short vowel followed by a consonant. In English the word \"cat\" constitutes a heavy syllable."""@en ;
        rdfs:isDefinedBy "http://postdata.linhd.uned.es/ontology/postdata-poeticAnalysis#" ;
        rdfs:label "weight"@en .


###  http://postdata.linhd.uned.es/ontology/postdata-poeticAnalysis#wordNumber
:wordNumber rdf:type owl:DatatypeProperty ;
            rdfs:subPropertyOf <http://purl.org/ontology/olo/core#index> ;
            rdfs:domain :Word ;
            rdfs:range xsd:positiveInteger ;
            rdfs:comment """Position of the Word within the Line to which it belongs.

For example, if we take the last line of the poem \"Canary\" by Rita Dove, the word \"mystery\" has the position 8 in the line."""@en ;
            rdfs:isDefinedBy "http://postdata.linhd.uned.es/ontology/postdata-poeticAnalysis#" ;
            rdfs:label "word number"@en .


###  http://postdata.linhd.uned.es/ontology/postdata-poeticAnalysis#wordSense
:wordSense rdf:type owl:DatatypeProperty ;
           rdfs:subPropertyOf owl:topDataProperty ;
           rdfs:domain :Word ;
           rdfs:range xsd:string ;
           rdfs:comment """One of the meanings of a word or phrase.

For example, in the poem \"Suspiro y pruebo con la voz doliente\" by Fernando de Herrera, the sense of the word “suspiro” is, according to the Diccionario de la Real Academia Española (the Dictionary of the Royal Spanish Academy), “Dar suspiros” (sigh)."""@en ;
           rdfs:isDefinedBy "http://postdata.linhd.uned.es/ontology/postdata-poeticAnalysis#" ;
           rdfs:label "word sense"@en .


###  http://purl.org/ontology/olo/core#index
<http://purl.org/ontology/olo/core#index> rdf:type owl:DatatypeProperty .


###  http://purl.org/ontology/olo/core#length
<http://purl.org/ontology/olo/core#length> rdf:type owl:DatatypeProperty .


###  http://www.w3.org/2002/07/owl#topDataProperty
owl:topDataProperty rdfs:subPropertyOf owl:topDataProperty .


#################################################################
#    Classes
#################################################################

###  http://postdata.linhd.uned.es/ontology/postdata-core#Agent
<http://postdata.linhd.uned.es/ontology/postdata-core#Agent> rdf:type owl:Class .


###  http://postdata.linhd.uned.es/ontology/postdata-core#AgentRole
<http://postdata.linhd.uned.es/ontology/postdata-core#AgentRole> rdf:type owl:Class ;
                                                                 rdfs:label "Agent Role"@en .


###  http://postdata.linhd.uned.es/ontology/postdata-core#Event
<http://postdata.linhd.uned.es/ontology/postdata-core#Event> rdf:type owl:Class .


###  http://postdata.linhd.uned.es/ontology/postdata-core#Excerpt
<http://postdata.linhd.uned.es/ontology/postdata-core#Excerpt> rdf:type owl:Class ;
                                                               rdfs:subClassOf <http://postdata.linhd.uned.es/ontology/postdata-core#LinguisticObject> .


###  http://postdata.linhd.uned.es/ontology/postdata-core#LinguisticObject
<http://postdata.linhd.uned.es/ontology/postdata-core#LinguisticObject> rdf:type owl:Class ;
                                                                        rdfs:label "Linguistic Object"@en .


###  http://postdata.linhd.uned.es/ontology/postdata-core#Place
<http://postdata.linhd.uned.es/ontology/postdata-core#Place> rdf:type owl:Class .


###  http://postdata.linhd.uned.es/ontology/postdata-core#Redaction
<http://postdata.linhd.uned.es/ontology/postdata-core#Redaction> rdf:type owl:Class ;
                                                                 rdfs:subClassOf [ rdf:type owl:Restriction ;
                                                                                   owl:onProperty :firstLine ;
                                                                                   owl:maxQualifiedCardinality "1"^^xsd:nonNegativeInteger ;
                                                                                   owl:onClass :Line
                                                                                 ] ,
                                                                                 [ rdf:type owl:Restriction ;
                                                                                   owl:onProperty :rhymeMatchingType ;
                                                                                   owl:maxQualifiedCardinality "1"^^xsd:nonNegativeInteger ;
                                                                                   owl:onClass [ owl:intersectionOf ( <http://www.w3.org/2004/02/skos/core#Concept>
                                                                                                                      [ rdf:type owl:Restriction ;
                                                                                                                        owl:onProperty <http://www.w3.org/2004/02/skos/core#inScheme> ;
                                                                                                                        owl:hasValue <http://postdata.linhd.uned.es/kos/rhymeMatching-type>
                                                                                                                      ]
                                                                                                                    ) ;
                                                                                                 rdf:type owl:Class
                                                                                               ]
                                                                                 ] .


###  http://postdata.linhd.uned.es/ontology/postdata-poeticAnalysis#Acrostic
:Acrostic rdf:type owl:Class ;
          rdfs:subClassOf :LiteraryDevice ;
          rdfs:label "Acrostic"@en .


###  http://postdata.linhd.uned.es/ontology/postdata-poeticAnalysis#AnalyticalUnit
:AnalyticalUnit rdf:type owl:Class ;
                rdfs:label "Analytical Unit"@en .


###  http://postdata.linhd.uned.es/ontology/postdata-poeticAnalysis#BasicAnalyticalUnit
:BasicAnalyticalUnit rdf:type owl:Class ;
                     rdfs:subClassOf :AnalyticalUnit ;
                     rdfs:label "Basic Analytical Unit"@en .


###  http://postdata.linhd.uned.es/ontology/postdata-poeticAnalysis#Enjambment
:Enjambment rdf:type owl:Class ;
            rdfs:subClassOf :LiteraryDevice .


###  http://postdata.linhd.uned.es/ontology/postdata-poeticAnalysis#FigureOfSpeech
:FigureOfSpeech rdf:type owl:Class ;
                rdfs:subClassOf :LiteraryDevice ;
                rdfs:comment "A word or phrase used in a non-literal sense for rhetorical or vivid effect"@en ;
                rdfs:isDefinedBy "http://postdata.linhd.uned.es/ontology/postdata-poeticAnalysis#"@en ;
                rdfs:label "Figure Of Speech"@en .


###  http://postdata.linhd.uned.es/ontology/postdata-poeticAnalysis#Foot
:Foot rdf:type owl:Class ;
      rdfs:subClassOf :AnalyticalUnit ,
                      <http://purl.org/ontology/olo/core#Slot> ,
                      [ rdf:type owl:Restriction ;
                        owl:onProperty :clausula ;
                        owl:maxQualifiedCardinality "1"^^xsd:nonNegativeInteger ;
                        owl:onClass [ owl:intersectionOf ( <http://www.w3.org/2004/02/skos/core#Concept>
                                                           [ rdf:type owl:Restriction ;
                                                             owl:onProperty <http://www.w3.org/2004/02/skos/core#inScheme> ;
                                                             owl:hasValue <http://postdata.linhd.uned.es/kos/clausula>
                                                           ]
                                                         ) ;
                                      rdf:type owl:Class
                                    ]
                      ] ;
      rdfs:comment "A unit of poetic meter consisting of stressed and unstressed syllables or long and short syllables in any of various set combinations."@en ;
      rdfs:label "Foot"@en ;
      rdfs:seeAlso "https://ahdictionary.com/word/search.html?q=foot" ,
                   "https://www.poetryfoundation.org/learn/glossary-terms/foot" .


###  http://postdata.linhd.uned.es/ontology/postdata-poeticAnalysis#FootList
:FootList rdf:type owl:Class ;
          rdfs:subClassOf <http://purl.org/ontology/olo/core#OrderedList> ;
          rdfs:label "Foot List"@en .


###  http://postdata.linhd.uned.es/ontology/postdata-poeticAnalysis#GrammaticalSyllable
:GrammaticalSyllable rdf:type owl:Class ;
                     rdfs:subClassOf :AnalyticalUnit ,
                                     <http://purl.org/ontology/olo/core#Slot> ,
                                     [ rdf:type owl:Restriction ;
                                       owl:onProperty :weight ;
                                       owl:someValuesFrom xsd:string
                                     ] ,
                                     [ rdf:type owl:Restriction ;
                                       owl:onProperty :content ;
                                       owl:qualifiedCardinality "1"^^xsd:nonNegativeInteger ;
                                       owl:onDataRange xsd:string
                                     ] ,
                                     [ rdf:type owl:Restriction ;
                                       owl:onProperty :absoluteLineNumber ;
                                       owl:maxQualifiedCardinality "1"^^xsd:nonNegativeInteger ;
                                       owl:onDataRange xsd:string
                                     ] ,
                                     [ rdf:type owl:Restriction ;
                                       owl:onProperty :isRefrain ;
                                       owl:maxQualifiedCardinality "1"^^xsd:nonNegativeInteger ;
                                       owl:onDataRange xsd:boolean
                                     ] ;
                     rdfs:comment """A single unit of speech sound as written or spoken; specifically, a vowel preceded by zero to three consonants (“awl,” “bring,” “strand”), and followed by zero to four consonants (“too,” “brag,” “gloss,” “stings,” “sixths”).

This class corresponds to the definition of grammatical syllables that in some literary traditions like French poetry and Sanskrit determines the metre of basic rythmic structure of a Line.

Eg.: The word ignite is composed of two syllables: ig and nite."""@en ;
                     rdfs:isDefinedBy "http://postdata.linhd.uned.es/ontology/postdata-poeticAnalysis#" ;
                     rdfs:label "Grammatical Syllable"@en ;
                     rdfs:seeAlso "https://en.wikipedia.org/wiki/Syllable" ,
                                  "https://www.poetryfoundation.org/learn/glossary-terms/syllable" .


###  http://postdata.linhd.uned.es/ontology/postdata-poeticAnalysis#GrammaticalSyllableList
:GrammaticalSyllableList rdf:type owl:Class ;
                         rdfs:subClassOf <http://purl.org/ontology/olo/core#OrderedList> ;
                         rdfs:label "Grammatical Syllable List"@en .


###  http://postdata.linhd.uned.es/ontology/postdata-poeticAnalysis#Intertextuality
:Intertextuality rdf:type owl:Class ;
                 rdfs:subClassOf :LiteraryDevice ;
                 <http://purl.org/dc/elements/1.1/date> "2018-06-16T18:37:24Z"^^xsd:dateTime ;
                 rdfs:comment "Shared textual materials between two or more contemporary texts; Text from which information or ideas are derived for the composition of the Opus/Redaction;Text that took information or ideas from the Opus/Redaction" ;
                 rdfs:label "Intertextuality"@en .


###  http://postdata.linhd.uned.es/ontology/postdata-poeticAnalysis#Line
:Line rdf:type owl:Class ;
      rdfs:subClassOf :StructuralUnit ,
                      <http://purl.org/ontology/olo/core#Slot> ,
                      owl:Thing ,
                      [ rdf:type owl:Restriction ;
                        owl:onProperty :isPatternOf ;
                        owl:maxQualifiedCardinality "1"^^xsd:nonNegativeInteger ;
                        owl:onClass :LinePattern
                      ] ,
                      [ rdf:type owl:Restriction ;
                        owl:onProperty :absoluteLineNumber ;
                        owl:maxQualifiedCardinality "1"^^xsd:nonNegativeInteger ;
                        owl:onDataRange xsd:string
                      ] ,
                      [ rdf:type owl:Restriction ;
                        owl:onProperty :content ;
                        owl:maxQualifiedCardinality "1"^^xsd:nonNegativeInteger ;
                        owl:onDataRange xsd:string
                      ] ,
                      [ rdf:type owl:Restriction ;
                        owl:onProperty :isRefrain ;
                        owl:maxQualifiedCardinality "1"^^xsd:nonNegativeInteger ;
                        owl:onDataRange xsd:boolean
                      ] ;
      rdfs:comment """A line is a subdivision of a poem, specifically a group of words arranged into a row that ends with a line break. Although the word for a single poetic line is verse, that term now tends to be used to signify poetic form more generally. A line break is the termination of the line of a poem and the beginning of a new line.

Eg.: “As armas e os barões assinalados” - from Os Lusíadas"""@en ;
      rdfs:isDefinedBy "http://postdata.linhd.uned.es/ontology/postdata-poeticAnalysis#" ;
      rdfs:label "Line"@en ;
      rdfs:seeAlso "https://en.wikipedia.org/wiki/Line_(poetry)" ,
                   "https://poetryarchive.org/glossary/line/" .


###  http://postdata.linhd.uned.es/ontology/postdata-poeticAnalysis#LineList
:LineList rdf:type owl:Class ;
          rdfs:subClassOf <http://purl.org/ontology/olo/core#OrderedList> ;
          rdfs:comment "A Line List is an ordered list of slots of type Line that is used to represent the contents of a Redaction. Any Redaction has a Line List composed by a minimum of one Line."@en ;
          rdfs:isDefinedBy "http://postdata.linhd.uned.es/ontology/postdata-poeticAnalysis#" ;
          rdfs:label "Line List"@en .


###  http://postdata.linhd.uned.es/ontology/postdata-poeticAnalysis#LinePattern
:LinePattern rdf:type owl:Class ;
             rdfs:subClassOf :Pattern ,
                             [ rdf:type owl:Restriction ;
                               owl:onProperty :feetType ;
                               owl:maxQualifiedCardinality "1"^^xsd:nonNegativeInteger ;
                               owl:onClass [ owl:intersectionOf ( <http://www.w3.org/2004/02/skos/core#Concept>
                                                                  [ rdf:type owl:Restriction ;
                                                                    owl:onProperty <http://www.w3.org/2004/02/skos/core#inScheme> ;
                                                                    owl:hasValue <http://postdata.linhd.uned.es/kos/feet-type>
                                                                  ]
                                                                ) ;
                                             rdf:type owl:Class
                                           ]
                             ] ,
                             [ rdf:type owl:Restriction ;
                               owl:onProperty :accentedVowels ;
                               owl:maxQualifiedCardinality "1"^^xsd:nonNegativeInteger ;
                               owl:onDataRange xsd:string
                             ] ,
                             [ rdf:type owl:Restriction ;
                               owl:onProperty :altPatterningMetricalScheme ;
                               owl:maxQualifiedCardinality "1"^^xsd:nonNegativeInteger ;
                               owl:onDataRange xsd:string
                             ] ,
                             [ rdf:type owl:Restriction ;
                               owl:onProperty :altSyllabicMetricalScheme ;
                               owl:maxQualifiedCardinality "1"^^xsd:nonNegativeInteger ;
                               owl:onDataRange xsd:string
                             ] ,
                             [ rdf:type owl:Restriction ;
                               owl:onProperty :grammaticalStressPattern ;
                               owl:maxQualifiedCardinality "1"^^xsd:nonNegativeInteger ;
                               owl:onDataRange xsd:string
                             ] ,
                             [ rdf:type owl:Restriction ;
                               owl:onProperty :hasAnacrusis ;
                               owl:maxQualifiedCardinality "1"^^xsd:nonNegativeInteger ;
                               owl:onDataRange xsd:boolean
                             ] ,
                             [ rdf:type owl:Restriction ;
                               owl:onProperty :hasCaesura ;
                               owl:maxQualifiedCardinality "1"^^xsd:nonNegativeInteger ;
                               owl:onDataRange xsd:boolean
                             ] ,
                             [ rdf:type owl:Restriction ;
                               owl:onProperty :metricalNotes ;
                               owl:maxQualifiedCardinality "1"^^xsd:nonNegativeInteger ;
                               owl:onDataRange xsd:string
                             ] ,
                             [ rdf:type owl:Restriction ;
                               owl:onProperty :patterningMetricalScheme ;
                               owl:maxQualifiedCardinality "1"^^xsd:nonNegativeInteger ;
                               owl:onDataRange xsd:string
                             ] ,
                             [ rdf:type owl:Restriction ;
                               owl:onProperty :syllabicMetricalScheme ;
                               owl:maxQualifiedCardinality "1"^^xsd:nonNegativeInteger ;
                               owl:onDataRange xsd:string
                             ] ;
             <http://purl.org/dc/elements/1.1/date> "2018-06-16T18:37:24Z"^^xsd:dateTime ;
             rdfs:comment """The prosodic analysis using a Line as the unit of reference
Eg.: The number of syllables of the Line"""@en ;
             rdfs:label "Line Pattern"@en .


###  http://postdata.linhd.uned.es/ontology/postdata-poeticAnalysis#LiteraryDevice
:LiteraryDevice rdf:type owl:Class ;
                rdfs:label "Literary Device"@en .


###  http://postdata.linhd.uned.es/ontology/postdata-poeticAnalysis#Metaplasm
:Metaplasm rdf:type owl:Class ;
           rdfs:subClassOf :LiteraryDevice ;
           rdfs:comment """A figure of transformation or metaplasm is a figure of diction that consists of altering the writing or pronunciation of words without altering their meaning.
Some examples are dieresis, syneresis, sinalefa or hiatus."""@en ;
           rdfs:isDefinedBy "http://postdata.linhd.uned.es/ontology/postdata-prosodicElements"@en ;
           rdfs:label "Metaplasm"@en .


###  http://postdata.linhd.uned.es/ontology/postdata-poeticAnalysis#MetricalEncoding
:MetricalEncoding rdf:type owl:Class ;
                  rdfs:subClassOf [ rdf:type owl:Restriction ;
                                    owl:onProperty :metricalNotes ;
                                    owl:maxQualifiedCardinality "1"^^xsd:nonNegativeInteger ;
                                    owl:onDataRange xsd:string
                                  ] ;
                  <http://purl.org/dc/elements/1.1/creator> "mluisadiez" ;
                  <http://purl.org/dc/elements/1.1/date> "2018-06-16T18:37:24Z"^^xsd:dateTime ;
                  rdfs:comment """The notation employed to represent a metrical pattern.
Eg.: The definition of the plus sign to encode strong positions."""@en ;
                  rdfs:isDefinedBy "http://postdata.linhd.uned.es/ontology/postdata-prosodicElements"@en ;
                  rdfs:label "Metrical Encoding"@en .


###  http://postdata.linhd.uned.es/ontology/postdata-poeticAnalysis#MetricalSyllable
:MetricalSyllable rdf:type owl:Class ;
                  rdfs:subClassOf :BasicAnalyticalUnit ,
                                  <http://purl.org/ontology/olo/core#Slot> ;
                  rdfs:comment "Metric syllable built by applying metaplasms to syllables."@en ;
                  rdfs:isDefinedBy "http://postdata.linhd.uned.es/ontology/postdata-prosodicElements"@en ;
                  rdfs:label "Metrical Syllable"@en .


###  http://postdata.linhd.uned.es/ontology/postdata-poeticAnalysis#MetricalSyllableList
:MetricalSyllableList rdf:type owl:Class ;
                      rdfs:subClassOf <http://purl.org/ontology/olo/core#OrderedList> ;
                      rdfs:label "Metrical Syllable List"@en .


###  http://postdata.linhd.uned.es/ontology/postdata-poeticAnalysis#Mora
:Mora rdf:type owl:Class ;
      rdfs:subClassOf :BasicAnalyticalUnit ,
                      <http://purl.org/ontology/olo/core#Slot> ;
      rdfs:label "Mora"@en .


###  http://postdata.linhd.uned.es/ontology/postdata-poeticAnalysis#MoraList
:MoraList rdf:type owl:Class ;
          rdfs:subClassOf <http://purl.org/ontology/olo/core#OrderedList> ;
          rdfs:label "Mora List"@en .


###  http://postdata.linhd.uned.es/ontology/postdata-poeticAnalysis#Pattern
:Pattern rdf:type owl:Class .


###  http://postdata.linhd.uned.es/ontology/postdata-poeticAnalysis#Punctuation
:Punctuation rdf:type owl:Class ;
             rdfs:subClassOf :StructuralUnit ,
                             <http://purl.org/ontology/olo/core#Slot> ,
                             [ rdf:type owl:Restriction ;
                               owl:onProperty :content ;
                               owl:qualifiedCardinality "1"^^xsd:nonNegativeInteger ;
                               owl:onDataRange xsd:string
                             ] ;
             rdfs:comment """Specific markings, signs and symbols that are used in and around sentences to give them structure and to allow for correct understanding and comprehension.

Eg.: the colon \":\""""@en ;
             rdfs:isDefinedBy "http://postdata.linhd.uned.es/ontology/postdata-poeticAnalysis#" ;
             rdfs:label "Punctuation"@en ;
             rdfs:seeAlso "https://www.thefreedictionary.com/English-Punctuation.htm" .


###  http://postdata.linhd.uned.es/ontology/postdata-poeticAnalysis#PunctuationList
:PunctuationList rdf:type owl:Class ;
                 rdfs:subClassOf <http://purl.org/ontology/olo/core#OrderedList> ;
                 rdfs:comment "This class represents an ordered list of punctuations that may appear in a Line."@en ;
                 rdfs:isDefinedBy "http://postdata.linhd.uned.es/ontology/postdata-poeticAnalysis#" ;
                 rdfs:label "Punctuation List"@en .


###  http://postdata.linhd.uned.es/ontology/postdata-poeticAnalysis#RedactionPattern
:RedactionPattern rdf:type owl:Class ;
                  rdfs:subClassOf :Pattern ,
                                  [ rdf:type owl:Restriction ;
                                    owl:onProperty :metricalType ;
                                    owl:maxQualifiedCardinality "1"^^xsd:nonNegativeInteger ;
                                    owl:onClass [ owl:intersectionOf ( <http://www.w3.org/2004/02/skos/core#Concept>
                                                                       [ rdf:type owl:Restriction ;
                                                                         owl:onProperty <http://www.w3.org/2004/02/skos/core#inScheme> ;
                                                                         owl:hasValue <http://postdata.linhd.uned.es/kos/metrical-type>
                                                                       ]
                                                                     ) ;
                                                  rdf:type owl:Class
                                                ]
                                  ] ,
                                  [ rdf:type owl:Restriction ;
                                    owl:onProperty :rhymeMatchingType ;
                                    owl:maxQualifiedCardinality "1"^^xsd:nonNegativeInteger ;
                                    owl:onClass [ owl:intersectionOf ( <http://www.w3.org/2004/02/skos/core#Concept>
                                                                       [ rdf:type owl:Restriction ;
                                                                         owl:onProperty <http://www.w3.org/2004/02/skos/core#inScheme> ;
                                                                         owl:hasValue <http://postdata.linhd.uned.es/kos/rhymeMatching-type>
                                                                       ]
                                                                     ) ;
                                                  rdf:type owl:Class
                                                ]
                                  ] ,
                                  [ rdf:type owl:Restriction ;
                                    owl:onProperty :altPatterningMetricalScheme ;
                                    owl:maxQualifiedCardinality "1"^^xsd:nonNegativeInteger ;
                                    owl:onDataRange xsd:string
                                  ] ,
                                  [ rdf:type owl:Restriction ;
                                    owl:onProperty :altRhymeScheme ;
                                    owl:maxQualifiedCardinality "1"^^xsd:nonNegativeInteger ;
                                    owl:onDataRange xsd:string
                                  ] ,
                                  [ rdf:type owl:Restriction ;
                                    owl:onProperty :altSyllabicMetricalScheme ;
                                    owl:maxQualifiedCardinality "1"^^xsd:nonNegativeInteger ;
                                    owl:onDataRange xsd:string
                                  ] ,
                                  [ rdf:type owl:Restriction ;
                                    owl:onProperty :grammaticalStressPattern ;
                                    owl:maxQualifiedCardinality "1"^^xsd:nonNegativeInteger ;
                                    owl:onDataRange xsd:string
                                  ] ,
                                  [ rdf:type owl:Restriction ;
                                    owl:onProperty :hasAnacrusis ;
                                    owl:maxQualifiedCardinality "1"^^xsd:nonNegativeInteger ;
                                    owl:onDataRange xsd:boolean
                                  ] ,
                                  [ rdf:type owl:Restriction ;
                                    owl:onProperty :hasCaesura ;
                                    owl:maxQualifiedCardinality "1"^^xsd:nonNegativeInteger ;
                                    owl:onDataRange xsd:boolean
                                  ] ,
                                  [ rdf:type owl:Restriction ;
                                    owl:onProperty :metricalNotes ;
                                    owl:maxQualifiedCardinality "1"^^xsd:nonNegativeInteger ;
                                    owl:onDataRange xsd:string
                                  ] ,
                                  [ rdf:type owl:Restriction ;
                                    owl:onProperty :patterningMetricalScheme ;
                                    owl:maxQualifiedCardinality "1"^^xsd:nonNegativeInteger ;
                                    owl:onDataRange xsd:string
                                  ] ,
                                  [ rdf:type owl:Restriction ;
                                    owl:onProperty :rhymeScheme ;
                                    owl:maxQualifiedCardinality "1"^^xsd:nonNegativeInteger ;
                                    owl:onDataRange xsd:string
                                  ] ,
                                  [ rdf:type owl:Restriction ;
                                    owl:onProperty :syllabicMetricalScheme ;
                                    owl:maxQualifiedCardinality "1"^^xsd:nonNegativeInteger ;
                                    owl:onDataRange xsd:string
                                  ] ;
                  <http://purl.org/dc/elements/1.1/creator> "mluisadiez" ;
                  <http://purl.org/dc/elements/1.1/date> "2018-06-16T18:37:24Z"^^xsd:dateTime ;
                  rdfs:comment """The prosodic analysis using a Redaction as the unit of reference
Eg.: The complete distribution of accented syllables of a work"""@en ;
                  rdfs:label "Redaction Pattern"@en .


###  http://postdata.linhd.uned.es/ontology/postdata-poeticAnalysis#Rhyme
:Rhyme rdf:type owl:Class ;
       <http://purl.org/dc/elements/1.1/creator> "mluisadiez"@en ;
       rdfs:comment "Repetition of similar sounding words occurring at the end of lines in poems or songs"@en ;
       rdfs:label "Rhyme"@en .


###  http://postdata.linhd.uned.es/ontology/postdata-poeticAnalysis#Scansion
:Scansion rdf:type owl:Class ;
          rdfs:comment "Event scansion is performed by some agent (person or computer software) taking a redaction as input and generates a set of lists and patterns for the elements of analysis considered."@en .


###  http://postdata.linhd.uned.es/ontology/postdata-poeticAnalysis#ScansionProcess
:ScansionProcess rdf:type owl:Class ;
                 rdfs:subClassOf <http://postdata.linhd.uned.es/ontology/postdata-core#Event> ;
                 rdfs:label "Scansion Process"@en .


###  http://postdata.linhd.uned.es/ontology/postdata-poeticAnalysis#Scheme
:Scheme rdf:type owl:Class ;
        rdfs:subClassOf :FigureOfSpeech ;
        rdfs:label "Scheme"@en .


###  http://postdata.linhd.uned.es/ontology/postdata-poeticAnalysis#Stanza
:Stanza rdf:type owl:Class ;
        rdfs:subClassOf :StructuralUnit ,
                        <http://purl.org/ontology/olo/core#Slot> ,
                        owl:Thing ,
                        [ rdf:type owl:Restriction ;
                          owl:onProperty :firstLine ;
                          owl:qualifiedCardinality "1"^^xsd:nonNegativeInteger ;
                          owl:onClass :Line
                        ] ,
                        [ rdf:type owl:Restriction ;
                          owl:onProperty :lastLine ;
                          owl:qualifiedCardinality "1"^^xsd:nonNegativeInteger ;
                          owl:onClass :Line
                        ] ,
                        [ rdf:type owl:Restriction ;
                          owl:onProperty :isPatternOf ;
                          owl:maxQualifiedCardinality "1"^^xsd:nonNegativeInteger ;
                          owl:onClass :Pattern
                        ] ,
                        [ rdf:type owl:Restriction ;
                          owl:onProperty :rhymeMatchingType ;
                          owl:maxQualifiedCardinality "1"^^xsd:nonNegativeInteger ;
                          owl:onClass [ owl:intersectionOf ( <http://www.w3.org/2004/02/skos/core#Concept>
                                                             [ rdf:type owl:Restriction ;
                                                               owl:onProperty <http://www.w3.org/2004/02/skos/core#inScheme> ;
                                                               owl:hasValue <http://postdata.linhd.uned.es/kos/rhymeMatching-type>
                                                             ]
                                                           ) ;
                                        rdf:type owl:Class
                                      ]
                        ] ,
                        [ rdf:type owl:Restriction ;
                          owl:onProperty :content ;
                          owl:maxQualifiedCardinality "1"^^xsd:nonNegativeInteger ;
                          owl:onDataRange xsd:string
                        ] ,
                        [ rdf:type owl:Restriction ;
                          owl:onProperty :paraphrasis ;
                          owl:maxQualifiedCardinality "1"^^xsd:nonNegativeInteger ;
                          owl:onDataRange xsd:string
                        ] ;
        rdfs:comment """A grouping of lines separated from others in a poem. In modern free verse, the stanza, like a prose paragraph, can be used to mark a shift in mood, time, or thought.

Eg.: As armas e os barões assinalados,
Que da ocidental praia Lusitana,
Por mares nunca de antes navegados,
Passaram ainda além da Taprobana,
Em perigos e guerras esforçados,
Mais do que prometia a força humana,
E entre gente remota edificaram
Novo Reino, que tanto sublimaram;"""@en ;
        rdfs:isDefinedBy "http://postdata.linhd.uned.es/ontology/postdata-poeticAnalysis#"@en ;
        rdfs:label "Stanza"@en ;
        rdfs:seeAlso "https://www.poetryfoundation.org/learn/glossary-terms/stanza" .


###  http://postdata.linhd.uned.es/ontology/postdata-poeticAnalysis#StanzaList
:StanzaList rdf:type owl:Class ;
            rdfs:subClassOf <http://purl.org/ontology/olo/core#OrderedList> ;
            rdfs:comment "A Stanza List is an ordered list of slots of type Stanza that is used to represent the contents of a Redaction. Any Redaction has a Stanza List composed by a minimum of one Stanza."@en ;
            rdfs:isDefinedBy "http://postdata.linhd.uned.es/ontology/postdata-poeticAnalysis#" ;
            rdfs:label "Stanza List"@en .


###  http://postdata.linhd.uned.es/ontology/postdata-poeticAnalysis#StanzaPattern
:StanzaPattern rdf:type owl:Class ;
               rdfs:subClassOf :Pattern ,
                               [ rdf:type owl:Restriction ;
                                 owl:onProperty :clausulaSchemeType ;
                                 owl:maxQualifiedCardinality "1"^^xsd:nonNegativeInteger ;
                                 owl:onClass [ owl:intersectionOf ( <http://www.w3.org/2004/02/skos/core#Concept>
                                                                    [ rdf:type owl:Restriction ;
                                                                      owl:onProperty <http://www.w3.org/2004/02/skos/core#inScheme> ;
                                                                      owl:hasValue <http://postdata.linhd.uned.es/kos/clausulaScheme-type>
                                                                    ]
                                                                  ) ;
                                               rdf:type owl:Class
                                             ]
                               ] ,
                               [ rdf:type owl:Restriction ;
                                 owl:onProperty :feetType ;
                                 owl:maxQualifiedCardinality "1"^^xsd:nonNegativeInteger ;
                                 owl:onClass [ owl:intersectionOf ( <http://www.w3.org/2004/02/skos/core#Concept>
                                                                    [ rdf:type owl:Restriction ;
                                                                      owl:onProperty <http://www.w3.org/2004/02/skos/core#inScheme> ;
                                                                      owl:hasValue <http://postdata.linhd.uned.es/kos/feet-type>
                                                                    ]
                                                                  ) ;
                                               rdf:type owl:Class
                                             ]
                               ] ,
                               [ rdf:type owl:Restriction ;
                                 owl:onProperty :metricalType ;
                                 owl:maxQualifiedCardinality "1"^^xsd:nonNegativeInteger ;
                                 owl:onClass [ owl:intersectionOf ( <http://www.w3.org/2004/02/skos/core#Concept>
                                                                    [ rdf:type owl:Restriction ;
                                                                      owl:onProperty <http://www.w3.org/2004/02/skos/core#inScheme> ;
                                                                      owl:hasValue <http://postdata.linhd.uned.es/kos/metrical-type>
                                                                    ]
                                                                  ) ;
                                               rdf:type owl:Class
                                             ]
                               ] ,
                               [ rdf:type owl:Restriction ;
                                 owl:onProperty :rhymeMatchingType ;
                                 owl:maxQualifiedCardinality "1"^^xsd:nonNegativeInteger ;
                                 owl:onClass [ owl:intersectionOf ( <http://www.w3.org/2004/02/skos/core#Concept>
                                                                    [ rdf:type owl:Restriction ;
                                                                      owl:onProperty <http://www.w3.org/2004/02/skos/core#inScheme> ;
                                                                      owl:hasValue <http://postdata.linhd.uned.es/kos/rhymeMatching-type>
                                                                    ]
                                                                  ) ;
                                               rdf:type owl:Class
                                             ]
                               ] ,
                               [ rdf:type owl:Restriction ;
                                 owl:onProperty :altPatterningMetricalScheme ;
                                 owl:maxQualifiedCardinality "1"^^xsd:nonNegativeInteger ;
                                 owl:onDataRange xsd:string
                               ] ,
                               [ rdf:type owl:Restriction ;
                                 owl:onProperty :altRhymeScheme ;
                                 owl:maxQualifiedCardinality "1"^^xsd:nonNegativeInteger ;
                                 owl:onDataRange xsd:string
                               ] ,
                               [ rdf:type owl:Restriction ;
                                 owl:onProperty :altSyllabicMetricalScheme ;
                                 owl:maxQualifiedCardinality "1"^^xsd:nonNegativeInteger ;
                                 owl:onDataRange xsd:string
                               ] ,
                               [ rdf:type owl:Restriction ;
                                 owl:onProperty :hasCaesura ;
                                 owl:maxQualifiedCardinality "1"^^xsd:nonNegativeInteger ;
                                 owl:onDataRange xsd:boolean
                               ] ,
                               [ rdf:type owl:Restriction ;
                                 owl:onProperty :metricalNotes ;
                                 owl:maxQualifiedCardinality "1"^^xsd:nonNegativeInteger ;
                                 owl:onDataRange xsd:string
                               ] ,
                               [ rdf:type owl:Restriction ;
                                 owl:onProperty :patterningMetricalScheme ;
                                 owl:maxQualifiedCardinality "1"^^xsd:nonNegativeInteger ;
                                 owl:onDataRange xsd:string
                               ] ,
                               [ rdf:type owl:Restriction ;
                                 owl:onProperty :rhymeScheme ;
                                 owl:maxQualifiedCardinality "1"^^xsd:nonNegativeInteger ;
                                 owl:onDataRange xsd:string
                               ] ,
                               [ rdf:type owl:Restriction ;
                                 owl:onProperty :syllabicMetricalScheme ;
                                 owl:maxQualifiedCardinality "1"^^xsd:nonNegativeInteger ;
                                 owl:onDataRange xsd:string
                               ] ;
               <http://purl.org/dc/elements/1.1/date> "2018-06-16T18:37:24Z"^^xsd:dateTime ;
               rdfs:comment """The prosodic analysis using a Stanza as the unit of reference
Eg.: The number of lines of a Stanza or its categorisation according to metrics (such as “quatrain”)"""@en ;
               rdfs:label "Stanza Pattern"@en .


###  http://postdata.linhd.uned.es/ontology/postdata-poeticAnalysis#StructuralUnit
:StructuralUnit rdf:type owl:Class ;
                rdfs:subClassOf <http://postdata.linhd.uned.es/ontology/postdata-core#LinguisticObject> ;
                rdfs:label "Structural Unit"@en .


###  http://postdata.linhd.uned.es/ontology/postdata-poeticAnalysis#Symbol
:Symbol rdf:type owl:Class ;
        rdfs:comment "Each element of the notation used to describe a metrical pattern"@en ;
        rdfs:isDefinedBy "http://postdata.linhd.uned.es/ontology/postdata-prosodicElements"@en ;
        rdfs:label "Symbol"@en .


###  http://postdata.linhd.uned.es/ontology/postdata-poeticAnalysis#Trope
:Trope rdf:type owl:Class ;
       rdfs:subClassOf :FigureOfSpeech ;
       rdfs:label "Trope"@en .


###  http://postdata.linhd.uned.es/ontology/postdata-poeticAnalysis#Word
:Word rdf:type owl:Class ;
      rdfs:subClassOf :StructuralUnit ,
                      <http://purl.org/ontology/olo/core#Slot> ,
                      [ rdf:type owl:Restriction ;
                        owl:onProperty :isInflectedForm ;
                        owl:maxQualifiedCardinality "1"^^xsd:nonNegativeInteger ;
                        owl:onClass :Word
                      ] ,
                      [ rdf:type owl:Restriction ;
                        owl:onProperty :content ;
                        owl:qualifiedCardinality "1"^^xsd:nonNegativeInteger ;
                        owl:onDataRange xsd:string
                      ] ,
                      [ rdf:type owl:Restriction ;
                        owl:onProperty :lemma ;
                        owl:maxQualifiedCardinality "1"^^xsd:nonNegativeInteger ;
                        owl:onDataRange xsd:string
                      ] ,
                      [ rdf:type owl:Restriction ;
                        owl:onProperty :morphologicalAnnotation ;
                        owl:maxQualifiedCardinality "1"^^xsd:nonNegativeInteger ;
                        owl:onDataRange xsd:string
                      ] ,
                      [ rdf:type owl:Restriction ;
                        owl:onProperty :phoneticTranscription ;
                        owl:maxQualifiedCardinality "1"^^xsd:nonNegativeInteger ;
                        owl:onDataRange xsd:string
                      ] ;
      rdfs:comment """The smallest symbol or set of symbols that are used to form lexical units. Words are used with others (or sometimes alone) to form a sentence.

Eg.: The word “life”"""@en ;
      rdfs:isDefinedBy "http://postdata.linhd.uned.es/ontology/postdata-poeticAnalysis#" ;
      rdfs:label "Word"@en ;
      rdfs:seeAlso "https://en.wikipedia.org/wiki/Lexical_item" ,
                   "https://en.wikipedia.org/wiki/Word" .


###  http://postdata.linhd.uned.es/ontology/postdata-poeticAnalysis#WordList
:WordList rdf:type owl:Class ;
          rdfs:subClassOf <http://purl.org/ontology/olo/core#OrderedList> ;
          rdfs:label "Word List"@en .


###  http://postdata.linhd.uned.es/ontology/postdata-transmission#Manifestation
<http://postdata.linhd.uned.es/ontology/postdata-transmission#Manifestation> rdf:type owl:Class ;
                                                                             rdfs:label "Manifestation"@en .


###  http://purl.org/ontology/olo/core#OrderedList
<http://purl.org/ontology/olo/core#OrderedList> rdf:type owl:Class .


###  http://purl.org/ontology/olo/core#Slot
<http://purl.org/ontology/olo/core#Slot> rdf:type owl:Class .


###  http://www.w3.org/2004/02/skos/core#Concept
<http://www.w3.org/2004/02/skos/core#Concept> rdf:type owl:Class .


###  http://www.w3.org/2004/02/skos/core#ConceptScheme
<http://www.w3.org/2004/02/skos/core#ConceptScheme> rdf:type owl:Class .


#################################################################
#    Individuals
#################################################################

###  http://postdata.linhd.uned.es/kos/clausula
<http://postdata.linhd.uned.es/kos/clausula> rdf:type owl:NamedIndividual ,
                                                      <http://www.w3.org/2004/02/skos/core#ConceptScheme> .


###  http://postdata.linhd.uned.es/kos/clausulaScheme-type
<http://postdata.linhd.uned.es/kos/clausulaScheme-type> rdf:type owl:NamedIndividual ,
                                                                 <http://www.w3.org/2004/02/skos/core#ConceptScheme> .


###  http://postdata.linhd.uned.es/kos/feet-type
<http://postdata.linhd.uned.es/kos/feet-type> rdf:type owl:NamedIndividual ,
                                                       <http://www.w3.org/2004/02/skos/core#ConceptScheme> .


###  http://postdata.linhd.uned.es/kos/foot-type
<http://postdata.linhd.uned.es/kos/foot-type> rdf:type owl:NamedIndividual ,
                                                       <http://www.w3.org/2004/02/skos/core#ConceptScheme> .


###  http://postdata.linhd.uned.es/kos/footUnit-type
<http://postdata.linhd.uned.es/kos/footUnit-type> rdf:type owl:NamedIndividual ,
                                                           <http://www.w3.org/2004/02/skos/core#ConceptScheme> .


###  http://postdata.linhd.uned.es/kos/metaplasm-type
<http://postdata.linhd.uned.es/kos/metaplasm-type> rdf:type owl:NamedIndividual ,
                                                            <http://www.w3.org/2004/02/skos/core#ConceptScheme> .


###  http://postdata.linhd.uned.es/kos/metrical-category
<http://postdata.linhd.uned.es/kos/metrical-category> rdf:type owl:NamedIndividual ,
                                                               <http://www.w3.org/2004/02/skos/core#ConceptScheme> .


###  http://postdata.linhd.uned.es/kos/metrical-complexity
<http://postdata.linhd.uned.es/kos/metrical-complexity> rdf:type owl:NamedIndividual ,
                                                                 <http://www.w3.org/2004/02/skos/core#ConceptScheme> .


###  http://postdata.linhd.uned.es/kos/metrical-context
<http://postdata.linhd.uned.es/kos/metrical-context> rdf:type owl:NamedIndividual ,
                                                              <http://www.w3.org/2004/02/skos/core#ConceptScheme> .


###  http://postdata.linhd.uned.es/kos/metrical-type
<http://postdata.linhd.uned.es/kos/metrical-type> rdf:type owl:NamedIndividual ,
                                                           <http://www.w3.org/2004/02/skos/core#ConceptScheme> .


###  http://postdata.linhd.uned.es/kos/nucleus-type
<http://postdata.linhd.uned.es/kos/nucleus-type> rdf:type owl:NamedIndividual ,
                                                          <http://www.w3.org/2004/02/skos/core#ConceptScheme> .


###  http://postdata.linhd.uned.es/kos/part-of-speech
<http://postdata.linhd.uned.es/kos/part-of-speech> rdf:type owl:NamedIndividual ,
                                                            <http://www.w3.org/2004/02/skos/core#ConceptScheme> .


###  http://postdata.linhd.uned.es/kos/rhetorical-operation
<http://postdata.linhd.uned.es/kos/rhetorical-operation> rdf:type owl:NamedIndividual ,
                                                                  <http://www.w3.org/2004/02/skos/core#ConceptScheme> .


###  http://postdata.linhd.uned.es/kos/rhymeDisposition-type
<http://postdata.linhd.uned.es/kos/rhymeDisposition-type> rdf:type owl:NamedIndividual ,
                                                                   <http://www.w3.org/2004/02/skos/core#ConceptScheme> .


###  http://postdata.linhd.uned.es/kos/rhymeMatching-type
<http://postdata.linhd.uned.es/kos/rhymeMatching-type> rdf:type owl:NamedIndividual ,
                                                                <http://www.w3.org/2004/02/skos/core#ConceptScheme> .


###  http://postdata.linhd.uned.es/kos/stanza-type
<http://postdata.linhd.uned.es/kos/stanza-type> rdf:type owl:NamedIndividual ,
                                                         <http://www.w3.org/2004/02/skos/core#ConceptScheme> .


###  http://postdata.linhd.uned.es/kos/stanzaEdition-type
<http://postdata.linhd.uned.es/kos/stanzaEdition-type> rdf:type owl:NamedIndividual ,
                                                                <http://www.w3.org/2004/02/skos/core#ConceptScheme> .


###  http://postdata.linhd.uned.es/kos/type-of-acrostic
<http://postdata.linhd.uned.es/kos/type-of-acrostic> rdf:type owl:NamedIndividual ,
                                                              <http://www.w3.org/2004/02/skos/core#ConceptScheme> .


###  http://postdata.linhd.uned.es/kos/type-of-intertextuality
<http://postdata.linhd.uned.es/kos/type-of-intertextuality> rdf:type owl:NamedIndividual ,
                                                                     <http://www.w3.org/2004/02/skos/core#ConceptScheme> .


###  http://postdata.linhd.uned.es/kos/type-of-scheme
<http://postdata.linhd.uned.es/kos/type-of-scheme> rdf:type owl:NamedIndividual ,
                                                            <http://www.w3.org/2004/02/skos/core#ConceptScheme> .


###  http://postdata.linhd.uned.es/kos/type-of-trope
<http://postdata.linhd.uned.es/kos/type-of-trope> rdf:type owl:NamedIndividual ,
                                                           <http://www.w3.org/2004/02/skos/core#ConceptScheme> .


###  http://postdata.linhd.uned.es/kos/versification-type
<http://postdata.linhd.uned.es/kos/versification-type> rdf:type owl:NamedIndividual ,
                                                                <http://www.w3.org/2004/02/skos/core#ConceptScheme> .


###  http://postdata.linhd.uned.es/ontology/postdata-poeticAnalysis#scansion-type
:scansion-type rdf:type owl:NamedIndividual ,
                        <http://www.w3.org/2004/02/skos/core#ConceptScheme> .


###  http://postdata.linhd.uned.es/ontology/postdata-poeticAnalysis#type-of-enjambment
:type-of-enjambment rdf:type owl:NamedIndividual ,
                             <http://www.w3.org/2004/02/skos/core#ConceptScheme> .


#################################################################
#    Annotations
#################################################################

<http://iflastandards.info/ns/fr/frbr/frbroo/CLP104_subject_to> rdfs:comment """This property associates a publication, i.e. an instance of F3 Manifestation Product Type, with an instance of E30 Right, which applies to all exemplars of that publication, as long as they are recognised as exemplars of that publication.
The rights covered by this property may include: acquisition or access authorisation; terms of availability; access restrictions on the Manifestation Product Type; etc.
"""@en ;
                                                                rdfs:label "subject to"@en .


<http://iflastandards.info/ns/fr/frbr/frbroo/CLP104i_applies_to> rdfs:comment """
"""@en ;
                                                                 rdfs:label "applies to"@en .


<http://iflastandards.info/ns/fr/frbr/frbroo/CLP105_right_held_by> rdfs:comment """This property associates a publication, i.e. an instance of F3 Manifestation Product Type, with an instance of E39 Actor, who holds an instance of E30 Right on all exemplars of that publication, as long as they are recognised as exemplars of that publication.
"""@en ;
                                                                   rdfs:label "right held by"@en .


<http://iflastandards.info/ns/fr/frbr/frbroo/CLP105i_right_on> rdfs:comment """
"""@en ;
                                                               rdfs:label "right on"@en .


<http://iflastandards.info/ns/fr/frbr/frbroo/CLP2_should_have_type> rdfs:comment """This property associates a publication, i.e. an instance of F3 Manifestation Product Type, with an instance of E55 Type, which all exemplars of that publication should belong to, as long as they are recognised as exemplars of that publication. Typically, this property is observed on one exemplar of a publication, and extrapolated to all other exemplars of the same publication. This logical inference is an induction along the path that can be modelled as: F3 Manifestation Product Type R7i has example F5 Item P41i was classified by E17 Type Assignment P42 assigned E55 Type.
It can happen that a given exemplar, or subset of exemplars, originally produced, or intended to be produced, with that characteristic, accidentally lacks it. This fact should be recorded as a property of F5 Item, and not of F3 Manifestation Product Type.
"""@en ;
                                                                    rdfs:label "should have type"@en .


<http://iflastandards.info/ns/fr/frbr/frbroo/CLP2i_should_be_type_of> rdfs:comment """
"""@en ;
                                                                      rdfs:label "should be type of"@en .


<http://iflastandards.info/ns/fr/frbr/frbroo/CLP43_should_have_dimension> rdfs:comment """This property associates a publication, i.e. an instance of F3 Manifestation Product Type, with an instance of E54 Dimension, which all exemplars of that publication should have, as long as they are recognised as exemplars of that publication. Typically, this property is observed on one exemplar of a publication, and extrapolated to all other exemplars of the same publication. This logical inference is an induction along the path that can be modelled as: F3 Manifestation Product Type R7i has example F5 Item P39i was measured by E16 Measurement P40 observed dimension E54 Dimension.
It can happen that a given exemplar, or subset of exemplars, originally produced, or intended to be produced, with that characteristic, accidentally lacks it. This fact should be recorded as a property of F5 Item, and not of F3 Manifestation Product Type.
"""@en ;
                                                                          rdfs:label "should have dimension"@en .


<http://iflastandards.info/ns/fr/frbr/frbroo/CLP43i_should_be_dimension_of> rdfs:comment """
"""@en ;
                                                                            rdfs:label "should be dimension of"@en .


<http://iflastandards.info/ns/fr/frbr/frbroo/CLP45_should_consist_of> rdfs:comment """This property associates a publication, i.e. an instance of F3 Manifestation Product Type, with an instance of E57 Material, which all exemplars of that publication should consist of, as long as they are recognised as exemplars of that publication. Typically, this property is observed on one exemplar of a publication, and extrapolated to all other exemplars of the same publication. This logical inference is an induction along the path that can be modelled as: F3 Manifestation Product Type R7i has example F5 Item P41i was classified by E17 Type Assignment P42 assigned E57 Material.
It can happen that a given exemplar, or subset of exemplars, originally produced, or intended to be produced, with that characteristic, accidentally lacks it. This fact should be recorded as a property of F5 Item, and not of F3 Manifestation Product Type.
"""@en ;
                                                                      rdfs:label "should consist of"@en .


<http://iflastandards.info/ns/fr/frbr/frbroo/CLP45i_should_be_incorporated_in> rdfs:comment """
"""@en ;
                                                                               rdfs:label "should be incorporated in"@en .


<http://iflastandards.info/ns/fr/frbr/frbroo/CLP46_should_be_composed_of> rdfs:comment """This property associates an instance of F3 Manifestation Product Type which prescribes that all its Items will contain as parts an Item of another instance of F3 Manifestation Product Type with that instance of F3 Manifestation Product Type.
"""@en ;
                                                                          rdfs:label "should be composed of"@en .


<http://iflastandards.info/ns/fr/frbr/frbroo/CLP46i_may_form_part_of> rdfs:comment """
"""@en ;
                                                                      rdfs:label "may form part of"@en .


<http://iflastandards.info/ns/fr/frbr/frbroo/CLR6_should_carry> rdfs:comment """This property associates a publication, i.e. an instance of F3 Manifestation Product Type, with an instance of F24 Publication Expression, which all exemplars of that publication should carry, as long as they are recognised as complete exemplars of that publication. Typically, this property is observed on one exemplar of a publication, and extrapolated to all other exemplars of the same publication. This logical inference is an induction along the path that can be modelled as: F3 Manifestation Product Type R7i has example F5 Item R6 carries F24 Publication Expression.
It can happen that a given exemplar, or a subset of exemplars, originally produced, or intended to be produced with that characteristic, accidentally lacks part of the publication expression. This fact should be recorded as a property of F5 Item, and not of F3 Manifestation Product Type.
"""@en ;
                                                                rdfs:label "should carry"@en .


<http://iflastandards.info/ns/fr/frbr/frbroo/CLR6i_should_be_carried_by> rdfs:comment """
"""@en ;
                                                                         rdfs:label "should be carried by"@en .


<http://iflastandards.info/ns/fr/frbr/frbroo/R10_has_member> rdfs:comment """This property associates an instance of F15 Complex Work with an instance of F1 Work that forms part of it. 
"""@en ;
                                                             rdfs:label "has member"@en .


<http://iflastandards.info/ns/fr/frbr/frbroo/R10i_is_member_of> rdfs:comment """
"""@en ;
                                                                rdfs:label "is member of"@en .


<http://iflastandards.info/ns/fr/frbr/frbroo/R11_has_issuing_rule> rdfs:comment """This property associates an instance of F18 Serial Work with the instance of E29 Design or Procedure that specifies the issuing policy planned by this Work, such as sequencing pattern, expected frequency and expected regularity.
This property is a shortcut of the full path: F18 Serial Work R23i was realised through F30 Publication Event P16 used specific object E29 Design or Procedure.
"""@en ;
                                                                   rdfs:label "has issuing rule"@en .


<http://iflastandards.info/ns/fr/frbr/frbroo/R11i_is_issuing_rule_of> rdfs:comment """
"""@en ;
                                                                      rdfs:label "is issuing rule of"@en .


<http://iflastandards.info/ns/fr/frbr/frbroo/R12_is_realised_in> rdfs:comment """This property associates an instance of F20 Performance Work with an instance of F25 Performance Plan that consists of signs (words, figures, etc.) which express the directions the instance of F20 Performance Work consists of.
"""@en ;
                                                                 rdfs:label "is realised in"@en .


<http://iflastandards.info/ns/fr/frbr/frbroo/R12i_realises> rdfs:comment """
"""@en ;
                                                            rdfs:label "realises"@en .


<http://iflastandards.info/ns/fr/frbr/frbroo/R13_is_realised_in> rdfs:comment """This property associates an instance of F21 Recording Work with an instance of F26 Recording realising the instance of F21 Recording Work.
This is a shortcut of the more elaborated path through R22 was realised through, F29 Recording Event and R21 created, which should be used when information about the recording event is available.
"""@en ;
                                                                 rdfs:label "is realised in"@en .


<http://iflastandards.info/ns/fr/frbr/frbroo/R13i_realises> rdfs:comment """
"""@en ;
                                                            rdfs:label "realises"@en .


<http://iflastandards.info/ns/fr/frbr/frbroo/R15_has_fragment> rdfs:comment """This property associates the fragment of an expression and the expression of which it is a fragment.
"""@en ;
                                                               rdfs:label "has fragment"@en .


<http://iflastandards.info/ns/fr/frbr/frbroo/R15i_is_fragment_of> rdfs:comment """
"""@en ;
                                                                  rdfs:label "is fragment of"@en .


<http://iflastandards.info/ns/fr/frbr/frbroo/R16_initiated> rdfs:comment """This property associates the first conception of a work and the work itself that ensued from a given initial idea.
It marks the origin of the causality chain that results in a work’s coming into existence.
"""@en ;
                                                            rdfs:label "initiated"@en .


<http://iflastandards.info/ns/fr/frbr/frbroo/R16i_was_initiated_by> rdfs:comment """
"""@en ;
                                                                    rdfs:label "was initiated by"@en .


<http://iflastandards.info/ns/fr/frbr/frbroo/R17_created> rdfs:comment """This property associates the expression that was first externalised during a particular creation event with that particular creation event.
"""@en ;
                                                          rdfs:label "created"@en .


<http://iflastandards.info/ns/fr/frbr/frbroo/R17i_was_created_by> rdfs:comment """
"""@en ;
                                                                  rdfs:label "was created by"@en .


<http://iflastandards.info/ns/fr/frbr/frbroo/R18_created> rdfs:comment """This property associates an instance of F28 Expression Creation with the first physical objects in which the resulting instance of F2 Expression was embodied.
"""@en ;
                                                          rdfs:label "created"@en .


<http://iflastandards.info/ns/fr/frbr/frbroo/R18i_was_created_by> rdfs:comment """
"""@en ;
                                                                  rdfs:label "was created by"@en .


<http://iflastandards.info/ns/fr/frbr/frbroo/R19_created_a_realization_of> rdfs:comment """This property associates an instance of F28 Expression Creation with the corresponding instance of F14 Individual Work or an instance of F15 Complex Work of which the corresponding instance of F14 Individual Work is a member.
"""@en ;
                                                                           rdfs:label "created a realization of"@en .


<http://iflastandards.info/ns/fr/frbr/frbroo/R19i_was_realised_through> rdfs:comment """
"""@en ;
                                                                        rdfs:label "was realised through"@en .


<http://iflastandards.info/ns/fr/frbr/frbroo/R1_is_logical_successor_of> rdfs:comment """This property associates an instance of F1 Work which logically continues the content of another instance of F1 Work with the latter.
"""@en ;
                                                                         rdfs:label "is logical successor of"@en .


<http://iflastandards.info/ns/fr/frbr/frbroo/R1i_has_successor> rdfs:comment """
"""@en ;
                                                                rdfs:label "has successor"@en .


<http://iflastandards.info/ns/fr/frbr/frbroo/R20_recorded> rdfs:comment """This property associates an instance of F29 Recording Event with the instance of E2 Temporal Entity which was captured.
"""@en ;
                                                           rdfs:label "recorded"@en .


<http://iflastandards.info/ns/fr/frbr/frbroo/R20i_was_recorded_through> rdfs:comment """
"""@en ;
                                                                        rdfs:label "was recorded through"@en .


<http://iflastandards.info/ns/fr/frbr/frbroo/R21_created> rdfs:comment """This property associates an instance of F29 Recording Event with the instance of F26 Recording that was created.
"""@en ;
                                                          rdfs:label "created"@en .


<http://iflastandards.info/ns/fr/frbr/frbroo/R21i_was_created_through> rdfs:comment """
"""@en ;
                                                                       rdfs:label "was created through"@en .


<http://iflastandards.info/ns/fr/frbr/frbroo/R22_created_a_realization_of> rdfs:comment """This property associates an instance of F29 Recording Event with the instance of F21 Recording Work it realised.
"""@en ;
                                                                           rdfs:label "created a realization of"@en .


<http://iflastandards.info/ns/fr/frbr/frbroo/R22i_was_realised_through> rdfs:comment """
"""@en ;
                                                                        rdfs:label "was realised through"@en .


<http://iflastandards.info/ns/fr/frbr/frbroo/R23_created_a_realization_of> rdfs:comment """This property associates an instance of F30 Publication Event with the instance of F19 Publication Work it realised.
"""@en ;
                                                                           rdfs:label "created a realization of"@en .


<http://iflastandards.info/ns/fr/frbr/frbroo/R23i_was_realised_through> rdfs:comment """
"""@en ;
                                                                        rdfs:label "was realised through"@en .


<http://iflastandards.info/ns/fr/frbr/frbroo/R24_created> rdfs:comment """This property associates the instance of F24 Publication Expression that was created during a particular F30 Publication Event with that F30 Publication Event.
"""@en ;
                                                          rdfs:label "created"@en .


<http://iflastandards.info/ns/fr/frbr/frbroo/R24i_was_created_through> rdfs:comment """
"""@en ;
                                                                       rdfs:label "was created through"@en .


<http://iflastandards.info/ns/fr/frbr/frbroo/R25_performed> rdfs:comment """This property associates an instance of F31 Performance with the instance of F25 Performance Plan to which all those participating in the performance were supposed to conform.
"""@en ;
                                                            rdfs:label "performed"@en .


<http://iflastandards.info/ns/fr/frbr/frbroo/R25i_was_performed_in> rdfs:comment """
"""@en ;
                                                                    rdfs:label "was performed in"@en .


<http://iflastandards.info/ns/fr/frbr/frbroo/R26_produced_things_of_type> rdfs:comment """This property associates an instance of F32 Carrier Production Event with the instance of F3 Manifestation Product Type it produced items of.
"""@en ;
                                                                          rdfs:label "produced things of type"@en .


<http://iflastandards.info/ns/fr/frbr/frbroo/R26i_was_produced_by> rdfs:comment """
"""@en ;
                                                                   rdfs:label "was produced by"@en .


<http://iflastandards.info/ns/fr/frbr/frbroo/R27_used_as_source_material> rdfs:comment """This property associates an instance of F32 Carrier Production Event with the set of signs provided by the publisher to be carried by all of the produced items.
"""@en ;
                                                                          rdfs:label "used as source material"@en .


<http://iflastandards.info/ns/fr/frbr/frbroo/R27i_was_used_by> rdfs:comment """
"""@en ;
                                                               rdfs:label "was used by"@en .


<http://iflastandards.info/ns/fr/frbr/frbroo/R28_produced> rdfs:comment """This property associates an instance of F32 Carrier Production Event with any one of the produced items (i.e., the instances of F5 Item or F53 Material Copy).
"""@en ;
                                                           rdfs:label "produced"@en .


<http://iflastandards.info/ns/fr/frbr/frbroo/R28i_was_produced_by> rdfs:comment """
"""@en ;
                                                                   rdfs:label "was produced by"@en .


<http://iflastandards.info/ns/fr/frbr/frbroo/R29_reproduced> rdfs:comment """This property associates an instance of F33 Reproduction Event with an instance of E84 Information Carrier it reproduces.
"""@en ;
                                                             rdfs:label "reproduced"@en .


<http://iflastandards.info/ns/fr/frbr/frbroo/R29i_was_reproduced_by> rdfs:comment """
"""@en ;
                                                                     rdfs:label "was reproduced by"@en .


<http://iflastandards.info/ns/fr/frbr/frbroo/R2_is_derivative_of> rdfs:comment """This property associates an instance of F1 Work which modifies the content of another instance of F1 Work with the latter. The property R2.1 has type of this property allows for specifying the kind of derivation, such as adaptation, summarisation etc.
"""@en ;
                                                                  rdfs:label "is derivative of"@en .


<http://iflastandards.info/ns/fr/frbr/frbroo/R2i_has_derivative> rdfs:comment """
"""@en ;
                                                                 rdfs:label "has derivative"@en .


<http://iflastandards.info/ns/fr/frbr/frbroo/R30_produced> rdfs:comment """This property associates an instance of F33 Reproduction Event with an instance of E84 Information Carrier it produces.
"""@en ;
                                                           rdfs:label "produced"@en .


<http://iflastandards.info/ns/fr/frbr/frbroo/R30i_was_produced_by> rdfs:comment """
"""@en ;
                                                                   rdfs:label "was produced by"@en .


<http://iflastandards.info/ns/fr/frbr/frbroo/R31_is_reproduction_of> rdfs:comment """This property associates an instance of E84 Information Carrier which is a reproduction of another instance of E84 Information Carrier with the latter. It is considered that a reproduction of multiple originals resulting in a single product requires a merging of those objects prior to the reproduction. Therefore an Information Carrier is regarded to be a reproduction of one and only one original. This property is a shortcut of the more fully developed path from E84 Information Carrier through R30 produced (was produced by), F33 Reproduction Event R29 reproduced (was reproduced by) to E84 Information Carrier.
"""@en ;
                                                                     rdfs:label "is reproduction of"@en .


<http://iflastandards.info/ns/fr/frbr/frbroo/R31i_has_reproduction> rdfs:comment """
"""@en ;
                                                                    rdfs:label "has reproduction"@en .


<http://iflastandards.info/ns/fr/frbr/frbroo/R32_is_warranted_by> rdfs:comment """This property associates an instance of F35 Nomen Use Statement with an instance of F52 Name Use Activity which provides evidence for the use of the particular nomen in the stated sense. The association between this name use activity and a source for it may be described by the property P70 documents (is documented in).
"""@en ;
                                                                  rdfs:label "is warranted by"@en .


<http://iflastandards.info/ns/fr/frbr/frbroo/R32i_warrants> rdfs:comment """
"""@en ;
                                                            rdfs:label "warrants"@en .


<http://iflastandards.info/ns/fr/frbr/frbroo/R34_has_validity_period> rdfs:comment """This property associates an instance of F34 KOS with the instance of E52 Time-Span describing the period for which the particular KOS Expression was regarded as valid by its maintainers. Each change of validity status of a nomen use statement within a KOS should be associated with a release change of the KOS. The individual time-span of a validity state of a nomen would be the union of the time-spans of the KOS in which the Nomen was declared to have the particular validity status (provisional, accepted, obsolete etc...).
"""@en ;
                                                                      rdfs:label "has validity period"@en .


<http://iflastandards.info/ns/fr/frbr/frbroo/R34i_is_validity_period_of> rdfs:comment """
"""@en ;
                                                                         rdfs:label "is validity period of"@en .


<http://iflastandards.info/ns/fr/frbr/frbroo/R35_specified_by> rdfs:comment """This property associates an instance of F35 Nomen Use Statement with an instance of F34 KOS in which the Nomen Use Statement has a given status. The property R35.1 allows for specifying the particular status of the nomen use statement within the KOS. An instance of R35 is specified by should have only one status.
"""@en ;
                                                               rdfs:label "specified by"@en .


<http://iflastandards.info/ns/fr/frbr/frbroo/R35i_specifies> rdfs:comment """
"""@en ;
                                                             rdfs:label "specifies"@en .


<http://iflastandards.info/ns/fr/frbr/frbroo/R36_uses_script_conversion> rdfs:comment """This property associates an instance of F35 Nomen Use Statement with the instance of F36 Script Conversion that was used to create the Nomen referred to in the Nomen Use Statement. The source of this conversion may or may not be explicitly mentioned. Is shortcut of: F35 Nomen Use Statement R17 was created by (created) F28 Expression Creation P33 used specific technique (was used by) E29 Design or Procedure.
"""@en ;
                                                                         rdfs:label "uses script conversion"@en .


<http://iflastandards.info/ns/fr/frbr/frbroo/R36i_is_script_conversion_used_in> rdfs:comment """This property associates an instance of F35 Nomen Use Statement with the instance of F12 Nomen for which it declares usage.
"""@en ;
                                                                                rdfs:label "is script conversion used in"@en .


<http://iflastandards.info/ns/fr/frbr/frbroo/R37_states_as_nomen> rdfs:comment """
"""@en ;
                                                                  rdfs:label "states as nomen"@en .


<http://iflastandards.info/ns/fr/frbr/frbroo/R37i_is_stated_as_nomen_in> rdfs:comment """
"""@en ;
                                                                         rdfs:label "is stated as nomen in"@en .


<http://iflastandards.info/ns/fr/frbr/frbroo/R38_refers_to_thema> rdfs:comment """This property associates an instance of F35 Nomen Use Statement with the instance of E1 CRM Entity for which it declares the usage of a nomen.
"""@en ;
                                                                  rdfs:label "refers to thema"@en .


<http://iflastandards.info/ns/fr/frbr/frbroo/R38i_is_thema_of> rdfs:comment """
"""@en ;
                                                               rdfs:label "is thema of"@en .


<http://iflastandards.info/ns/fr/frbr/frbroo/R39_is_intended_for> rdfs:comment """This property associates an instance of F35 Nomen Use Statement with an instance of E74 Group which is the target audience for which the associated nomen use is intended. To indicate that the associated nomen is declared as preferred in all contexts, the instance of E74 Group is ‘mankind’.
"""@en ;
                                                                  rdfs:label "is intended for"@en .


<http://iflastandards.info/ns/fr/frbr/frbroo/R39i_is_target_audience_in> rdfs:comment """
"""@en ;
                                                                         rdfs:label "is target audience in"@en .


<http://iflastandards.info/ns/fr/frbr/frbroo/R3_is_realised_in> rdfs:comment """This property associates an instance of F22 Self-Contained Expression with an instance of F1 Work.
This property expresses the association that exists between an expression (F22) and the work that this expression conveys. The semantics of the association will be different depending on what specific subtype of F1 Work the work is an instance of. If the work is an instance of F14 Individual Work, the F22 Self-Contained Expression completely conveys the individual work. If the work is an instance of F15 Complex Work, the F22 Self-Contained Expression conveys an alternative member of the complex work.
Our factual knowledge of how a given work is realised into an expression is often limited and this property makes it possible to express the association between instances of F22 Self-Contained Expression and the work it conveys without using the more developed paths.
The property R3.1 has type: E55 Type allows for specifying the role played by the referred to expression in the overall bibliographic history of the work (e.g., ‘progenitor expression’, on which all other expressions of the same work are based; ‘reference for canonical citations’, in the sense of the HuCit ontology developed by Matteo Romanello and Michele Pasin; ‘earliest draft’, ‘intermediate draft’, ‘final clean draft’, ‘princeps edition’, etc.).
"""@en ;
                                                                rdfs:label "is realised in"@en .


<http://iflastandards.info/ns/fr/frbr/frbroo/R3i_realises> rdfs:comment """
"""@en ;
                                                           rdfs:label "realises"@en .


<http://iflastandards.info/ns/fr/frbr/frbroo/R40_has_representative_expression> rdfs:comment """This property identifies an instance of F22 Self-Contained Expression that has been chosen as the most characteristic expression of the instance of F1 Work of which it is an expression. There is no other semantic implication to this notion of being characteristic than to be an adequate candidate to uniquely identify the Work realized by it. Prototypically, this is the instance of F22 Self-Contained Expression that is deemed characteristic of an instance of F15 Complex Work.
Typically, any expression that is not regarded as “representative” for the work it expresses, would require a controlled access point, with qualifiers specifying the differences between that expression and a representative expression, although this may not always be done in practice. The title of a Work may not be one taken from a representative expression.
A given work can have more than one representative expression, provided the differences between these expressions are not deemed “substantial.” If the anticipated needs of users are not considered to call for bibliographic distinctions between variant expressions of a work, then even expressions that differ significantly from each other can be regarded as equally representative for the work. (See FRBR: Final Report, p. 19-20).
A given expression can be deemed representative for a work with regard to some of its aspects (e.g., the text contained in an edition the title proper of which reads ‘The tragicall historie of HAMLET Prince of Denmarke’, and the language of that text), and not representative for it with regard to some other aspects (e.g., the title proper ‘The tragicall historie of HAMLET Prince of Denmarke’ itself, which, being different from the title that is regarded as “representative” for Shakespeare’s work, will require the use of a controlled access point).
R40 has representative expression is a shortcut of the more developed path F1 Work R50i was assigned by F42 Representative Expression Assignment R51 assigned F2 Expression.

"""@en ;
                                                                                rdfs:label "has representative expression"@en .


<http://iflastandards.info/ns/fr/frbr/frbroo/R40i_is_representative_expression_for> rdfs:comment """
"""@en ;
                                                                                    rdfs:label "is representative expression for"@en .


<http://iflastandards.info/ns/fr/frbr/frbroo/R41_has_rep_manifestation_product_type> rdfs:comment """This property identifies an instance of F3 Manifestation Product Type that has been chosen as the most characteristic Manifestation Product Type of the instance of F2 Expression of which it is a manifestation.
Identifying an instance of F3 Manifestation Product Type that is representative for an instance of F2 Expression makes it possible in turn to identify an instance of F2 Expression that is representative for an instance of F1 Work, and to decide what should be regarded as the title of the work.
The title of an Expression may not be one taken from a representative Manifestation Product Type or Manifestation Singleton.
A given expression can have more than one Representative Manifestation Product Type.
R41 has representative manifestation product type is a shortcut of the more developed path F2 Expression R48i was assigned by F41 Representative Manifestation Assignment R49 assigned F3 Manifestation Product Type.

"""@en ;
                                                                                     rdfs:label "has rep manifestation product type"@en .


<http://iflastandards.info/ns/fr/frbr/frbroo/R41i_is_rep_manifestation_product_type_for> rdfs:comment """
"""@en ;
                                                                                         rdfs:label "is rep manifestation product type for"@en .


<http://iflastandards.info/ns/fr/frbr/frbroo/R42_is_representative_manifestation_singleton_for> rdfs:comment """This property identifies an instance of Manifestation Singleton that has been declared as the unique representative for an instance of F2 Expression by some bibliographic agency.
This property identifies an instance of F4 Manifestation Singleton that has been chosen as the most characteristic Manifestation Singleton of the instance of F2 Expression of which it is a manifestation.
Identifying an instance of F4 Manifestation Singleton that is representative for an instance of F2 Expression makes it possible in turn to identify an instance of F2 Expression that is representative for an instance of F1 Work, and to decide what should be regarded as the title of the work.
The title of an Expression may not be one taken from a representative Manifestation Product Type or Manifestation Singleton.
A given expression can have more than one representative Manifestation Singleton.
It is a shortcut for the more developed path: F2 Expression R48i was assigned by F41 Representative Manifestation Assignment R53 assigned F4 Manifestation Singleton.

"""@en ;
                                                                                                rdfs:label "is representative manifestation singleton for"@en .


<http://iflastandards.info/ns/fr/frbr/frbroo/R42i_has_representative_manifestation_singleton> rdfs:comment """
"""@en ;
                                                                                              rdfs:label "has representative manifestation singleton"@en .


<http://iflastandards.info/ns/fr/frbr/frbroo/R43_carried_out_by> rdfs:comment """This property associates a bibliographic agency (represented by one or more of its cataloguers) and the assigning of which Manifestation (i.e., which instance of F3 Manifestation Product Type or F4 Manifestation Singleton) is representative for a given expression.
In cataloguing practice, such a relationship is usually just implicit. However, it can become explicit, for example when a bibliographic agency creates an authority record for a given work and fills the “Source” field with information about the publication that contains the expression that was used by the bibliographic agency to establish the controlled access point for the work realised in that expression.
"""@en ;
                                                                 rdfs:label "carried out by"@en .


<http://iflastandards.info/ns/fr/frbr/frbroo/R43i_performed> rdfs:comment """
"""@en ;
                                                             rdfs:label "performed"@en .


<http://iflastandards.info/ns/fr/frbr/frbroo/R44_carried_out_by> rdfs:comment """This property associates a bibliographic agency (represented by one or more of its cataloguers) and the assigning of which expression is representative for a given Work.
In cataloguing practice, such a relationship is usually just implicit. However, it can become explicit, for example when a bibliographic agency creates an authority record for a given work and fills the “Source” field with information about the publication that contains the expression that was used by the bibliographic agency to establish the controlled access point for the work realised in that expression.

"""@en ;
                                                                 rdfs:label "carried out by"@en .


<http://iflastandards.info/ns/fr/frbr/frbroo/R44i_performed> rdfs:comment """
"""@en ;
                                                             rdfs:label "performed"@en .


<http://iflastandards.info/ns/fr/frbr/frbroo/R45_assigned_to> rdfs:comment """This property identifies the entity to which an actor, such as a bibliographic agency, assigned an instance of F13 Identifier.
"""@en ;
                                                              rdfs:label "assigned to"@en .


<http://iflastandards.info/ns/fr/frbr/frbroo/R45i_was_assigned_by> rdfs:comment """
"""@en ;
                                                                   rdfs:label "was assigned by"@en .


<http://iflastandards.info/ns/fr/frbr/frbroo/R46_assigned_to> rdfs:comment """This property associates the instance of F13 Identifier assigned to an instance of E1 CRM Entity and the event of assigning it.
"""@en ;
                                                              rdfs:label "assigned to"@en .


<http://iflastandards.info/ns/fr/frbr/frbroo/R46i_was_assigned_by> rdfs:comment """
"""@en ;
                                                                   rdfs:label "was assigned by"@en .


<http://iflastandards.info/ns/fr/frbr/frbroo/R48_assigned_to> rdfs:comment """This property associates the event of assigning a representative instance of F3 Manifestation Product Type or F4 Manifestation Singleton with the expression to which it was assigned.
"""@en ;
                                                              rdfs:label "assigned to"@en .


<http://iflastandards.info/ns/fr/frbr/frbroo/R48i_was_assigned_by> rdfs:comment """
"""@en ;
                                                                   rdfs:label "was assigned by"@en .


<http://iflastandards.info/ns/fr/frbr/frbroo/R49_assigned> rdfs:comment """This property associates the event of assigning a representative instance of F3 Manifestation Product Type with the F3 Manifestation Product Type which has been assigned.
"""@en ;
                                                           rdfs:label "assigned"@en .


<http://iflastandards.info/ns/fr/frbr/frbroo/R49i_was_assigned_by> rdfs:comment """
"""@en ;
                                                                   rdfs:label "was assigned by"@en .


<http://iflastandards.info/ns/fr/frbr/frbroo/R4_carriers_provided_by> rdfs:comment """This property associates a publication, i.e. an instance of F3 Manifestation Product Type, with an instance of F2 Expression, which all exemplars of that publication should carry, as long as they are recognised as complete exemplars of that publication. Typically, this property is observed on one exemplar of a publication, and extrapolated to all other exemplars of the same publication.
This property is a shortcut of: F2 Expression P165i is incorporated in F24 Publication Expression CLR6i should be carried by F3 Manifestation Product Type.
"""@en ;
                                                                      rdfs:label "carriers provided by"@en .


<http://iflastandards.info/ns/fr/frbr/frbroo/R4i_comprises_carriers_of> rdfs:comment """
"""@en ;
                                                                        rdfs:label "comprises carriers of"@en .


<http://iflastandards.info/ns/fr/frbr/frbroo/R50_assigned_to> rdfs:comment """This property associates the event of assigning a representative instance of F2 Expression with the instance of F15 Complex Work to which it was assigned.
"""@en ;
                                                              rdfs:label "assigned to"@en .


<http://iflastandards.info/ns/fr/frbr/frbroo/R50i_was_assigned_by> rdfs:comment """
"""@en ;
                                                                   rdfs:label "was assigned by"@en .


<http://iflastandards.info/ns/fr/frbr/frbroo/R51_assigned> rdfs:comment """This property associates the event of assigning a representative instance of F2 Expression with the F2 Expression which has been assigned.
"""@en ;
                                                           rdfs:label "assigned"@en .


<http://iflastandards.info/ns/fr/frbr/frbroo/R51i_was_assigned_by> rdfs:comment """
"""@en ;
                                                                   rdfs:label "was assigned by"@en .


<http://iflastandards.info/ns/fr/frbr/frbroo/R52_used_rule> rdfs:comment """This property associates the event of assigning an instance of F13 Identifier with the instructions followed by an actor, such as a Bibliographic Agency, in creating that identifier.
"""@en ;
                                                            rdfs:label "used rule"@en .


<http://iflastandards.info/ns/fr/frbr/frbroo/R52i_was_the_rule_used_in> rdfs:comment """
"""@en ;
                                                                        rdfs:label "was the rule used in"@en .


<http://iflastandards.info/ns/fr/frbr/frbroo/R53_assigned> rdfs:comment """This property associates the event of assigning a representative instance of F4 Manifestation Singleton with the F4 Manifestation Singleton which has been assigned.
"""@en ;
                                                           rdfs:label "assigned"@en .


<http://iflastandards.info/ns/fr/frbr/frbroo/R53i_was_assigned_by> rdfs:comment """
"""@en ;
                                                                   rdfs:label "was assigned by"@en .


<http://iflastandards.info/ns/fr/frbr/frbroo/R54_has_nomen_language> rdfs:comment """This property associates an instance of F35 Nomen Use Statement with an instance of E56 Language which is a target language for the associated nomen use.
"""@en ;
                                                                     rdfs:label "has nomen language"@en .


<http://iflastandards.info/ns/fr/frbr/frbroo/R54i_is_language_of_nomen_in> rdfs:comment """
"""@en ;
                                                                           rdfs:label "is language of nomen in"@en .


<http://iflastandards.info/ns/fr/frbr/frbroo/R55_has_nomen_form> rdfs:comment """This property associates an instance of F35 Nomen Use Statement with the instance of E55 Type that characterizes the Nomen referred to in the Nomen Use Statement, such as abbreviation, full name etc. In the case of abbreviations, the source of this form may or may not be explicitly mentioned.
"""@en ;
                                                                 rdfs:label "has nomen form"@en .


<http://iflastandards.info/ns/fr/frbr/frbroo/R55i_is_nomen_form_in> rdfs:comment """
"""@en ;
                                                                    rdfs:label "is nomen form in"@en .


<http://iflastandards.info/ns/fr/frbr/frbroo/R56_has_related_use> rdfs:comment """This property associates an instance of F35 Nomen Use Statement with another instance of F35 Nomen Use Statement which has a related use in some context, such as alternative, lexical variant, replacing former use etc. The property R56.1 allows for specifying the particular kind of the nomen use statement relationship.
"""@en ;
                                                                  rdfs:label "has related use"@en .


<http://iflastandards.info/ns/fr/frbr/frbroo/R56i_is_related_use_for> rdfs:comment """
"""@en ;
                                                                      rdfs:label "is related use for"@en .


<http://iflastandards.info/ns/fr/frbr/frbroo/R57_is_based_on> rdfs:comment """This property associates an instance of F38 Character with an instance of E39 Actor that the character is motivated by or is intended to represent. An instance of F38 Character may be based on a combination of features taken from several actors. This property is a shortcut of the more fully developed path from E28 Conceptual Object, restricted to F38 Character, through the inverse of P94 has created (was created by), E65 Creation P17 was motivated by (motivated) to E1 CRM Entity restricted to E39 Actor.
"""@en ;
                                                              rdfs:label "is based on"@en .


<http://iflastandards.info/ns/fr/frbr/frbroo/R57i_is_basis_for> rdfs:comment """
"""@en ;
                                                                rdfs:label "is basis for"@en .


<http://iflastandards.info/ns/fr/frbr/frbroo/R58_has_fictional_member> rdfs:comment """This property associates an instance of F38 Character representing a group with another instance of F38 Character that is presented in relevant fiction as a member of the fictional group.
"""@en ;
                                                                       rdfs:label "has fictional member"@en .


<http://iflastandards.info/ns/fr/frbr/frbroo/R58i_is_fictional_member_of> rdfs:comment """
"""@en ;
                                                                          rdfs:label "is fictional member of"@en .


<http://iflastandards.info/ns/fr/frbr/frbroo/R59_had_typical_subject> rdfs:comment """This property associates an instance of F51 Pursuit with the instance of E1 CRM Entity that is the typical subject of the associated activity, such as an area of expertise in which the actor is engaged or was engaged.
"""@en ;
                                                                      rdfs:label "had typical subject"@en .


<http://iflastandards.info/ns/fr/frbr/frbroo/R59i_was_typical_subject_of> rdfs:comment """
"""@en ;
                                                                          rdfs:label "was typical subject of"@en .


<http://iflastandards.info/ns/fr/frbr/frbroo/R5_has_component> rdfs:comment """This property associates an F2 Expression X with a structural component Y that conveys in itself the complete concept of a work that is member of (R10) the overall work realized by X.
It does not cover the relationship that exists between pre-existing expressions that are re-used in a new, larger expression and that new, larger expression. Such a relationship is modelled by P165 incorporates.
"""@en ;
                                                               rdfs:label "has component"@en .


<http://iflastandards.info/ns/fr/frbr/frbroo/R5i_is_component_of> rdfs:comment """
"""@en ;
                                                                  rdfs:label "is component of"@en .


<http://iflastandards.info/ns/fr/frbr/frbroo/R60_used_to_use_language> rdfs:comment """This property associates an instance of F51 Pursuit with the instance of E56 Language that was characteristically used for the products of the associated activity.
The property R60.1 has type of use allows for specifying a particular form of use.
"""@en ;
                                                                       rdfs:label "used to use language"@en .


<http://iflastandards.info/ns/fr/frbr/frbroo/R60i_was_language_used_by> rdfs:comment """
"""@en ;
                                                                        rdfs:label "was language used by"@en .


<http://iflastandards.info/ns/fr/frbr/frbroo/R61_occured_in_kind_of_context> rdfs:comment """This property associates an instance of F52 Name Use Activity with the instance of E55 Type that characterises the kind of role or context within which the associated name was used.
"""@en ;
                                                                             rdfs:label "occured in kind of context"@en .


<http://iflastandards.info/ns/fr/frbr/frbroo/R61i_was_kind_of_context_for> rdfs:comment """
"""@en ;
                                                                           rdfs:label "was kind of context for"@en .


<http://iflastandards.info/ns/fr/frbr/frbroo/R62_was_used_for_membership_in> rdfs:comment """This property associates an instance of F52 Name Use Activity with the instance of E74 Group that characterises the context within which the associated name was used for membership in that group.
"""@en ;
                                                                             rdfs:label "was used for membership in"@en .


<http://iflastandards.info/ns/fr/frbr/frbroo/R62i_was_context_for> rdfs:comment """
"""@en ;
                                                                   rdfs:label "was context for"@en .


<http://iflastandards.info/ns/fr/frbr/frbroo/R63_named> rdfs:comment """This property associates an instance of F52 Name Use Activity with the instance of E1 CRM Entity that the associated name was used for.
"""@en ;
                                                        rdfs:label "named"@en .


<http://iflastandards.info/ns/fr/frbr/frbroo/R63i_was_named_by> rdfs:comment """
"""@en ;
                                                                rdfs:label "was named by"@en .


<http://iflastandards.info/ns/fr/frbr/frbroo/R64_used_name> rdfs:comment """This property associates an instance of F52 Name Use Activity with the instance of E41 Appellation that was used for the associated entity.
"""@en ;
                                                            rdfs:label "used name"@en .


<http://iflastandards.info/ns/fr/frbr/frbroo/R64i_was_name_used_by> rdfs:comment """
"""@en ;
                                                                    rdfs:label "was name used by"@en .


<http://iflastandards.info/ns/fr/frbr/frbroo/R65_recorded_aspects_of> rdfs:comment """This property associates an instance of F29 Recording Event with an instance of E18 Physical Thing some of whose features, at the time of recording, were recorded in that process.
"""@en ;
                                                                      rdfs:label "recorded aspects of"@en .


<http://iflastandards.info/ns/fr/frbr/frbroo/R65i_had_aspects_recorded_through> rdfs:comment """
"""@en ;
                                                                                rdfs:label "had aspects recorded through"@en .


<http://iflastandards.info/ns/fr/frbr/frbroo/R66_included_performed_version_of> rdfs:comment """This property associates an instance of F31 Performance with a product of the mind that was performed in the course of that instance of F31 Performance.
According to the level of knowledge available about the performance, the range of this property can actually be specialised as either an instance of F1 Work (if nothing is known as to which specific expression of the work was performed), or of F2 Expression (if there is a reasonable amount of certainty as to which specific expression—e.g., a well identified translation of a play—of the work was performed).
In addition to being a subproperty of P16 used specific object (was used for), this property also is a shortcut of the fully developed path that goes from F31 Performance to F1 Work through: R25 performed F25 Performance Plan P165 incorporates F22 Self-Contained Expression R3i realises. In this fully developed path, the specific instance of F22 Self-Contained Expression can be precisely identified and described for its own sake, or it can just be known to have necessarily existed.

"""@en ;
                                                                                rdfs:label "included performed version of"@en .


<http://iflastandards.info/ns/fr/frbr/frbroo/R66i_had_a_performed_version_through> rdfs:comment """
"""@en ;
                                                                                   rdfs:label "had a performed version through"@en .


<http://iflastandards.info/ns/fr/frbr/frbroo/R6_carries> rdfs:comment """This property associates an instance of F54 Utilised Information Carrier with the unique instance of F24 Publication Expression it carries.
"""@en ;
                                                         rdfs:label "carries"@en .


<http://iflastandards.info/ns/fr/frbr/frbroo/R6i_is_carried_by> rdfs:comment """
"""@en ;
                                                                rdfs:label "is carried by"@en .


<http://iflastandards.info/ns/fr/frbr/frbroo/R7_is_example_of> rdfs:comment """This property associates a publication with one of its exemplars.
It is a shortcut of the more developed path: F5 Item R28i was produced by F32 Carrier Production R26 produced things of type (was produced by): F3 Manifestation Product Type.
"""@en ;
                                                               rdfs:label "is example of"@en .


<http://iflastandards.info/ns/fr/frbr/frbroo/R7i_has_example> rdfs:comment """
"""@en ;
                                                              rdfs:label "has example"@en .


<http://iflastandards.info/ns/fr/frbr/frbroo/R8_consists_of> rdfs:comment """This property associates an instance of F13 Identifier with one of the non-syntactic instances of E90 Symbolic Object which form part of it.
"""@en ;
                                                             rdfs:label "consists of"@en .


<http://iflastandards.info/ns/fr/frbr/frbroo/R8i_forms_part_of> rdfs:comment """
"""@en ;
                                                                rdfs:label "forms part of"@en .


<http://iflastandards.info/ns/fr/frbr/frbroo/R9_is_realised_in> rdfs:comment """This property associates an F14 Individual Work with the unique F22 Self-Contained Expression that completely conveys it.
It is a shortcut for the more developed path: F14 Individual Work R19i was realised through F28 Expression Creation R17 created F22 Self-Contained Expression.
"""@en ;
                                                                rdfs:label "is realised in"@en .


<http://iflastandards.info/ns/fr/frbr/frbroo/R9i_realises> rdfs:comment """
"""@en ;
                                                           rdfs:label "realises"@en .


###  Generated by the OWL API (version 5.1.14) https://github.com/owlcs/owlapi/
